# PLEASE DO NOT EDIT THIS CODE!
# This code was generated by the Eclipse Acceleo module UCMIS M2T on 2023-05-25 10:41:35.
# Target language is 'Ontology Turtle' ('onto.ttl') generated on the basis of the model 'DDICDIModels'.

# Ontology for Agents
# based on the UML package DDICDIModels::DDICDILibrary::Classes::Agents
@prefix rdf:   <http://www.w3.org/1999/02/22-rdf-syntax-ns#> .
@prefix rdfs:  <http://www.w3.org/2000/01/rdf-schema#> .
@prefix owl:   <http://www.w3.org/2002/07/owl#> .
@prefix xsd:   <http://www.w3.org/2001/XMLSchema#> .
@prefix dc:    <http://purl.org/dc/elements/1.1/> .
@prefix skos:  <http://www.w3.org/2004/02/skos/core#> .
@prefix ucmis: <http://example.org/TODO/ucmis/> .
@prefix cdi:   <http://ddialliance.org/Specification/DDI-CDI/1.0/RDF/> .

<Agents.onto.ttl> a owl:Ontology;
  rdfs:label "Agents";
  rdfs:comment "This package contains classes which define the various types of actors which exist in the DDI-CDI Library, along with their supporting classes."@en;
.

# class Agent
# based on the UML class DDICDIModels::DDICDILibrary::Classes::Agents::Agent
cdi:Agent
  a rdfs:Class, owl:Class, ucmis:Class;
  rdfs:label "Agent";
  rdfs:comment "Definition\n==========\nActor that performs a role in relation to a process or product.\n\nExamples\n========\nAnalyst performing edits on data, interviewer conducting an interview, a relational database management system managing data, organization publishing data on a regular basis, creator or contributor of a publication.\n\nExplanatory notes\n=================\nfoaf:Agent is: An agent (eg. person, group, software or physical artifact). prov:Agent is: An agent is something that bears some form of responsibility for an activity taking place, for the existence of an entity, or for another agent's activity."@en;
  
.

cdi:Agent-catalogDetails
  a rdf:Property, owl:ObjectProperty, ucmis:Attribute;
  rdfs:label "catalogDetails";
  rdfs:comment "Bundles the information useful for a data catalog entry. Examples would be creator, contributor, title, copyright, embargo, and license information. A set of information useful for attribution, data discovery, and access. This is information that is tied to the identity of the object. If this information changes the version of the associated object changes."@en;
  rdfs:domain cdi:Agent;
  rdfs:range cdi:CatalogDetails;
.

cdi:Agent-identifier
  a rdf:Property, owl:ObjectProperty, ucmis:Attribute;
  rdfs:label "identifier";
  rdfs:comment "Identifier for objects requiring short- or long-lasting referencing and management."@en;
  rdfs:domain cdi:Agent;
  rdfs:range cdi:Identifier;
.

cdi:Agent-image
  a rdf:Property, owl:ObjectProperty, ucmis:Attribute;
  rdfs:label "image";
  rdfs:comment "Information regarding image associated with the agent."@en;
  rdfs:domain cdi:Agent;
  rdfs:range cdi:PrivateImage;
.

cdi:Agent-purpose
  a rdf:Property, owl:ObjectProperty, ucmis:Attribute;
  rdfs:label "purpose";
  rdfs:comment "Intent or reason for the object/the description of the object."@en;
  rdfs:domain cdi:Agent;
  rdfs:range cdi:InternationalString;
.



# class AgentListing
# based on the UML class DDICDIModels::DDICDILibrary::Classes::Agents::AgentListing
cdi:AgentListing
  a rdfs:Class, owl:Class, ucmis:Class;
  rdfs:label "AgentListing";
  rdfs:comment "Definition \n============ \nListing of agents of any type who may be organized to describe relationships between agents.  \n\nExamples \n========== \nOrganizations contributing to a project. Individuals within an agency. All organizations, individuals, and machines identified within the collections of an archive. A listing of organizations contributing to a network for the purposes of providing data.\n\nExplanatory notes \n=================== \nRelationships between agents are fluid and reflect effective dates of the relationship. An agent may have multiple relationships which may be sequential or concurrent. Relationships may or may not be hierarchical in nature. All Agents are serialized individually and brought into relationships as appropriate."@en;
  
.

cdi:AgentListing-allowsDuplicates
  a rdf:Property, owl:DatatypeProperty, ucmis:Attribute;
  rdfs:label "allowsDuplicates";
  rdfs:comment "If value is False, the members are unique within the collection - if True, there may be duplicates. (Note that a mathematical \"bag\" permits duplicates and is unordered - a \"set\" does not have duplicates and may be ordered.)"@en;
  rdfs:domain cdi:AgentListing;
  rdfs:range xsd:boolean;
.

cdi:AgentListing-identifier
  a rdf:Property, owl:ObjectProperty, ucmis:Attribute;
  rdfs:label "identifier";
  rdfs:comment "Identifier for objects requiring short- or long-lasting referencing and management."@en;
  rdfs:domain cdi:AgentListing;
  rdfs:range cdi:Identifier;
.

cdi:AgentListing-name
  a rdf:Property, owl:ObjectProperty, ucmis:Attribute;
  rdfs:label "name";
  rdfs:comment "Human understandable name (liguistic signifier, word, phrase, or mnemonic). May follow ISO/IEC 11179-5 naming principles, and have context provided to specify usage."@en;
  rdfs:domain cdi:AgentListing;
  rdfs:range cdi:ObjectName;
.

cdi:AgentListing-purpose
  a rdf:Property, owl:ObjectProperty, ucmis:Attribute;
  rdfs:label "purpose";
  rdfs:comment "Intent or reason for the object/the description of the object."@en;
  rdfs:domain cdi:AgentListing;
  rdfs:range cdi:InternationalString;
.


cdi:AgentListing_has_Agent
  a rdf:Property, owl:ObjectProperty, ucmis:Association;
  # ASSOCIATION
  rdfs:label "has";
  skos:altLabel "AgentListing_has_Agent";
  
  rdfs:domain cdi:AgentListing;
  rdfs:range cdi:Agent;
.

cdi:AgentListing_has_AgentPosition
  a rdf:Property, owl:ObjectProperty, ucmis:Association;
  # ASSOCIATION
  rdfs:label "has";
  skos:altLabel "AgentListing_has_AgentPosition";
  
  rdfs:domain cdi:AgentListing;
  rdfs:range cdi:AgentPosition;
.

cdi:AgentListing_isDefinedBy_Concept
  a rdf:Property, owl:ObjectProperty, ucmis:Association;
  # ASSOCIATION
  rdfs:label "isDefinedBy";
  skos:altLabel "AgentListing_isDefinedBy_Concept";
  rdfs:comment "The conceptual basis for the collection of members."@en;
  rdfs:domain cdi:AgentListing;
  rdfs:range cdi:Concept;
.

cdi:AgentListing_isMaintainedBy_Agent
  a rdf:Property, owl:ObjectProperty, ucmis:Association;
  # ASSOCIATION
  rdfs:label "isMaintainedBy";
  skos:altLabel "AgentListing_isMaintainedBy_Agent";
  rdfs:comment "The unit or group of persons within the organization responsible for the agent listing (i.e., for adding, changing or deleting agent entries)."@en;
  rdfs:domain cdi:AgentListing;
  rdfs:range cdi:Agent;
.


# class AgentPosition
# based on the UML class DDICDIModels::DDICDILibrary::Classes::Agents::AgentPosition
cdi:AgentPosition
  a rdfs:Class, owl:Class, ucmis:Class;
  rdfs:label "AgentPosition";
  rdfs:comment "Definition \n============ \nAssigns a sequence number to an agent in an agent listing."@en;
  
.

cdi:AgentPosition-identifier
  a rdf:Property, owl:ObjectProperty, ucmis:Attribute;
  rdfs:label "identifier";
  rdfs:comment "Identifier for objects requiring short- or long-lasting referencing and management."@en;
  rdfs:domain cdi:AgentPosition;
  rdfs:range cdi:Identifier;
.

cdi:AgentPosition-value
  a rdf:Property, owl:DatatypeProperty, ucmis:Attribute;
  rdfs:label "value";
  rdfs:comment "The index of the agent within an agent listing."@en;
  rdfs:domain cdi:AgentPosition;
  rdfs:range xsd:integer;
.


cdi:AgentPosition_indexes_Agent
  a rdf:Property, owl:ObjectProperty, ucmis:Association;
  # ASSOCIATION
  rdfs:label "indexes";
  skos:altLabel "AgentPosition_indexes_Agent";
  
  rdfs:domain cdi:AgentPosition;
  rdfs:range cdi:Agent;
.


# class AgentRelationship
# based on the UML class DDICDIModels::DDICDILibrary::Classes::Agents::AgentRelationship
cdi:AgentRelationship
  a rdfs:Class, owl:Class, ucmis:Class;
  rdfs:label "AgentRelationship";
  rdfs:comment "Definition \n============ \nDefines the relation of an agent within a structure.  \n\nExamples \n========== \nAn organization (source/parent) employing an individual (target/child); An individual (source/parent) supervisory to an individual (target/child); An organization (source/parent) overseeing a project (organization) (target/child). Select appropriate relationship using the controlled vocabulary available through the semantics attribute.   \n\nExplanatory notes \n=================== \nUsed to define the relations of agents in a hierarchical structure, or in other networks. Projects can be understood as temporary organizations."@en;
  
.

cdi:AgentRelationship-effectiveDates
  a rdf:Property, owl:ObjectProperty, ucmis:Attribute;
  rdfs:label "effectiveDates";
  rdfs:comment "Effective dates of the relationship expressed as a start and end Date (using ISO and/or non-ISO date structures)."@en;
  rdfs:domain cdi:AgentRelationship;
  rdfs:range cdi:DateRange;
.

cdi:AgentRelationship-identifier
  a rdf:Property, owl:ObjectProperty, ucmis:Attribute;
  rdfs:label "identifier";
  rdfs:comment "Identifier for objects requiring short- or long-lasting referencing and management."@en;
  rdfs:domain cdi:AgentRelationship;
  rdfs:range cdi:Identifier;
.

cdi:AgentRelationship-semantics
  a rdf:Property, owl:ObjectProperty, ucmis:Attribute;
  rdfs:label "semantics";
  rdfs:comment "Specifies the semantics of the object in reference to a vocabulary, ontology, etc."@en;
  rdfs:domain cdi:AgentRelationship;
  rdfs:range cdi:ControlledVocabularyEntry;
.


cdi:AgentRelationship_hasSource_Agent
  a rdf:Property, owl:ObjectProperty, ucmis:Association;
  # ASSOCIATION
  rdfs:label "hasSource";
  skos:altLabel "AgentRelationship_hasSource_Agent";
  rdfs:comment "The subject in the description of a paired relationship â€“ for example the Parent agent in the hierarchical Parent of Child relationship."@en;
  rdfs:domain cdi:AgentRelationship;
  rdfs:range cdi:Agent;
.

cdi:AgentRelationship_hasTarget_Agent
  a rdf:Property, owl:ObjectProperty, ucmis:Association;
  # ASSOCIATION
  rdfs:label "hasTarget";
  skos:altLabel "AgentRelationship_hasTarget_Agent";
  rdfs:comment "The object in the description of a paired relationship â€“ for example the Object agent in the hierarchical Parent of Child relationship."@en;
  rdfs:domain cdi:AgentRelationship;
  rdfs:range cdi:Agent;
.


# class AgentStructure
# based on the UML class DDICDIModels::DDICDILibrary::Classes::Agents::AgentStructure
cdi:AgentStructure
  a rdfs:Class, owl:Class, ucmis:Class;
  rdfs:label "AgentStructure";
  rdfs:comment "Definition \n============ \nDefines the relationships between agents in a collection for a specified period and purpose.  \n\nExamples \n========== \nIndividual employed by an organization. A unit or project (organization) within another organization. Individual supervised by another individual.  \n\nExplanatory notes \n=================== \nCan describe relations between agents rather than roles within a project or in relationship to a product. Roles are defined by the parent class and relationship name that uses an agent as a target."@en;
  
.

cdi:AgentStructure-effectiveDates
  a rdf:Property, owl:ObjectProperty, ucmis:Attribute;
  rdfs:label "effectiveDates";
  rdfs:comment "The effective start and end date of the relationship."@en;
  rdfs:domain cdi:AgentStructure;
  rdfs:range cdi:DateRange;
.

cdi:AgentStructure-identifier
  a rdf:Property, owl:ObjectProperty, ucmis:Attribute;
  rdfs:label "identifier";
  rdfs:comment "Identifier for objects requiring short- or long-lasting referencing and management."@en;
  rdfs:domain cdi:AgentStructure;
  rdfs:range cdi:Identifier;
.

cdi:AgentStructure-name
  a rdf:Property, owl:ObjectProperty, ucmis:Attribute;
  rdfs:label "name";
  rdfs:comment "Human understandable name (liguistic signifier, word, phrase, or mnemonic). May follow ISO/IEC 11179-5 naming principles, and have context provided to specify usage."@en;
  rdfs:domain cdi:AgentStructure;
  rdfs:range cdi:ObjectName;
.

cdi:AgentStructure-privacy
  a rdf:Property, owl:ObjectProperty, ucmis:Attribute;
  rdfs:label "privacy";
  rdfs:comment "Level of privacy regarding this relationship."@en;
  rdfs:domain cdi:AgentStructure;
  rdfs:range cdi:ControlledVocabularyEntry;
.

cdi:AgentStructure-purpose
  a rdf:Property, owl:ObjectProperty, ucmis:Attribute;
  rdfs:label "purpose";
  rdfs:comment "Intent or reason for the object/the description of the object."@en;
  rdfs:domain cdi:AgentStructure;
  rdfs:range cdi:InternationalString;
.

cdi:AgentStructure-semantics
  a rdf:Property, owl:ObjectProperty, ucmis:Attribute;
  rdfs:label "semantics";
  rdfs:comment "Specifies the semantics of the object in reference to a vocabulary, ontology, etc."@en;
  rdfs:domain cdi:AgentStructure;
  rdfs:range cdi:ControlledVocabularyEntry;
.

cdi:AgentStructure-specification
  a rdf:Property, owl:ObjectProperty, ucmis:Attribute;
  rdfs:label "specification";
  rdfs:comment "Provides information on reflexivity, transitivity, and symmetry of relationship using a descriptive term from an enumerated list. Use if all relations within this relation structure are of the same specification."@en;
  rdfs:domain cdi:AgentStructure;
  rdfs:range cdi:StructureSpecification;
.

cdi:AgentStructure-topology
  a rdf:Property, owl:ObjectProperty, ucmis:Attribute;
  rdfs:label "topology";
  rdfs:comment "Indicates the form of the associations among members of the collection. Specifies the way in which constituent parts are interrelated or arranged."@en;
  rdfs:domain cdi:AgentStructure;
  rdfs:range cdi:ControlledVocabularyEntry;
.

cdi:AgentStructure-totality
  a rdf:Property, owl:ObjectProperty, ucmis:Attribute;
  rdfs:label "totality";
  rdfs:comment "Indicates whether the related collections are comprehensive in terms of their coverage."@en;
  rdfs:domain cdi:AgentStructure;
  rdfs:range cdi:StructureExtent;
.


cdi:AgentStructure_has_AgentRelationship
  a rdf:Property, owl:ObjectProperty, ucmis:Association;
  # ASSOCIATION
  rdfs:label "has";
  skos:altLabel "AgentStructure_has_AgentRelationship";
  
  rdfs:domain cdi:AgentStructure;
  rdfs:range cdi:AgentRelationship;
.

cdi:AgentStructure_structures_AgentListing
  a rdf:Property, owl:ObjectProperty, ucmis:Association;
  # ASSOCIATION
  rdfs:label "structures";
  skos:altLabel "AgentStructure_structures_AgentListing";
  
  rdfs:domain cdi:AgentStructure;
  rdfs:range cdi:AgentListing;
.


# class Individual
# based on the UML class DDICDIModels::DDICDILibrary::Classes::Agents::Individual
cdi:Individual
  a rdfs:Class, owl:Class, ucmis:Class;
  rdfs:label "Individual";
  rdfs:comment "Definition \n============ \nA person. (See for example the W3C Friend of a Friend Ontology - http://xmlns.com/foaf/spec/#term_Person).\n\nExamples \n========== \nIndividual employed by an organization. A person within a unit or project (organization). Albert Einstein, Bugs Bunny, Harry Potter, Ashley G. Williams, Gandalf.  \n\nExplanatory notes \n=================== \nDescribes people referred to in the description of data and process. Similar to the concept found in Schema.org, the W3C ORG Ontology, etc."@en;
  rdfs:subClassOf cdi:Agent;
.

cdi:Individual-contactInformation
  a rdf:Property, owl:ObjectProperty, ucmis:Attribute;
  rdfs:label "contactInformation";
  rdfs:comment "Contact information for the individual including location specification, address, URL, phone numbers, and other means of communication access. Sets of information can be repeated and date-stamped."@en;
  rdfs:domain cdi:Individual;
  rdfs:range cdi:ContactInformation;
.

cdi:Individual-individualName
  a rdf:Property, owl:ObjectProperty, ucmis:Attribute;
  rdfs:label "individualName";
  rdfs:comment "Name of an individual broken out into its component parts of prefix, first/given name, middle name, last/family/surname, and suffix."@en;
  rdfs:domain cdi:Individual;
  rdfs:range cdi:IndividualName;
.



# class Machine
# based on the UML class DDICDIModels::DDICDILibrary::Classes::Agents::Machine
cdi:Machine
  a rdfs:Class, owl:Class, ucmis:Class;
  rdfs:label "Machine";
  rdfs:comment "Definition\n============\nMechanism or computer program used to perform an act.\n\nExamples\n==========\nSAS program, photocopier\n\nExplanatory notes\n===================\nMay be used as a target to identify the agent who performed an action. Used to define hardware or software that act as agents in data capture, data processing, or other related actions."@en;
  rdfs:subClassOf cdi:Agent;
.

cdi:Machine-accessLocation
  a rdf:Property, owl:ObjectProperty, ucmis:Attribute;
  rdfs:label "accessLocation";
  rdfs:comment "Location of the machine for the purpose of access."@en;
  rdfs:domain cdi:Machine;
  rdfs:range cdi:AccessLocation;
.

cdi:Machine-function
  a rdf:Property, owl:ObjectProperty, ucmis:Attribute;
  rdfs:label "function";
  rdfs:comment "The business function of the machine according to a classification or typology."@en;
  rdfs:domain cdi:Machine;
  rdfs:range cdi:ControlledVocabularyEntry;
.

cdi:Machine-machineInterface
  a rdf:Property, owl:ObjectProperty, ucmis:Attribute;
  rdfs:label "machineInterface";
  rdfs:comment "Reference to the type of the machine interface according to a classification or typology."@en;
  rdfs:domain cdi:Machine;
  rdfs:range cdi:ControlledVocabularyEntry;
.

cdi:Machine-name
  a rdf:Property, owl:ObjectProperty, ucmis:Attribute;
  rdfs:label "name";
  rdfs:comment "Human understandable name (liguistic signifier, word, phrase, or mnemonic). May follow ISO/IEC 11179-5 naming principles, and have context provided to specify usage."@en;
  rdfs:domain cdi:Machine;
  rdfs:range cdi:ObjectName;
.

cdi:Machine-ownerOperatorContact
  a rdf:Property, owl:ObjectProperty, ucmis:Attribute;
  rdfs:label "ownerOperatorContact";
  rdfs:comment "Contact information for the owner/operator including location specification, address, URL, phone numbers, and other means of communication access. Sets of information can be repeated and date-stamped."@en;
  rdfs:domain cdi:Machine;
  rdfs:range cdi:ContactInformation;
.

cdi:Machine-typeOfMachine
  a rdf:Property, owl:ObjectProperty, ucmis:Attribute;
  rdfs:label "typeOfMachine";
  rdfs:comment "Describes the type of non-human actor (e.g., software, hardware, web service, etc.)."@en;
  rdfs:domain cdi:Machine;
  rdfs:range cdi:ControlledVocabularyEntry;
.



# class Organization
# based on the UML class DDICDIModels::DDICDILibrary::Classes::Agents::Organization
cdi:Organization
  a rdfs:Class, owl:Class, ucmis:Class;
  rdfs:label "Organization";
  rdfs:comment "Definition \n========== \nCollection of people organized within a framework of authority that can perform an act or be associated with another agent.  \n\nExamples \n========== \nCommonwealth Scientific and Industrial Research Organisation (CSIRO), U.S. Census Bureau, University of Michigan/Institute for Social Research, Research Data Alliance Agrisemantics Working Group.  \n\nExplanatory notes \n=================\nThe W3C Organization Ontology (https://www.w3.org/TR/vocab-org/#organizational_structure) definition: \"Represents a collection of people organized together into a community or other social, commercial or political structure. The group has some common purpose or reason for existence which goes beyond the set of people belonging to it and can act as an agent. Organizations are often decomposable into hierarchical structures.\""@en;
  rdfs:subClassOf cdi:Agent;
.

cdi:Organization-contactInformation
  a rdf:Property, owl:ObjectProperty, ucmis:Attribute;
  rdfs:label "contactInformation";
  rdfs:comment "Contact information for the organization including location specification, address, URL, phone numbers, and other means of communication access. Sets of information can be repeated and date-stamped."@en;
  rdfs:domain cdi:Organization;
  rdfs:range cdi:ContactInformation;
.

cdi:Organization-organizationName
  a rdf:Property, owl:ObjectProperty, ucmis:Attribute;
  rdfs:label "organizationName";
  rdfs:comment "Names by which the organization is known."@en;
  rdfs:domain cdi:Organization;
  rdfs:range cdi:OrganizationName;
.





