# PLEASE DO NOT EDIT THIS CODE!
# This code was generated by the Eclipse Acceleo module UCMIS M2T on 2024-03-16 23:40:16.
# Target language is 'Ontology Turtle' ('onto.ttl') generated on the basis of the model 'DDICDIModels'.

# Ontology for Dimensional
# based on the UML package DDICDIModels::DDICDILibrary::Classes::DataDescription::Dimensional
@prefix rdf:   <http://www.w3.org/1999/02/22-rdf-syntax-ns#> .
@prefix rdfs:  <http://www.w3.org/2000/01/rdf-schema#> .
@prefix owl:   <http://www.w3.org/2002/07/owl#> .
@prefix xsd:   <http://www.w3.org/2001/XMLSchema#> .
@prefix dc:    <http://purl.org/dc/elements/1.1/> .
@prefix skos:  <http://www.w3.org/2004/02/skos/core#> .
@prefix ucmis: <http://example.org/TODO/ucmis/> .
@prefix cdi:   <http://ddialliance.org/Specification/DDI-CDI/1.0/RDF/> .

<Dimensional.onto.ttl> a owl:Ontology;
  rdfs:label "Dimensional";
  rdfs:comment "This package contains the classes which are used to define multi-dimensional data structures (i.e., data cubes). It is important to note that the logical treatment of data as a multi-dimensional structure does not necessarily dictate a particular physical format for the data."@en;
.

# class DimensionalDataSet
# based on the UML class DDICDIModels::DDICDILibrary::Classes::DataDescription::Dimensional::DimensionalDataSet
cdi:DimensionalDataSet
  a rdfs:Class, owl:Class, ucmis:Class;
  rdfs:label "DimensionalDataSet";
  rdfs:comment "Definition\n============\nOrganized collection of multidimensional data. It is structured by a dimensional data structure.\n\nExamples\n==========\nA dimensional dataset with Income values in each data point, where the dimensions organizing the data points are Sex and Marital Status.\n\nExplanatory notes\n===================\nSimilar to Structural N-Cube."@en;
  rdfs:subClassOf cdi:DataSet;
.

cdi:DimensionalDataSet-name
  a rdf:Property, owl:ObjectProperty, ucmis:Attribute;
  rdfs:label "name";
  rdfs:comment "Human understandable name (liguistic signifier, word, phrase, or mnemonic). May follow ISO/IEC 11179-5 naming principles, and have context provided to specify usage."@en;
  rdfs:domain cdi:DimensionalDataSet;
  rdfs:range cdi:ObjectName;
.


cdi:DimensionalDataSet_represents_ScopedMeasure
  a rdf:Property, owl:ObjectProperty, ucmis:Association;
  # ASSOCIATION
  rdfs:label "represents";
  skos:altLabel "DimensionalDataSet_represents_ScopedMeasure";
  
  rdfs:domain cdi:DimensionalDataSet;
  rdfs:range cdi:ScopedMeasure;
.


# class DimensionalDataStructure
# based on the UML class DDICDIModels::DDICDILibrary::Classes::DataDescription::Dimensional::DimensionalDataStructure
cdi:DimensionalDataStructure
  a rdfs:Class, owl:Class, ucmis:Class;
  rdfs:label "DimensionalDataStructure";
  rdfs:comment "Definition\n============\nStructure of a dimensional data set (organized collection of multidimensional data). It is described by dimension, measure and attribute components.\n\nExamples\n==========\nThe structure described by [City, Average Income, Total Population] where City is a dimension and Average Income and Total Population are measures."@en;
  rdfs:subClassOf cdi:DataStructure;
.


cdi:DimensionalDataStructure_uses_DimensionGroup
  a rdf:Property, owl:ObjectProperty, ucmis:Association;
  # ASSOCIATION
  rdfs:label "uses";
  skos:altLabel "DimensionalDataStructure_uses_DimensionGroup";
  
  rdfs:domain cdi:DimensionalDataStructure;
  rdfs:range cdi:DimensionGroup;
.


# class DimensionalKey
# based on the UML class DDICDIModels::DDICDILibrary::Classes::DataDescription::Dimensional::DimensionalKey
cdi:DimensionalKey
  a rdfs:Class, owl:Class, ucmis:Class;
  rdfs:label "DimensionalKey";
  rdfs:comment "Definition\n============\nCollection of data instances that uniquely identify a collection of data points in a dimensional dataset.\n\nExamples\n==========\nCollection of \"male\", \"Ontario\" and \"married\" strings in a dimensional dataset where data points are identified by Sex, Province and Marital Status dimensions."@en;
  rdfs:subClassOf cdi:Key;
.



# class DimensionalKeyDefinition
# based on the UML class DDICDIModels::DDICDILibrary::Classes::DataDescription::Dimensional::DimensionalKeyDefinition
cdi:DimensionalKeyDefinition
  a rdfs:Class, owl:Class, ucmis:Class;
  rdfs:label "DimensionalKeyDefinition";
  rdfs:comment "Definition\n============\nCollection of concepts that uniquely defines a collection of data points in a dimensional dataset.\n\nExamples\n==========\nCollection of [Male], [Ontario] and [Married] categories in a dimensional dataset where data points are defined by Sex, Province and Marital Status dimensions."@en;
  rdfs:subClassOf cdi:KeyDefinition;
.



# class DimensionalKeyDefinitionMember
# based on the UML class DDICDIModels::DDICDILibrary::Classes::DataDescription::Dimensional::DimensionalKeyDefinitionMember
cdi:DimensionalKeyDefinitionMember
  a rdfs:Class, owl:Class, ucmis:Class;
  rdfs:label "DimensionalKeyDefinitionMember";
  rdfs:comment "Definition\n============\nSingle concept that is part of a dimensional key definition.\n\nExamples\n==========\nThe [Ontario] category in a dimensional dataset where data points are defined by Province and other dimensions."@en;
  rdfs:subClassOf cdi:ConceptualValue;
.


cdi:DimensionalKeyDefinitionMember_isRepresentedBy_DimensionalKeyMember
  a rdf:Property, owl:ObjectProperty, ucmis:Association;
  # ASSOCIATION
  rdfs:label "isRepresentedBy";
  skos:altLabel "DimensionalKeyDefinitionMember_isRepresentedBy_DimensionalKeyMember";
  
  rdfs:domain cdi:DimensionalKeyDefinitionMember;
  rdfs:range cdi:DimensionalKeyMember;
.


# class DimensionalKeyMember
# based on the UML class DDICDIModels::DDICDILibrary::Classes::DataDescription::Dimensional::DimensionalKeyMember
cdi:DimensionalKeyMember
  a rdfs:Class, owl:Class, ucmis:Class;
  rdfs:label "DimensionalKeyMember";
  rdfs:comment "Definition\n============\nSingle data instance that is part of a dimensional key. \n\nExamples\n==========\nThe \"Ontario\" string in a dimensional dataset where data points are identified by Province and other dimensions."@en;
  rdfs:subClassOf cdi:KeyMember;
.


cdi:DimensionalKeyMember_hasValueFrom_CodeList
  a rdf:Property, owl:ObjectProperty, ucmis:Association;
  # ASSOCIATION
  rdfs:label "hasValueFrom";
  skos:altLabel "DimensionalKeyMember_hasValueFrom_CodeList";
  
  rdfs:domain cdi:DimensionalKeyMember;
  rdfs:range cdi:CodeList;
.


# class DimensionGroup
# based on the UML class DDICDIModels::DDICDILibrary::Classes::DataDescription::Dimensional::DimensionGroup
cdi:DimensionGroup
  a rdfs:Class, owl:Class, ucmis:Class;
  rdfs:label "DimensionGroup";
  rdfs:comment "Definition\n============\nCollection of dimensions that can be reused across multiple dimensional structures.\n\nExamples\n==========\nSex, Province and Marital Status is a common set of dimensions used across a variety of dimensional data structures and might need to be maintained separately."@en;
  
.

cdi:DimensionGroup-identifier
  a rdf:Property, owl:ObjectProperty, ucmis:Attribute;
  rdfs:label "identifier";
  rdfs:comment "Identifier for objects requiring short- or long-lasting referencing and management."@en;
  rdfs:domain cdi:DimensionGroup;
  rdfs:range cdi:Identifier;
.

cdi:DimensionGroup-name
  a rdf:Property, owl:ObjectProperty, ucmis:Attribute;
  rdfs:label "name";
  rdfs:comment "Human understandable name (liguistic signifier, word, phrase, or mnemonic). May follow ISO/IEC 11179-5 naming principles, and have context provided to specify usage."@en;
  rdfs:domain cdi:DimensionGroup;
  rdfs:range cdi:ObjectName;
.


cdi:DimensionGroup_has_DimensionComponent
  a rdf:Property, owl:ObjectProperty, ucmis:Association;
  # ASSOCIATION
  rdfs:label "has";
  skos:altLabel "DimensionGroup_has_DimensionComponent";
  
  rdfs:domain cdi:DimensionGroup;
  rdfs:range cdi:DimensionComponent;
.


# class QualifiedMeasure
# based on the UML class DDICDIModels::DDICDILibrary::Classes::DataDescription::Dimensional::QualifiedMeasure
cdi:QualifiedMeasure
  a rdfs:Class, owl:Class, ucmis:Class;
  rdfs:label "QualifiedMeasure";
  rdfs:comment "Definition\n============\nA measure having a specific production method. \n\nExamples\n==========\nSeasonally adjusted monthly income."@en;
  rdfs:subClassOf cdi:MeasureComponent;
.


cdi:QualifiedMeasure_refines_MeasureComponent
  a rdf:Property, owl:ObjectProperty, ucmis:Association;
  # ASSOCIATION
  rdfs:label "refines";
  skos:altLabel "QualifiedMeasure_refines_MeasureComponent";
  
  rdfs:domain cdi:QualifiedMeasure;
  rdfs:range cdi:MeasureComponent;
.


# class RevisableDatum
# based on the UML class DDICDIModels::DDICDILibrary::Classes::DataDescription::Dimensional::RevisableDatum
cdi:RevisableDatum
  a rdfs:Class, owl:Class, ucmis:Class;
  rdfs:label "RevisableDatum";
  rdfs:comment "Definition\n============\nA datum that can be qualified by a revision.\n\nExamples\n==========\nThe April datum for Income revised in June."@en;
  rdfs:subClassOf cdi:Datum;
.

cdi:RevisableDatum-vintage
  a rdf:Property, owl:DatatypeProperty, ucmis:Attribute;
  rdfs:label "vintage";
  rdfs:comment "A revision sequence number for a datum."@en;
  rdfs:domain cdi:RevisableDatum;
  rdfs:range xsd:integer;
.


cdi:RevisableDatum_correspondsTo_Revision
  a rdf:Property, owl:ObjectProperty, ucmis:Association;
  # ASSOCIATION
  rdfs:label "correspondsTo";
  skos:altLabel "RevisableDatum_correspondsTo_Revision";
  
  rdfs:domain cdi:RevisableDatum;
  rdfs:range cdi:Revision;
.


# class Revision
# based on the UML class DDICDIModels::DDICDILibrary::Classes::DataDescription::Dimensional::Revision
cdi:Revision
  a rdfs:Class, owl:Class, ucmis:Class;
  rdfs:label "Revision";
  rdfs:comment "Definition\n============\nAlgorithm applied to produce a revised datum.\n\nExamples\n==========\nAn adjustment to monthly employment numbers to adjust for errors (sampling or non-sampling) in the underlying data."@en;
  
.

cdi:Revision-algorithm
  a rdf:Property, owl:DatatypeProperty, ucmis:Attribute;
  rdfs:label "algorithm";
  rdfs:comment "Actual code or reference to specific algorithm"@en;
  rdfs:domain cdi:Revision;
  rdfs:range xsd:string;
.

cdi:Revision-identifier
  a rdf:Property, owl:ObjectProperty, ucmis:Attribute;
  rdfs:label "identifier";
  rdfs:comment "Identifier for objects requiring short- or long-lasting referencing and management."@en;
  rdfs:domain cdi:Revision;
  rdfs:range cdi:Identifier;
.

cdi:Revision-overview
  a rdf:Property, owl:ObjectProperty, ucmis:Attribute;
  rdfs:label "overview";
  rdfs:comment "Short natural language account of the information obtained from the combination of properties and relationships associated with an object."@en;
  rdfs:domain cdi:Revision;
  rdfs:range cdi:InternationalString;
.



# class ScopedMeasure
# based on the UML class DDICDIModels::DDICDILibrary::Classes::DataDescription::Dimensional::ScopedMeasure
cdi:ScopedMeasure
  a rdfs:Class, owl:Class, ucmis:Class;
  rdfs:label "ScopedMeasure";
  rdfs:comment "Definition\n==========\nA qualified measure whose domain is a universe as an aggregate, i.e. a measure with a specific production method applied to a specific cell in a cube.\n\nExamples\n========\nSeasonally adjusted income for Single, Ontarians, Females."@en;
  
.

cdi:ScopedMeasure-frequency
  a rdf:Property, owl:ObjectProperty, ucmis:Attribute;
  rdfs:label "frequency";
  rdfs:comment "Time interval between successive measurements (i.e. applications) of a Scoped Measure."@en;
  rdfs:domain cdi:ScopedMeasure;
  rdfs:range cdi:InternationalString;
.

cdi:ScopedMeasure-identifier
  a rdf:Property, owl:ObjectProperty, ucmis:Attribute;
  rdfs:label "identifier";
  rdfs:comment "Identifier for objects requiring short- or long-lasting referencing and management."@en;
  rdfs:domain cdi:ScopedMeasure;
  rdfs:range cdi:Identifier;
.


cdi:ScopedMeasure_circumscribes_DimensionalKeyDefinition
  a rdf:Property, owl:ObjectProperty, ucmis:Association;
  # ASSOCIATION
  rdfs:label "circumscribes";
  skos:altLabel "ScopedMeasure_circumscribes_DimensionalKeyDefinition";
  rdfs:comment "A universe is specific to the specific cell associated with a scoped measure."@en;
  rdfs:domain cdi:ScopedMeasure;
  rdfs:range cdi:DimensionalKeyDefinition;
.

cdi:ScopedMeasure_generates_RevisableDatum
  a rdf:Property, owl:ObjectProperty, ucmis:Association;
  # ASSOCIATION
  rdfs:label "generates";
  skos:altLabel "ScopedMeasure_generates_RevisableDatum";
  rdfs:comment "Scoped measure generates one revisable datum."@en;
  rdfs:domain cdi:ScopedMeasure;
  rdfs:range cdi:RevisableDatum;
.

cdi:ScopedMeasure_restricts_QualifiedMeasure
  a rdf:Property, owl:ObjectProperty, ucmis:Association;
  # ASSOCIATION
  rdfs:label "restricts";
  skos:altLabel "ScopedMeasure_restricts_QualifiedMeasure";
  rdfs:comment "A scoped measure resticts a qualified measure to a particular cell."@en;
  rdfs:domain cdi:ScopedMeasure;
  rdfs:range cdi:QualifiedMeasure;
.




