# PLEASE DO NOT EDIT THIS CODE!
# This code was generated by the Eclipse Acceleo module UCMIS M2T on 2023-05-25 10:41:35.
# Target language is 'Ontology Turtle' ('onto.ttl') generated on the basis of the model 'DDICDIModels'.

# Ontology for Representations
# based on the UML package DDICDIModels::DDICDILibrary::Classes::Representations
@prefix rdf:   <http://www.w3.org/1999/02/22-rdf-syntax-ns#> .
@prefix rdfs:  <http://www.w3.org/2000/01/rdf-schema#> .
@prefix owl:   <http://www.w3.org/2002/07/owl#> .
@prefix xsd:   <http://www.w3.org/2001/XMLSchema#> .
@prefix dc:    <http://purl.org/dc/elements/1.1/> .
@prefix skos:  <http://www.w3.org/2004/02/skos/core#> .
@prefix ucmis: <http://example.org/TODO/ucmis/> .
@prefix cdi:   <http://ddialliance.org/Specification/DDI-CDI/1.0/RDF/> .

<Representations.onto.ttl> a owl:Ontology;
  rdfs:label "Representations";
  rdfs:comment "This package contains classes for describing the representation of values and meaning within data."@en;
.

# class AuthorizationSource
# based on the UML class DDICDIModels::DDICDILibrary::Classes::Representations::AuthorizationSource
cdi:AuthorizationSource
  a rdfs:Class, owl:Class, ucmis:Class;
  rdfs:label "AuthorizationSource";
  rdfs:comment "Definition \n============ \nIdentifies the authorizing agency and allows for the full text of the authorization (law, regulation, or other form of authorization).  \n\nExamples \n========== \nMay be used to list authorizations from oversight committees and other regulatory agencies.  \n\nExplanatory notes \n=================== \nSupports requirements for some statistical offices to identify the agency or law authorizing the collection or management of data or metadata."@en;
  
.

cdi:AuthorizationSource-authorizationDate
  a rdf:Property, owl:ObjectProperty, ucmis:Attribute;
  rdfs:label "authorizationDate";
  rdfs:comment "Identifies the date of authorization."@en;
  rdfs:domain cdi:AuthorizationSource;
  rdfs:range cdi:CombinedDate;
.

cdi:AuthorizationSource-catalogDetails
  a rdf:Property, owl:ObjectProperty, ucmis:Attribute;
  rdfs:label "catalogDetails";
  rdfs:comment "Bundles the information useful for a data catalog entry. \n\nExamples would be creator, contributor, title, copyright, embargo, and license information\n\nA set of information useful for attribution, data discovery, and access.\nThis is information that is tied to the identity of the object. If this information changes the version of the associated object changes."@en;
  rdfs:domain cdi:AuthorizationSource;
  rdfs:range cdi:CatalogDetails;
.

cdi:AuthorizationSource-identifier
  a rdf:Property, owl:ObjectProperty, ucmis:Attribute;
  rdfs:label "identifier";
  rdfs:comment "Identifier for objects requiring short- or long-lasting referencing and management."@en;
  rdfs:domain cdi:AuthorizationSource;
  rdfs:range cdi:Identifier;
.

cdi:AuthorizationSource-legalMandate
  a rdf:Property, owl:ObjectProperty, ucmis:Attribute;
  rdfs:label "legalMandate";
  rdfs:comment "Provide a legal citation to a law authorizing the study/data collection. For example, a legal citation for a law authorizing a country's census."@en;
  rdfs:domain cdi:AuthorizationSource;
  rdfs:range cdi:InternationalString;
.

cdi:AuthorizationSource-purpose
  a rdf:Property, owl:ObjectProperty, ucmis:Attribute;
  rdfs:label "purpose";
  rdfs:comment "Intent or reason for the object/the description of the object."@en;
  rdfs:domain cdi:AuthorizationSource;
  rdfs:range cdi:InternationalString;
.

cdi:AuthorizationSource-statementOfAuthorization
  a rdf:Property, owl:ObjectProperty, ucmis:Attribute;
  rdfs:label "statementOfAuthorization";
  rdfs:comment "Text of the authorization (law, mandate, approved business case)."@en;
  rdfs:domain cdi:AuthorizationSource;
  rdfs:range cdi:InternationalString;
.


cdi:AuthorizationSource_has_Agent
  a rdf:Property, owl:ObjectProperty, ucmis:Association;
  # ASSOCIATION
  rdfs:label "has";
  skos:altLabel "AuthorizationSource_has_Agent";
  
  rdfs:domain cdi:AuthorizationSource;
  rdfs:range cdi:Agent;
.


# class CategoryStatistic
# based on the UML class DDICDIModels::DDICDILibrary::Classes::Representations::CategoryStatistic
cdi:CategoryStatistic
  a rdfs:Class, owl:Class, ucmis:Class;
  rdfs:label "CategoryStatistic";
  rdfs:comment "Definition \n============ \nStatistics related to a specific category of an instance variable within a data set.  \n\nExamples \n========== \nThe percentage of females from a demographic data set.   \n\nExplanatory notes \n=================== \nStatistics at the data set are used as indicators during assessment of the appropriateness of using a some data for a particular purpose."@en;
  
.

cdi:CategoryStatistic-identifier
  a rdf:Property, owl:ObjectProperty, ucmis:Attribute;
  rdfs:label "identifier";
  rdfs:comment "Identifier for objects requiring short- or long-lasting referencing and management."@en;
  rdfs:domain cdi:CategoryStatistic;
  rdfs:range cdi:Identifier;
.

cdi:CategoryStatistic-statistic
  a rdf:Property, owl:ObjectProperty, ucmis:Attribute;
  rdfs:label "statistic";
  rdfs:comment "The value of the identified type of statistic for the category. May be repeated to provide unweighted or weighted values and different computation bases."@en;
  rdfs:domain cdi:CategoryStatistic;
  rdfs:range cdi:Statistic;
.

cdi:CategoryStatistic-typeOfCategoryStatistic
  a rdf:Property, owl:ObjectProperty, ucmis:Attribute;
  rdfs:label "typeOfCategoryStatistic";
  rdfs:comment "Indicates the type of information about the appearance of categories within the instance variable."@en;
  rdfs:domain cdi:CategoryStatistic;
  rdfs:range cdi:ControlledVocabularyEntry;
.


cdi:CategoryStatistic_appliesTo_InstanceVariable
  a rdf:Property, owl:ObjectProperty, ucmis:Association;
  # ASSOCIATION
  rdfs:label "appliesTo";
  skos:altLabel "CategoryStatistic_appliesTo_InstanceVariable";
  
  rdfs:domain cdi:CategoryStatistic;
  rdfs:range cdi:InstanceVariable;
.

cdi:CategoryStatistic_for_Category
  a rdf:Property, owl:ObjectProperty, ucmis:Association;
  # ASSOCIATION
  rdfs:label "for";
  skos:altLabel "CategoryStatistic_for_Category";
  
  rdfs:domain cdi:CategoryStatistic;
  rdfs:range cdi:Category;
.


# class ClassificationFamily
# based on the UML class DDICDIModels::DDICDILibrary::Classes::Representations::ClassificationFamily
cdi:ClassificationFamily
  a rdfs:Class, owl:Class, ucmis:Class;
  rdfs:label "ClassificationFamily";
  rdfs:comment "Definition\n============\nCollection of classification series related by being based on a common concept\n\nExamples\n==========\nA set of classification series (e.g., International Standard Industrial Classification (ISIC) and North American Industrial Classification System (NAICS)) based on the same concept - economic activity or industry.\n\nExplanatory notes\n===================\nDifferent classification databases may use different types of classification families and have different names for the families, as no standard has been agreed upon. [GSIM1.1] This is documented by the definingConcept relationship   (e.g. economic activity).[GSIM1.1]."@en;
  
.

cdi:ClassificationFamily-catalogDetails
  a rdf:Property, owl:ObjectProperty, ucmis:Attribute;
  rdfs:label "catalogDetails";
  rdfs:comment "Bundles the information useful for a data catalog entry. \n\nExamples would be creator, contributor, title, copyright, embargo, and license information\n\nA set of information useful for attribution, data discovery, and access.\nThis is information that is tied to the identity of the object. If this information changes the version of the associated object changes."@en;
  rdfs:domain cdi:ClassificationFamily;
  rdfs:range cdi:CatalogDetails;
.

cdi:ClassificationFamily-identifier
  a rdf:Property, owl:ObjectProperty, ucmis:Attribute;
  rdfs:label "identifier";
  rdfs:comment "Identifier for objects requiring short- or long-lasting referencing and management."@en;
  rdfs:domain cdi:ClassificationFamily;
  rdfs:range cdi:Identifier;
.

cdi:ClassificationFamily-name
  a rdf:Property, owl:ObjectProperty, ucmis:Attribute;
  rdfs:label "name";
  rdfs:comment "Human understandable name (liguistic signifier, word, phrase, or mnemonic). May follow ISO/IEC 11179-5 naming principles, and have context provided to specify usage."@en;
  rdfs:domain cdi:ClassificationFamily;
  rdfs:range cdi:ObjectName;
.

cdi:ClassificationFamily-purpose
  a rdf:Property, owl:ObjectProperty, ucmis:Attribute;
  rdfs:label "purpose";
  rdfs:comment "Intent or reason for the object/the description of the object."@en;
  rdfs:domain cdi:ClassificationFamily;
  rdfs:range cdi:InternationalString;
.


cdi:ClassificationFamily_isDefinedBy_Concept
  a rdf:Property, owl:ObjectProperty, ucmis:Association;
  # ASSOCIATION
  rdfs:label "isDefinedBy";
  skos:altLabel "ClassificationFamily_isDefinedBy_Concept";
  rdfs:comment "The conceptual basis for the collection of members."@en;
  rdfs:domain cdi:ClassificationFamily;
  rdfs:range cdi:Concept;
.

cdi:ClassificationFamily_groups_ClassificationSeries
  a rdf:Property, owl:ObjectProperty, ucmis:Association;
  # ASSOCIATION
  rdfs:label "groups";
  skos:altLabel "ClassificationFamily_groups_ClassificationSeries";
  
  rdfs:domain cdi:ClassificationFamily;
  rdfs:range cdi:ClassificationSeries;
.

cdi:ClassificationFamily_uses_ClassificationIndex
  a rdf:Property, owl:ObjectProperty, ucmis:Association;
  # ASSOCIATION
  rdfs:label "uses";
  skos:altLabel "ClassificationFamily_uses_ClassificationIndex";
  rdfs:comment "Classification indexes associated to the classification family."@en;
  rdfs:domain cdi:ClassificationFamily;
  rdfs:range cdi:ClassificationIndex;
.


# class ClassificationIndex
# based on the UML class DDICDIModels::DDICDILibrary::Classes::Representations::ClassificationIndex
cdi:ClassificationIndex
  a rdfs:Class, owl:Class, ucmis:Class;
  rdfs:label "ClassificationIndex";
  rdfs:comment "Definition \n============ \nOrdered list of classification index entries. \n\nExamples \n========== \nAn alphabetical index of a topically ordered statistical classification.  \n\nExplanatory notes \n=================== \nA classification index shows the relationship between text found in statistical data sources (responses to survey questionnaires, administrative records) and one or more statistical classifications.  A classification index may be used to assign the codes for classification items to observations in statistical collections. Note that a GenericStatistical Information Model (GSIM) Node is the equivalent of a DDI-CDI Member, and a GSIM Node Set is a DDI-CDI Collection. A classification index can relate to one particular or to several statistical classifications. (See the GSIM Statistical Classification Model: https://statswiki.unece.org/display/gsim/Statistical+Classification+Model.)"@en;
  
.

cdi:ClassificationIndex-allowsDuplicates
  a rdf:Property, owl:DatatypeProperty, ucmis:Attribute;
  rdfs:label "allowsDuplicates";
  rdfs:comment "If value is False, the members are unique within the collection - if True, there may be duplicates. (Note that a mathematical “bag” permits duplicates and is unordered - a “set” does not have duplicates and may be ordered.)"@en;
  rdfs:domain cdi:ClassificationIndex;
  rdfs:range xsd:boolean;
.

cdi:ClassificationIndex-availableLanguage
  a rdf:Property, owl:DatatypeProperty, ucmis:Attribute;
  rdfs:label "availableLanguage";
  rdfs:comment "A list of languages in which the Statistical Classification is available. If a Classification Index exists in several languages, the number of entries in each language may be different, as the number of terms describing any given phenomenon can change from one language to another. However, the same phenomena should be described in each language. Supports the indication of multiple languages within a single property. Supports use of codes defined by the RFC 1766."@en;
  rdfs:domain cdi:ClassificationIndex;
  rdfs:range xsd:language;
.

cdi:ClassificationIndex-catalogDetails
  a rdf:Property, owl:ObjectProperty, ucmis:Attribute;
  rdfs:label "catalogDetails";
  rdfs:comment "Bundles the information useful for a data catalog entry. \n\nExamples would be creator, contributor, title, copyright, embargo, and license information\n\nA set of information useful for attribution, data discovery, and access.\nThis is information that is tied to the identity of the object. If this information changes the version of the associated object changes."@en;
  rdfs:domain cdi:ClassificationIndex;
  rdfs:range cdi:CatalogDetails;
.

cdi:ClassificationIndex-codingInstruction
  a rdf:Property, owl:ObjectProperty, ucmis:Attribute;
  rdfs:label "codingInstruction";
  rdfs:comment "Additional information which drives the coding process for all entries in a Classification Index."@en;
  rdfs:domain cdi:ClassificationIndex;
  rdfs:range cdi:CommandCode;
.

cdi:ClassificationIndex-corrections
  a rdf:Property, owl:ObjectProperty, ucmis:Attribute;
  rdfs:label "corrections";
  rdfs:comment "Verbal summary description of corrections, which have occurred within the Classification Index. Corrections include changing the item code associated with a classification index entry."@en;
  rdfs:domain cdi:ClassificationIndex;
  rdfs:range cdi:InternationalString;
.

cdi:ClassificationIndex-identifier
  a rdf:Property, owl:ObjectProperty, ucmis:Attribute;
  rdfs:label "identifier";
  rdfs:comment "Identifier for objects requiring short- or long-lasting referencing and management."@en;
  rdfs:domain cdi:ClassificationIndex;
  rdfs:range cdi:Identifier;
.

cdi:ClassificationIndex-name
  a rdf:Property, owl:ObjectProperty, ucmis:Attribute;
  rdfs:label "name";
  rdfs:comment "Human understandable name (liguistic signifier, word, phrase, or mnemonic). May follow ISO/IEC 11179-5 naming principles, and have context provided to specify usage."@en;
  rdfs:domain cdi:ClassificationIndex;
  rdfs:range cdi:ObjectName;
.

cdi:ClassificationIndex-purpose
  a rdf:Property, owl:ObjectProperty, ucmis:Attribute;
  rdfs:label "purpose";
  rdfs:comment "Intent or reason for the object/the description of the object."@en;
  rdfs:domain cdi:ClassificationIndex;
  rdfs:range cdi:InternationalString;
.

cdi:ClassificationIndex-releaseDate
  a rdf:Property, owl:ObjectProperty, ucmis:Attribute;
  rdfs:label "releaseDate";
  rdfs:comment "Date when the current version of the classification index was released."@en;
  rdfs:domain cdi:ClassificationIndex;
  rdfs:range cdi:CombinedDate;
.


cdi:ClassificationIndex_hasContact_Agent
  a rdf:Property, owl:ObjectProperty, ucmis:Association;
  # ASSOCIATION
  rdfs:label "hasContact";
  skos:altLabel "ClassificationIndex_hasContact_Agent";
  rdfs:comment "Person(s) who may be contacted for additional information about the classification index."@en;
  rdfs:domain cdi:ClassificationIndex;
  rdfs:range cdi:Agent;
.

cdi:ClassificationIndex_isMaintainedBy_Agent
  a rdf:Property, owl:ObjectProperty, ucmis:Association;
  # ASSOCIATION
  rdfs:label "isMaintainedBy";
  skos:altLabel "ClassificationIndex_isMaintainedBy_Agent";
  rdfs:comment "The unit or group of persons within the organization responsible for the classification index (i.e., for adding, changing or deleting classification index entries)."@en;
  rdfs:domain cdi:ClassificationIndex;
  rdfs:range cdi:Agent;
.

cdi:ClassificationIndex_isDefinedBy_Concept
  a rdf:Property, owl:ObjectProperty, ucmis:Association;
  # ASSOCIATION
  rdfs:label "isDefinedBy";
  skos:altLabel "ClassificationIndex_isDefinedBy_Concept";
  rdfs:comment "The conceptual basis for the collection of members."@en;
  rdfs:domain cdi:ClassificationIndex;
  rdfs:range cdi:Concept;
.

cdi:ClassificationIndex_has_ClassificationIndexEntry
  a rdf:Property, owl:ObjectProperty, ucmis:Association;
  # ASSOCIATION
  rdfs:label "has";
  skos:altLabel "ClassificationIndex_has_ClassificationIndexEntry";
  
  rdfs:domain cdi:ClassificationIndex;
  rdfs:range cdi:ClassificationIndexEntry;
.

cdi:ClassificationIndex_has_ClassificationIndexEntryPosition
  a rdf:Property, owl:ObjectProperty, ucmis:Association;
  # ASSOCIATION
  rdfs:label "has";
  skos:altLabel "ClassificationIndex_has_ClassificationIndexEntryPosition";
  
  rdfs:domain cdi:ClassificationIndex;
  rdfs:range cdi:ClassificationIndexEntryPosition;
.


# class ClassificationIndexEntry
# based on the UML class DDICDIModels::DDICDILibrary::Classes::Representations::ClassificationIndexEntry
cdi:ClassificationIndexEntry
  a rdfs:Class, owl:Class, ucmis:Class;
  rdfs:label "ClassificationIndexEntry";
  rdfs:comment "Definition\n============\nWord or a short phrase corresponding to a classification item in a statistical classification, together with the code of the corresponding classification item.\n\nExamples\n==========\nThe name of a locality, an economic activity, or an occupational title with the associated code from a corresponding classification item.\n\nExplanatory notes\n===================\nEach Classification Index Entry (CIE) typically corresponds to one item of a Statistical Classification (SC). Although a CIE may be associated with a Classification Item (CI) at any Level of a SC, CIEs are normally associated with items at the lowest Level.\nA CIE corresponds to a CI if the CI classifies the CIE with respect to the SC of which the CI is a member.\nCIEs typically come from responses to survey questions or are verbatim descriptions in administrative records."@en;
  
.

cdi:ClassificationIndexEntry-catalogDetails
  a rdf:Property, owl:ObjectProperty, ucmis:Attribute;
  rdfs:label "catalogDetails";
  rdfs:comment "Bundles the information useful for a data catalog entry. \n\nExamples would be creator, contributor, title, copyright, embargo, and license information\n\nA set of information useful for attribution, data discovery, and access.\nThis is information that is tied to the identity of the object. If this information changes the version of the associated object changes."@en;
  rdfs:domain cdi:ClassificationIndexEntry;
  rdfs:range cdi:CatalogDetails;
.

cdi:ClassificationIndexEntry-codingInstruction
  a rdf:Property, owl:ObjectProperty, ucmis:Attribute;
  rdfs:label "codingInstruction";
  rdfs:comment "Additional information which drives the coding process for the Index Entry. Required when coding is dependent upon one or many other factors."@en;
  rdfs:domain cdi:ClassificationIndexEntry;
  rdfs:range cdi:CommandCode;
.

cdi:ClassificationIndexEntry-entry
  a rdf:Property, owl:ObjectProperty, ucmis:Attribute;
  rdfs:label "entry";
  rdfs:comment "Text describing the type of object/unit or object property."@en;
  rdfs:domain cdi:ClassificationIndexEntry;
  rdfs:range cdi:InternationalString;
.

cdi:ClassificationIndexEntry-identifier
  a rdf:Property, owl:ObjectProperty, ucmis:Attribute;
  rdfs:label "identifier";
  rdfs:comment "Identifier for objects requiring short- or long-lasting referencing and management."@en;
  rdfs:domain cdi:ClassificationIndexEntry;
  rdfs:range cdi:Identifier;
.

cdi:ClassificationIndexEntry-validDates
  a rdf:Property, owl:ObjectProperty, ucmis:Attribute;
  rdfs:label "validDates";
  rdfs:comment "The dates describing the validity period of the object. The date from which the object became valid must be defined if the map belongs to a \"floating\" construct. The date at which the object became invalid must be defined if the map belongs to a \"floating\" construct and is no longer valid."@en;
  rdfs:domain cdi:ClassificationIndexEntry;
  rdfs:range cdi:DateRange;
.



# class ClassificationIndexEntryPosition
# based on the UML class DDICDIModels::DDICDILibrary::Classes::Representations::ClassificationIndexEntryPosition
cdi:ClassificationIndexEntryPosition
  a rdfs:Class, owl:Class, ucmis:Class;
  rdfs:label "ClassificationIndexEntryPosition";
  rdfs:comment "Definition \n============ \nMember indicator for use with member type classification index entry."@en;
  
.

cdi:ClassificationIndexEntryPosition-identifier
  a rdf:Property, owl:ObjectProperty, ucmis:Attribute;
  rdfs:label "identifier";
  rdfs:comment "Identifier for objects requiring short- or long-lasting referencing and management."@en;
  rdfs:domain cdi:ClassificationIndexEntryPosition;
  rdfs:range cdi:Identifier;
.

cdi:ClassificationIndexEntryPosition-value
  a rdf:Property, owl:DatatypeProperty, ucmis:Attribute;
  rdfs:label "value";
  rdfs:comment "Index value of the member in an ordered array."@en;
  rdfs:domain cdi:ClassificationIndexEntryPosition;
  rdfs:range xsd:integer;
.


cdi:ClassificationIndexEntryPosition_indexes_ClassificationIndexEntry
  a rdf:Property, owl:ObjectProperty, ucmis:Association;
  # ASSOCIATION
  rdfs:label "indexes";
  skos:altLabel "ClassificationIndexEntryPosition_indexes_ClassificationIndexEntry";
  rdfs:comment "Restricts member target class to classification index entry."@en;
  rdfs:domain cdi:ClassificationIndexEntryPosition;
  rdfs:range cdi:ClassificationIndexEntry;
.


# class ClassificationItem
# based on the UML class DDICDIModels::DDICDILibrary::Classes::Representations::ClassificationItem
cdi:ClassificationItem
  a rdfs:Class, owl:Class, ucmis:Class;
  rdfs:label "ClassificationItem";
  rdfs:comment "Definition \n============ \nA space for a category within a statistical classification.   \n\nExamples \n========== \nIn the 2012 North American Industry Classification System (NAICS) one classification item has the category \"construction\", and has the Code 23, which designates construction in NAICS.\n\nExplanatory notes \n=================== \nA classification item defines the content and the borders of the category. A unit can be classified to one and only one item at each level of a statistical classification. As such a classification item is a placeholder for a position in a statistical classification. It contains a designation, for which code is a common kind; a category; and possibly other things.   This differentiates it from code which is a only kind of designation, in particular if it is an alphanumeric string assigned to stand in place of a category. Statistical classifications often have multiple levels. A level is defined as a set of classification items each the same number of relationships from the top or root classification item."@en;
  
.

cdi:ClassificationItem-changeFromPreviousVersion
  a rdf:Property, owl:ObjectProperty, ucmis:Attribute;
  rdfs:label "changeFromPreviousVersion";
  rdfs:comment "Describes the changes, which the item has been subject to from the previous version to the actual statistical classification."@en;
  rdfs:domain cdi:ClassificationItem;
  rdfs:range cdi:InternationalString;
.

cdi:ClassificationItem-changeLog
  a rdf:Property, owl:ObjectProperty, ucmis:Attribute;
  rdfs:label "changeLog";
  rdfs:comment "Describes the changes, which the item has been subject to during the life time of the actual statistical classification."@en;
  rdfs:domain cdi:ClassificationItem;
  rdfs:range cdi:InternationalString;
.

cdi:ClassificationItem-explanatoryNotes
  a rdf:Property, owl:ObjectProperty, ucmis:Attribute;
  rdfs:label "explanatoryNotes";
  rdfs:comment "A classification item may be associated with explanatory notes, which further describe and clarify the contents of the category. Explanatory notes consist of: General note: Contains either additional information about the category, or a general description of the category, which is not structured according to the \"includes\", \"includes also\", \"excludes\" pattern. Includes: Specifies the contents of the category. Includes also: A list of borderline cases, which belong to the described category. Excludes: A list of borderline cases, which do not belong to the described category. Excluded cases may contain a reference to the classification items to which the excluded cases belong."@en;
  rdfs:domain cdi:ClassificationItem;
  rdfs:range cdi:InternationalString;
.

cdi:ClassificationItem-futureNotes
  a rdf:Property, owl:ObjectProperty, ucmis:Attribute;
  rdfs:label "futureNotes";
  rdfs:comment "The future events describe an intended or implemented change (or a number of changes) related to an invalid item (e.g., these changes may have turned the now invalid item into one or several successor items). This allows for the possibility of following successors of the item in the future."@en;
  rdfs:domain cdi:ClassificationItem;
  rdfs:range cdi:InternationalString;
.

cdi:ClassificationItem-identifier
  a rdf:Property, owl:ObjectProperty, ucmis:Attribute;
  rdfs:label "identifier";
  rdfs:comment "Identifier for objects requiring short- or long-lasting referencing and management."@en;
  rdfs:domain cdi:ClassificationItem;
  rdfs:range cdi:Identifier;
.

cdi:ClassificationItem-isGenerated
  a rdf:Property, owl:DatatypeProperty, ucmis:Attribute;
  rdfs:label "isGenerated";
  rdfs:comment "Indicates whether or not the item has been generated to make the level to which it belongs complete."@en;
  rdfs:domain cdi:ClassificationItem;
  rdfs:range xsd:boolean;
.

cdi:ClassificationItem-isValid
  a rdf:Property, owl:DatatypeProperty, ucmis:Attribute;
  rdfs:label "isValid";
  rdfs:comment "Indicates whether or not the item is currently valid. If updates are allowed in the Statistical Classification, an item may be restricted in its validity, i.e. it may become valid or invalid after the Statistical Classification has been released."@en;
  rdfs:domain cdi:ClassificationItem;
  rdfs:range xsd:boolean;
.

cdi:ClassificationItem-name
  a rdf:Property, owl:ObjectProperty, ucmis:Attribute;
  rdfs:label "name";
  rdfs:comment "Human understandable name (liguistic signifier, word, phrase, or mnemonic). May follow ISO/IEC 11179-5 naming principles, and have context provided to specify usage. A Classification Item has an official name as provided by the owner or maintenance unit. The name describes the content of the category. The name is unique within the Statistical Classification to which the item belongs, except for categories that are identical at more than one level in a hierarchical classification. Use the context attribute to differentiate official names or alternate names for the Classification Item."@en;
  rdfs:domain cdi:ClassificationItem;
  rdfs:range cdi:ObjectName;
.

cdi:ClassificationItem-validDates
  a rdf:Property, owl:ObjectProperty, ucmis:Attribute;
  rdfs:label "validDates";
  rdfs:comment "The dates describing the validity period of the object. The date from which the object became valid must be defined if the map belongs to a \"floating\" construct. The date at which the object became invalid must be defined if the map belongs to a \"floating\" construct and is no longer valid."@en;
  rdfs:domain cdi:ClassificationItem;
  rdfs:range cdi:DateRange;
.


cdi:ClassificationItem_denotes_Category
  a rdf:Property, owl:ObjectProperty, ucmis:Association;
  # ASSOCIATION
  rdfs:label "denotes";
  skos:altLabel "ClassificationItem_denotes_Category";
  rdfs:comment "A definition for the code. Specialization of denotes for categories."@en;
  rdfs:domain cdi:ClassificationItem;
  rdfs:range cdi:Category;
.

cdi:ClassificationItem_uses_Notation
  a rdf:Property, owl:ObjectProperty, ucmis:Association;
  # ASSOCIATION
  rdfs:label "uses";
  skos:altLabel "ClassificationItem_uses_Notation";
  rdfs:comment "Classification item uses a notation."@en;
  rdfs:domain cdi:ClassificationItem;
  rdfs:range cdi:Notation;
.

cdi:ClassificationItem_excludes_ClassificationItem
  a rdf:Property, owl:ObjectProperty, ucmis:Association;
  # ASSOCIATION
  rdfs:label "excludes";
  skos:altLabel "ClassificationItem_excludes_ClassificationItem";
  rdfs:comment "Classification items to which the excluded cases belong (as described in explanatory notes)."@en;
  rdfs:domain cdi:ClassificationItem;
  rdfs:range cdi:ClassificationItem;
.

cdi:ClassificationItem_hasRulingBy_AuthorizationSource
  a rdf:Property, owl:ObjectProperty, ucmis:Association;
  # ASSOCIATION
  rdfs:label "hasRulingBy";
  skos:altLabel "ClassificationItem_hasRulingBy_AuthorizationSource";
  rdfs:comment "Case law rulings related to the classification item."@en;
  rdfs:domain cdi:ClassificationItem;
  rdfs:range cdi:AuthorizationSource;
.


# class ClassificationItemPosition
# based on the UML class DDICDIModels::DDICDILibrary::Classes::Representations::ClassificationItemPosition
cdi:ClassificationItemPosition
  a rdfs:Class, owl:Class, ucmis:Class;
  rdfs:label "ClassificationItemPosition";
  rdfs:comment "Definition\n============\nProvides a classification item with an index conveying the order of the classification item within a sequence, expressed as an integer, progressing upward from 0 or 1."@en;
  
.

cdi:ClassificationItemPosition-identifier
  a rdf:Property, owl:ObjectProperty, ucmis:Attribute;
  rdfs:label "identifier";
  rdfs:comment "Identifier for objects requiring short- or long-lasting referencing and management."@en;
  rdfs:domain cdi:ClassificationItemPosition;
  rdfs:range cdi:Identifier;
.

cdi:ClassificationItemPosition-value
  a rdf:Property, owl:DatatypeProperty, ucmis:Attribute;
  rdfs:label "value";
  rdfs:comment "Index value of the member in an ordered array."@en;
  rdfs:domain cdi:ClassificationItemPosition;
  rdfs:range xsd:integer;
.


cdi:ClassificationItemPosition_indexes_ClassificationItem
  a rdf:Property, owl:ObjectProperty, ucmis:Association;
  # ASSOCIATION
  rdfs:label "indexes";
  skos:altLabel "ClassificationItemPosition_indexes_ClassificationItem";
  rdfs:comment "Classification item position indexes zero to one classification items. The member containing the designation of the classification item."@en;
  rdfs:domain cdi:ClassificationItemPosition;
  rdfs:range cdi:ClassificationItem;
.


# class ClassificationItemRelationship
# based on the UML class DDICDIModels::DDICDILibrary::Classes::Representations::ClassificationItemRelationship
cdi:ClassificationItemRelationship
  a rdfs:Class, owl:Class, ucmis:Class;
  rdfs:label "ClassificationItemRelationship";
  rdfs:comment "Definition \n============ \nSource-target relationship between classification items in a classification item relation structure."@en;
  
.

cdi:ClassificationItemRelationship-identifier
  a rdf:Property, owl:ObjectProperty, ucmis:Attribute;
  rdfs:label "identifier";
  rdfs:comment "Identifier for objects requiring short- or long-lasting referencing and management."@en;
  rdfs:domain cdi:ClassificationItemRelationship;
  rdfs:range cdi:Identifier;
.

cdi:ClassificationItemRelationship-semantics
  a rdf:Property, owl:ObjectProperty, ucmis:Attribute;
  rdfs:label "semantics";
  rdfs:comment "Specifies the semantics of the object in reference to a vocabulary, ontology, etc."@en;
  rdfs:domain cdi:ClassificationItemRelationship;
  rdfs:range cdi:ControlledVocabularyEntry;
.


cdi:ClassificationItemRelationship_hasSource_ClassificationItem
  a rdf:Property, owl:ObjectProperty, ucmis:Association;
  # ASSOCIATION
  rdfs:label "hasSource";
  skos:altLabel "ClassificationItemRelationship_hasSource_ClassificationItem";
  
  rdfs:domain cdi:ClassificationItemRelationship;
  rdfs:range cdi:ClassificationItem;
.

cdi:ClassificationItemRelationship_hasTarget_ClassificationItem
  a rdf:Property, owl:ObjectProperty, ucmis:Association;
  # ASSOCIATION
  rdfs:label "hasTarget";
  skos:altLabel "ClassificationItemRelationship_hasTarget_ClassificationItem";
  rdfs:comment "Note that this can be realized as a collection to support tuples."@en;
  rdfs:domain cdi:ClassificationItemRelationship;
  rdfs:range cdi:ClassificationItem;
.


# class ClassificationItemStructure
# based on the UML class DDICDIModels::DDICDILibrary::Classes::Representations::ClassificationItemStructure
cdi:ClassificationItemStructure
  a rdfs:Class, owl:Class, ucmis:Class;
  rdfs:label "ClassificationItemStructure";
  rdfs:comment "Definition \n============ \nComplex relation structure for use with statistical classification.  \n\nExamples \n========== \nA classification item structure for the International Standard Classification of Occupations (ISCO-08: https://www.ilo.org/public/english/bureau/stat/isco/isco08/) would describe each of the major classifications as a parent of its sub-classifications. 1 Managers, for example would be listed as a parent of four sub groups: 11 Chief Executives, Senior Officials and Legislators; 12 Chief Executives, Senior Officials and Legislators; 13 Production and Specialized Services Managers; and 14 Hospitality, Retail and Other Services Managers.   \n\nExplanatory notes \n=================== \nThe classification item structure has a set of classification item relationships which are basically adjacency lists. A source classification item has a described relationship to a target list of classification items. The semantic might be, for example, \"parentOf\", or \"contains\", etc."@en;
  
.

cdi:ClassificationItemStructure-displayLabel
  a rdf:Property, owl:ObjectProperty, ucmis:Attribute;
  rdfs:label "displayLabel";
  rdfs:comment "A human-readable display label for the object. Supports the use of multiple languages. Repeat for labels with different content, for example, labels with differing length limitations."@en;
  rdfs:domain cdi:ClassificationItemStructure;
  rdfs:range cdi:LabelForDisplay;
.

cdi:ClassificationItemStructure-identifier
  a rdf:Property, owl:ObjectProperty, ucmis:Attribute;
  rdfs:label "identifier";
  rdfs:comment "Identifier for objects requiring short- or long-lasting referencing and management."@en;
  rdfs:domain cdi:ClassificationItemStructure;
  rdfs:range cdi:Identifier;
.

cdi:ClassificationItemStructure-name
  a rdf:Property, owl:ObjectProperty, ucmis:Attribute;
  rdfs:label "name";
  rdfs:comment "Human understandable name (liguistic signifier, word, phrase, or mnemonic). May follow ISO/IEC 11179-5 naming principles, and have context provided to specify usage."@en;
  rdfs:domain cdi:ClassificationItemStructure;
  rdfs:range cdi:ObjectName;
.

cdi:ClassificationItemStructure-purpose
  a rdf:Property, owl:ObjectProperty, ucmis:Attribute;
  rdfs:label "purpose";
  rdfs:comment "Intent or reason for the object/the description of the object."@en;
  rdfs:domain cdi:ClassificationItemStructure;
  rdfs:range cdi:InternationalString;
.

cdi:ClassificationItemStructure-semantics
  a rdf:Property, owl:ObjectProperty, ucmis:Attribute;
  rdfs:label "semantics";
  rdfs:comment "Specifies the semantics of the object in reference to a vocabulary, ontology, etc."@en;
  rdfs:domain cdi:ClassificationItemStructure;
  rdfs:range cdi:ControlledVocabularyEntry;
.

cdi:ClassificationItemStructure-specification
  a rdf:Property, owl:ObjectProperty, ucmis:Attribute;
  rdfs:label "specification";
  rdfs:comment "Provides information on reflexivity, transitivity, and symmetry of relationship using a descriptive term from an enumerated list. Use if all relations within this relation structure are of the same specification."@en;
  rdfs:domain cdi:ClassificationItemStructure;
  rdfs:range cdi:StructureSpecification;
.

cdi:ClassificationItemStructure-topology
  a rdf:Property, owl:ObjectProperty, ucmis:Attribute;
  rdfs:label "topology";
  rdfs:comment "Indicates the form of the associations among members of the collection. Specifies the way in which constituent parts are interrelated or arranged."@en;
  rdfs:domain cdi:ClassificationItemStructure;
  rdfs:range cdi:ControlledVocabularyEntry;
.

cdi:ClassificationItemStructure-totality
  a rdf:Property, owl:ObjectProperty, ucmis:Attribute;
  rdfs:label "totality";
  rdfs:comment "Indicates whether the related collections are comprehensive in terms of their coverage."@en;
  rdfs:domain cdi:ClassificationItemStructure;
  rdfs:range cdi:StructureExtent;
.


cdi:ClassificationItemStructure_has_ClassificationItemRelationship
  a rdf:Property, owl:ObjectProperty, ucmis:Association;
  # ASSOCIATION
  rdfs:label "has";
  skos:altLabel "ClassificationItemStructure_has_ClassificationItemRelationship";
  
  rdfs:domain cdi:ClassificationItemStructure;
  rdfs:range cdi:ClassificationItemRelationship;
.

cdi:ClassificationItemStructure_structures_StatisticalClassification
  a rdf:Property, owl:ObjectProperty, ucmis:Association;
  # ASSOCIATION
  rdfs:label "structures";
  skos:altLabel "ClassificationItemStructure_structures_StatisticalClassification";
  
  rdfs:domain cdi:ClassificationItemStructure;
  rdfs:range cdi:StatisticalClassification;
.


# class ClassificationPosition
# based on the UML class DDICDIModels::DDICDILibrary::Classes::Representations::ClassificationPosition
cdi:ClassificationPosition
  a rdfs:Class, owl:Class, ucmis:Class;
  rdfs:label "ClassificationPosition";
  rdfs:comment "Definition \n============\nThe index of a classification within a classification family expressed as an integer, progressing upward from 0 or 1."@en;
  
.

cdi:ClassificationPosition-identifier
  a rdf:Property, owl:ObjectProperty, ucmis:Attribute;
  rdfs:label "identifier";
  rdfs:comment "Identifier for objects requiring short- or long-lasting referencing and management."@en;
  rdfs:domain cdi:ClassificationPosition;
  rdfs:range cdi:Identifier;
.

cdi:ClassificationPosition-value
  a rdf:Property, owl:DatatypeProperty, ucmis:Attribute;
  rdfs:label "value";
  rdfs:comment "Index value of the member in an ordered array."@en;
  rdfs:domain cdi:ClassificationPosition;
  rdfs:range xsd:integer;
.


cdi:ClassificationPosition_indexes_StatisticalClassification
  a rdf:Property, owl:ObjectProperty, ucmis:Association;
  # ASSOCIATION
  rdfs:label "indexes";
  skos:altLabel "ClassificationPosition_indexes_StatisticalClassification";
  
  rdfs:domain cdi:ClassificationPosition;
  rdfs:range cdi:StatisticalClassification;
.


# class ClassificationSeries
# based on the UML class DDICDIModels::DDICDILibrary::Classes::Representations::ClassificationSeries
cdi:ClassificationSeries
  a rdfs:Class, owl:Class, ucmis:Class;
  rdfs:label "ClassificationSeries";
  rdfs:comment "Definition\n============\nEnsemble of one or more statistical classifications, based on the same concept, and related to each other as versions or updates.\n\nExamples\n==========\nISIC or ISCO\nSIC (with different published versions related to the publication year).\n\nExplanatory notes\n===================\nTypically, these statistical classifications have the same name."@en;
  
.

cdi:ClassificationSeries-allowsDuplicates
  a rdf:Property, owl:DatatypeProperty, ucmis:Attribute;
  rdfs:label "allowsDuplicates";
  rdfs:comment "If value is False, the members are unique within the collection - if True, there may be duplicates. (Note that a mathematical “bag” permits duplicates and is unordered - a “set” does not have duplicates and may be ordered.)"@en;
  rdfs:domain cdi:ClassificationSeries;
  rdfs:range xsd:boolean;
.

cdi:ClassificationSeries-catalogDetails
  a rdf:Property, owl:ObjectProperty, ucmis:Attribute;
  rdfs:label "catalogDetails";
  rdfs:comment "Bundles the information useful for a data catalog entry. \n\nExamples would be creator, contributor, title, copyright, embargo, and license information\n\nA set of information useful for attribution, data discovery, and access.\nThis is information that is tied to the identity of the object. If this information changes the version of the associated object changes."@en;
  rdfs:domain cdi:ClassificationSeries;
  rdfs:range cdi:CatalogDetails;
.

cdi:ClassificationSeries-context
  a rdf:Property, owl:ObjectProperty, ucmis:Attribute;
  rdfs:label "context";
  rdfs:comment "Classification series can be designed in a specific context of use. This property indicates that context, and supports the use of an external controlled vocabulary for this purpose."@en;
  rdfs:domain cdi:ClassificationSeries;
  rdfs:range cdi:ControlledVocabularyEntry;
.

cdi:ClassificationSeries-identifier
  a rdf:Property, owl:ObjectProperty, ucmis:Attribute;
  rdfs:label "identifier";
  rdfs:comment "Identifier for objects requiring short- or long-lasting referencing and management."@en;
  rdfs:domain cdi:ClassificationSeries;
  rdfs:range cdi:Identifier;
.

cdi:ClassificationSeries-keyword
  a rdf:Property, owl:ObjectProperty, ucmis:Attribute;
  rdfs:label "keyword";
  rdfs:comment "A classification series can be associated with one or a number of keywords."@en;
  rdfs:domain cdi:ClassificationSeries;
  rdfs:range cdi:ControlledVocabularyEntry;
.

cdi:ClassificationSeries-name
  a rdf:Property, owl:ObjectProperty, ucmis:Attribute;
  rdfs:label "name";
  rdfs:comment "Human understandable name (liguistic signifier, word, phrase, or mnemonic). May follow ISO/IEC 11179-5 naming principles, and have context provided to specify usage."@en;
  rdfs:domain cdi:ClassificationSeries;
  rdfs:range cdi:ObjectName;
.

cdi:ClassificationSeries-objectsOrUnitsClassified
  a rdf:Property, owl:ObjectProperty, ucmis:Attribute;
  rdfs:label "objectsOrUnitsClassified";
  rdfs:comment "A classification series is designed to classify a specific type of object/unit according to a specific attribute."@en;
  rdfs:domain cdi:ClassificationSeries;
  rdfs:range cdi:ControlledVocabularyEntry;
.

cdi:ClassificationSeries-purpose
  a rdf:Property, owl:ObjectProperty, ucmis:Attribute;
  rdfs:label "purpose";
  rdfs:comment "Intent or reason for the object/the description of the object."@en;
  rdfs:domain cdi:ClassificationSeries;
  rdfs:range cdi:InternationalString;
.

cdi:ClassificationSeries-subject
  a rdf:Property, owl:ObjectProperty, ucmis:Attribute;
  rdfs:label "subject";
  rdfs:comment "Scientific domains, disciplines, or areas of statistics in which the classification series is implemented."@en;
  rdfs:domain cdi:ClassificationSeries;
  rdfs:range cdi:ControlledVocabularyEntry;
.


cdi:ClassificationSeries_isOwnedBy_Agent
  a rdf:Property, owl:ObjectProperty, ucmis:Association;
  # ASSOCIATION
  rdfs:label "isOwnedBy";
  skos:altLabel "ClassificationSeries_isOwnedBy_Agent";
  rdfs:comment "The statistical office or other authority, which created and maintains the statistical classification(s) related to the classification series. A classification series may have several owners."@en;
  rdfs:domain cdi:ClassificationSeries;
  rdfs:range cdi:Agent;
.

cdi:ClassificationSeries_isDefinedBy_Concept
  a rdf:Property, owl:ObjectProperty, ucmis:Association;
  # ASSOCIATION
  rdfs:label "isDefinedBy";
  skos:altLabel "ClassificationSeries_isDefinedBy_Concept";
  rdfs:comment "The conceptual basis for the collection of members."@en;
  rdfs:domain cdi:ClassificationSeries;
  rdfs:range cdi:Concept;
.

cdi:ClassificationSeries_has_ClassificationPosition
  a rdf:Property, owl:ObjectProperty, ucmis:Association;
  # ASSOCIATION
  rdfs:label "has";
  skos:altLabel "ClassificationSeries_has_ClassificationPosition";
  
  rdfs:domain cdi:ClassificationSeries;
  rdfs:range cdi:ClassificationPosition;
.

cdi:ClassificationSeries_has_StatisticalClassification
  a rdf:Property, owl:ObjectProperty, ucmis:Association;
  # ASSOCIATION
  rdfs:label "has";
  skos:altLabel "ClassificationSeries_has_StatisticalClassification";
  
  rdfs:domain cdi:ClassificationSeries;
  rdfs:range cdi:StatisticalClassification;
.


# class ClassificationSeriesStructure
# based on the UML class DDICDIModels::DDICDILibrary::Classes::Representations::ClassificationSeriesStructure
cdi:ClassificationSeriesStructure
  a rdfs:Class, owl:Class, ucmis:Class;
  rdfs:label "ClassificationSeriesStructure";
  rdfs:comment "Definition\n============\nStructure for describing the complex relationships between statistical classifications in a classification series.\n\nExamples\n==========\nA classification series that branches into separately versioned classifications.\n\nExplanatory notes\n===================\nCan use relation specification information to more fully describe the relationship between members such as parent/child, whole/part, general/specific, equivalence, etc."@en;
  
.

cdi:ClassificationSeriesStructure-identifier
  a rdf:Property, owl:ObjectProperty, ucmis:Attribute;
  rdfs:label "identifier";
  rdfs:comment "Identifier for objects requiring short- or long-lasting referencing and management."@en;
  rdfs:domain cdi:ClassificationSeriesStructure;
  rdfs:range cdi:Identifier;
.

cdi:ClassificationSeriesStructure-name
  a rdf:Property, owl:ObjectProperty, ucmis:Attribute;
  rdfs:label "name";
  rdfs:comment "Human understandable name (liguistic signifier, word, phrase, or mnemonic). May follow ISO/IEC 11179-5 naming principles, and have context provided to specify usage."@en;
  rdfs:domain cdi:ClassificationSeriesStructure;
  rdfs:range cdi:ObjectName;
.

cdi:ClassificationSeriesStructure-purpose
  a rdf:Property, owl:ObjectProperty, ucmis:Attribute;
  rdfs:label "purpose";
  rdfs:comment "Intent or reason for the object/the description of the object."@en;
  rdfs:domain cdi:ClassificationSeriesStructure;
  rdfs:range cdi:InternationalString;
.

cdi:ClassificationSeriesStructure-semantics
  a rdf:Property, owl:ObjectProperty, ucmis:Attribute;
  rdfs:label "semantics";
  rdfs:comment "Specifies the semantics of the object in reference to a vocabulary, ontology, etc."@en;
  rdfs:domain cdi:ClassificationSeriesStructure;
  rdfs:range cdi:ControlledVocabularyEntry;
.

cdi:ClassificationSeriesStructure-specification
  a rdf:Property, owl:ObjectProperty, ucmis:Attribute;
  rdfs:label "specification";
  rdfs:comment "Provides information on reflexivity, transitivity, and symmetry of relationship using a descriptive term from an enumerated list. Use if all relations within this relation structure are of the same specification."@en;
  rdfs:domain cdi:ClassificationSeriesStructure;
  rdfs:range cdi:StructureSpecification;
.

cdi:ClassificationSeriesStructure-topology
  a rdf:Property, owl:ObjectProperty, ucmis:Attribute;
  rdfs:label "topology";
  rdfs:comment "Indicates the form of the associations among members of the collection. Specifies the way in which constituent parts are interrelated or arranged."@en;
  rdfs:domain cdi:ClassificationSeriesStructure;
  rdfs:range cdi:ControlledVocabularyEntry;
.

cdi:ClassificationSeriesStructure-totality
  a rdf:Property, owl:ObjectProperty, ucmis:Attribute;
  rdfs:label "totality";
  rdfs:comment "Indicates whether the related collections are comprehensive in terms of their coverage."@en;
  rdfs:domain cdi:ClassificationSeriesStructure;
  rdfs:range cdi:StructureExtent;
.


cdi:ClassificationSeriesStructure_has_StatisticalClassificationRelationship
  a rdf:Property, owl:ObjectProperty, ucmis:Association;
  # ASSOCIATION
  rdfs:label "has";
  skos:altLabel "ClassificationSeriesStructure_has_StatisticalClassificationRelationship";
  
  rdfs:domain cdi:ClassificationSeriesStructure;
  rdfs:range cdi:StatisticalClassificationRelationship;
.

cdi:ClassificationSeriesStructure_structures_ClassificationSeries
  a rdf:Property, owl:ObjectProperty, ucmis:Association;
  # ASSOCIATION
  rdfs:label "structures";
  skos:altLabel "ClassificationSeriesStructure_structures_ClassificationSeries";
  
  rdfs:domain cdi:ClassificationSeriesStructure;
  rdfs:range cdi:ClassificationSeries;
.


# class Code
# based on the UML class DDICDIModels::DDICDILibrary::Classes::Representations::Code
cdi:Code
  a rdfs:Class, owl:Class, ucmis:Class;
  rdfs:label "Code";
  rdfs:comment "Definition \n============ \nThe characters used as a symbol to designate a category within a codelist or classification. (Formally, a sign for which the signifier is non-linguistic alphanumeric string.)   \n\nExamples \n========== \nThe letter M might stand for the category \"Male\" in the codeList called \"Gender\".  \n\nExplanatory notes \n=================== \nA non-linguistic alphanumeric string is one which does not correspond to a word in natural language. For use in a codelist. The representation property (value) is expressed as it would be found in a data file. Multiple representations may relate to the same category but should be expressed as separate codes.  It should not be confused with a classification item which is a placeholder for a position in a statistical classification."@en;
  
.

cdi:Code-identifier
  a rdf:Property, owl:ObjectProperty, ucmis:Attribute;
  rdfs:label "identifier";
  rdfs:comment "Identifier for objects requiring short- or long-lasting referencing and management."@en;
  rdfs:domain cdi:Code;
  rdfs:range cdi:Identifier;
.


cdi:Code_denotes_Category
  a rdf:Property, owl:ObjectProperty, ucmis:Association;
  # ASSOCIATION
  rdfs:label "denotes";
  skos:altLabel "Code_denotes_Category";
  rdfs:comment "A definition for the code. Specialization of denotes for categories."@en;
  rdfs:domain cdi:Code;
  rdfs:range cdi:Category;
.

cdi:Code_uses_Notation
  a rdf:Property, owl:ObjectProperty, ucmis:Association;
  # ASSOCIATION
  rdfs:label "uses";
  skos:altLabel "Code_uses_Notation";
  
  rdfs:domain cdi:Code;
  rdfs:range cdi:Notation;
.


# class CodeList
# based on the UML class DDICDIModels::DDICDILibrary::Classes::Representations::CodeList
cdi:CodeList
  a rdfs:Class, owl:Class, ucmis:Class;
  rdfs:label "CodeList";
  rdfs:comment "Definition \n============ \nList of codes and associated categories.  \n\nExamples \n========== \nThe codes \"M\" and \"F\" could point to \"Male\" and \"Female\" categories respectively.  A code list for an occupational classification system like the International Standard Classification of Occupations (ISCO-08: https://www.ilo.org/public/english/bureau/stat/isco/isco08/) could use a classification relation structure to describe a hierarchy (Chief Executives and Administrative and Commercial Managers as subtypes of Managers).   \n\nExplanatory notes \n=================== \nList may be flat or hierarchical. A hierarchical structure may have an indexed order for intended presentation even though the content within levels of the hierarchy are conceptually unordered. For hierarchical structures classification item structure is used to provide additional information on the structure and organization of the categories. Note that a category set can be structured by a classification relation structure without the need for associating any codes with the categories. This allows for the creation of a category set, for example for a response domain, without an associated codelist."@en;
  rdfs:subClassOf cdi:EnumerationDomain;
.

cdi:CodeList-allowsDuplicates
  a rdf:Property, owl:DatatypeProperty, ucmis:Attribute;
  rdfs:label "allowsDuplicates";
  rdfs:comment "If value is False, the members are unique within the collection - if True, there may be duplicates. (Note that a mathematical “bag” permits duplicates and is unordered - a “set” does not have duplicates and may be ordered.)"@en;
  rdfs:domain cdi:CodeList;
  rdfs:range xsd:boolean;
.


cdi:CodeList_has_Code
  a rdf:Property, owl:ObjectProperty, ucmis:Association;
  # ASSOCIATION
  rdfs:label "has";
  skos:altLabel "CodeList_has_Code";
  
  rdfs:domain cdi:CodeList;
  rdfs:range cdi:Code;
.

cdi:CodeList_has_CodePosition
  a rdf:Property, owl:ObjectProperty, ucmis:Association;
  # ASSOCIATION
  rdfs:label "has";
  skos:altLabel "CodeList_has_CodePosition";
  
  rdfs:domain cdi:CodeList;
  rdfs:range cdi:CodePosition;
.


# class CodeListStructure
# based on the UML class DDICDIModels::DDICDILibrary::Classes::Representations::CodeListStructure
cdi:CodeListStructure
  a rdfs:Class, owl:Class, ucmis:Class;
  rdfs:label "CodeListStructure";
  rdfs:comment "Definition\n============\nRelation structure of codes within a codelist.\n\nExplanatory notes\n===================\nAllows for the specification of complex relationships among codes. The code list structure employs a set of code relationips to describe the relationship among concepts. Each code relationship is a one to many description of connections between codes. Together they might commonly describe relationships as complex as a hierarchy."@en;
  
.

cdi:CodeListStructure-identifier
  a rdf:Property, owl:ObjectProperty, ucmis:Attribute;
  rdfs:label "identifier";
  rdfs:comment "Identifier for objects requiring short- or long-lasting referencing and management."@en;
  rdfs:domain cdi:CodeListStructure;
  rdfs:range cdi:Identifier;
.

cdi:CodeListStructure-name
  a rdf:Property, owl:ObjectProperty, ucmis:Attribute;
  rdfs:label "name";
  rdfs:comment "Human understandable name (liguistic signifier, word, phrase, or mnemonic). May follow ISO/IEC 11179-5 naming principles, and have context provided to specify usage."@en;
  rdfs:domain cdi:CodeListStructure;
  rdfs:range cdi:ObjectName;
.

cdi:CodeListStructure-purpose
  a rdf:Property, owl:ObjectProperty, ucmis:Attribute;
  rdfs:label "purpose";
  rdfs:comment "Intent or reason for the object/the description of the object."@en;
  rdfs:domain cdi:CodeListStructure;
  rdfs:range cdi:InternationalString;
.

cdi:CodeListStructure-semantics
  a rdf:Property, owl:ObjectProperty, ucmis:Attribute;
  rdfs:label "semantics";
  rdfs:comment "Specifies the semantics of the object in reference to a vocabulary, ontology, etc."@en;
  rdfs:domain cdi:CodeListStructure;
  rdfs:range cdi:ControlledVocabularyEntry;
.

cdi:CodeListStructure-specification
  a rdf:Property, owl:ObjectProperty, ucmis:Attribute;
  rdfs:label "specification";
  rdfs:comment "Provides information on reflexivity, transitivity, and symmetry of relationship using a descriptive term from an enumerated list. Use if all relations within this relation structure are of the same specification."@en;
  rdfs:domain cdi:CodeListStructure;
  rdfs:range cdi:StructureSpecification;
.

cdi:CodeListStructure-topology
  a rdf:Property, owl:ObjectProperty, ucmis:Attribute;
  rdfs:label "topology";
  rdfs:comment "Indicates the form of the associations among members of the collection. Specifies the way in which constituent parts are interrelated or arranged."@en;
  rdfs:domain cdi:CodeListStructure;
  rdfs:range cdi:ControlledVocabularyEntry;
.

cdi:CodeListStructure-totality
  a rdf:Property, owl:ObjectProperty, ucmis:Attribute;
  rdfs:label "totality";
  rdfs:comment "Indicates whether the related collections are comprehensive in terms of their coverage."@en;
  rdfs:domain cdi:CodeListStructure;
  rdfs:range cdi:StructureExtent;
.


cdi:CodeListStructure_has_CodeRelationship
  a rdf:Property, owl:ObjectProperty, ucmis:Association;
  # ASSOCIATION
  rdfs:label "has";
  skos:altLabel "CodeListStructure_has_CodeRelationship";
  
  rdfs:domain cdi:CodeListStructure;
  rdfs:range cdi:CodeRelationship;
.

cdi:CodeListStructure_structures_CodeList
  a rdf:Property, owl:ObjectProperty, ucmis:Association;
  # ASSOCIATION
  rdfs:label "structures";
  skos:altLabel "CodeListStructure_structures_CodeList";
  
  rdfs:domain cdi:CodeListStructure;
  rdfs:range cdi:CodeList;
.


# class CodePosition
# based on the UML class DDICDIModels::DDICDILibrary::Classes::Representations::CodePosition
cdi:CodePosition
  a rdfs:Class, owl:Class, ucmis:Class;
  rdfs:label "CodePosition";
  rdfs:comment "Definition \n============ \nAn index within an order intended for presentation (even though the content within levels of the hierarchy may be conceptually unordered). Expressed as an integer counting upward from 01 or 1."@en;
  
.

cdi:CodePosition-identifier
  a rdf:Property, owl:ObjectProperty, ucmis:Attribute;
  rdfs:label "identifier";
  rdfs:comment "Identifier for objects requiring short- or long-lasting referencing and management."@en;
  rdfs:domain cdi:CodePosition;
  rdfs:range cdi:Identifier;
.

cdi:CodePosition-value
  a rdf:Property, owl:DatatypeProperty, ucmis:Attribute;
  rdfs:label "value";
  rdfs:comment "Index value of the member in an ordered array."@en;
  rdfs:domain cdi:CodePosition;
  rdfs:range xsd:integer;
.


cdi:CodePosition_indexes_Code
  a rdf:Property, owl:ObjectProperty, ucmis:Association;
  # ASSOCIATION
  rdfs:label "indexes";
  skos:altLabel "CodePosition_indexes_Code";
  
  rdfs:domain cdi:CodePosition;
  rdfs:range cdi:Code;
.


# class CodeRelationship
# based on the UML class DDICDIModels::DDICDILibrary::Classes::Representations::CodeRelationship
cdi:CodeRelationship
  a rdfs:Class, owl:Class, ucmis:Class;
  rdfs:label "CodeRelationship";
  rdfs:comment "Definition\n============\nSource target relationship between codes in a code relation structure."@en;
  
.

cdi:CodeRelationship-identifier
  a rdf:Property, owl:ObjectProperty, ucmis:Attribute;
  rdfs:label "identifier";
  rdfs:comment "Identifier for objects requiring short- or long-lasting referencing and management."@en;
  rdfs:domain cdi:CodeRelationship;
  rdfs:range cdi:Identifier;
.

cdi:CodeRelationship-semantics
  a rdf:Property, owl:ObjectProperty, ucmis:Attribute;
  rdfs:label "semantics";
  rdfs:comment "Specifies the semantics of the object in reference to a vocabulary, ontology, etc."@en;
  rdfs:domain cdi:CodeRelationship;
  rdfs:range cdi:ControlledVocabularyEntry;
.


cdi:CodeRelationship_hasSource_Code
  a rdf:Property, owl:ObjectProperty, ucmis:Association;
  # ASSOCIATION
  rdfs:label "hasSource";
  skos:altLabel "CodeRelationship_hasSource_Code";
  
  rdfs:domain cdi:CodeRelationship;
  rdfs:range cdi:Code;
.

cdi:CodeRelationship_hasTarget_Code
  a rdf:Property, owl:ObjectProperty, ucmis:Association;
  # ASSOCIATION
  rdfs:label "hasTarget";
  skos:altLabel "CodeRelationship_hasTarget_Code";
  rdfs:comment "Note that this can be realized as a collection to support tuples."@en;
  rdfs:domain cdi:CodeRelationship;
  rdfs:range cdi:Code;
.


# class CorrespondenceTable
# based on the UML class DDICDIModels::DDICDILibrary::Classes::Representations::CorrespondenceTable
cdi:CorrespondenceTable
  a rdfs:Class, owl:Class, ucmis:Class;
  rdfs:label "CorrespondenceTable";
  rdfs:comment "Definition \n============ \nSet of relationships between the members within or between statistical classifications.  \n\nExamples \n========== \nCorrespondence between the U.S. Standard Industrial Classification (SIC) and North American Industrial Classification System (NAICS).  \n\nExplanatory notes \n=================== \nCorrespondence tables are used with statistical classifications. For instance, it can relate two versions from the same classification series; statistical classifications from different classification series; a variant and the version on which it is based; or different versions of a variant. In the first and last examples, the correspondence table facilitates comparability over time."@en;
  
.

cdi:CorrespondenceTable-catalogDetails
  a rdf:Property, owl:ObjectProperty, ucmis:Attribute;
  rdfs:label "catalogDetails";
  rdfs:comment "Bundles the information useful for a data catalog entry. \n\nExamples would be creator, contributor, title, copyright, embargo, and license information\n\nA set of information useful for attribution, data discovery, and access.\nThis is information that is tied to the identity of the object. If this information changes the version of the associated object changes."@en;
  rdfs:domain cdi:CorrespondenceTable;
  rdfs:range cdi:CatalogDetails;
.

cdi:CorrespondenceTable-effectiveDates
  a rdf:Property, owl:ObjectProperty, ucmis:Attribute;
  rdfs:label "effectiveDates";
  rdfs:comment "Effective period of validity of the correspondence table. The correspondence table expresses the relationships between the two classifications as they existed on the period specified in the table."@en;
  rdfs:domain cdi:CorrespondenceTable;
  rdfs:range cdi:DateRange;
.

cdi:CorrespondenceTable-identifier
  a rdf:Property, owl:ObjectProperty, ucmis:Attribute;
  rdfs:label "identifier";
  rdfs:comment "Identifier for objects requiring short- or long-lasting referencing and management."@en;
  rdfs:domain cdi:CorrespondenceTable;
  rdfs:range cdi:Identifier;
.


cdi:CorrespondenceTable_hasContact_Agent
  a rdf:Property, owl:ObjectProperty, ucmis:Association;
  # ASSOCIATION
  rdfs:label "hasContact";
  skos:altLabel "CorrespondenceTable_hasContact_Agent";
  rdfs:comment "The person(s) who may be contacted for additional information about the correspondence table. Can be an individual or organization."@en;
  rdfs:domain cdi:CorrespondenceTable;
  rdfs:range cdi:Agent;
.

cdi:CorrespondenceTable_isMaintainedBy_Agent
  a rdf:Property, owl:ObjectProperty, ucmis:Association;
  # ASSOCIATION
  rdfs:label "isMaintainedBy";
  skos:altLabel "CorrespondenceTable_isMaintainedBy_Agent";
  rdfs:comment "The unit or group of persons who are responsible for the correspondence table (i.e., for maintaining and updating it)."@en;
  rdfs:domain cdi:CorrespondenceTable;
  rdfs:range cdi:Agent;
.

cdi:CorrespondenceTable_isOwnedBy_Agent
  a rdf:Property, owl:ObjectProperty, ucmis:Association;
  # ASSOCIATION
  rdfs:label "isOwnedBy";
  skos:altLabel "CorrespondenceTable_isOwnedBy_Agent";
  rdfs:comment "The statistical office, other authority or section that created and maintains the correspondence table. A correspondence table may have several owners."@en;
  rdfs:domain cdi:CorrespondenceTable;
  rdfs:range cdi:Agent;
.

cdi:CorrespondenceTable_has_ConceptMap
  a rdf:Property, owl:ObjectProperty, ucmis:Association;
  # ASSOCIATION
  rdfs:label "has";
  skos:altLabel "CorrespondenceTable_has_ConceptMap";
  rdfs:comment "Correspondence table has zero to many concept maps."@en;
  rdfs:domain cdi:CorrespondenceTable;
  rdfs:range cdi:ConceptMap;
.

cdi:CorrespondenceTable_hasSource_Level
  a rdf:Property, owl:ObjectProperty, ucmis:Association;
  # ASSOCIATION
  rdfs:label "hasSource";
  skos:altLabel "CorrespondenceTable_hasSource_Level";
  rdfs:comment "Level from which the correspondence is made. Correspondences might be restricted to a specified level in the node set. In this case, target items are assigned only to source items on the given level. If no level is indicated, source items can be assigned to any level of the target node set."@en;
  rdfs:domain cdi:CorrespondenceTable;
  rdfs:range cdi:Level;
.

cdi:CorrespondenceTable_hasTarget_Level
  a rdf:Property, owl:ObjectProperty, ucmis:Association;
  # ASSOCIATION
  rdfs:label "hasTarget";
  skos:altLabel "CorrespondenceTable_hasTarget_Level";
  rdfs:comment "Level to which the correspondence is made. Correspondences might be restricted to a specified Level in the node set. In this case, target items are assigned only to source items on the given level. If no level is indicated, target items can be assigned to any level of the source node set."@en;
  rdfs:domain cdi:CorrespondenceTable;
  rdfs:range cdi:Level;
.

cdi:CorrespondenceTable_mapsTo_StatisticalClassification
  a rdf:Property, owl:ObjectProperty, ucmis:Association;
  # ASSOCIATION
  rdfs:label "mapsTo";
  skos:altLabel "CorrespondenceTable_mapsTo_StatisticalClassification";
  rdfs:comment "The statistical classification(s) from which the correspondence is made."@en;
  rdfs:domain cdi:CorrespondenceTable;
  rdfs:range cdi:StatisticalClassification;
.


# class EnumerationDomain
# based on the UML class DDICDIModels::DDICDILibrary::Classes::Representations::EnumerationDomain
cdi:EnumerationDomain
  a rdfs:Class, owl:Class, ucmis:Class;
  rdfs:label "EnumerationDomain";
  rdfs:comment "Definition \n============ \nA base class acting as an extension point to allow all codifications (codelist, statistical classification, etc.) to be understood as enumerated value domains."@en;
  
.

cdi:EnumerationDomain-identifier
  a rdf:Property, owl:ObjectProperty, ucmis:Attribute;
  rdfs:label "identifier";
  rdfs:comment "Identifier for objects requiring short- or long-lasting referencing and management."@en;
  rdfs:domain cdi:EnumerationDomain;
  rdfs:range cdi:Identifier;
.

cdi:EnumerationDomain-name
  a rdf:Property, owl:ObjectProperty, ucmis:Attribute;
  rdfs:label "name";
  rdfs:comment "Human understandable name (liguistic signifier, word, phrase, or mnemonic). May follow ISO/IEC 11179-5 naming principles, and have context provided to specify usage."@en;
  rdfs:domain cdi:EnumerationDomain;
  rdfs:range cdi:ObjectName;
.

cdi:EnumerationDomain-purpose
  a rdf:Property, owl:ObjectProperty, ucmis:Attribute;
  rdfs:label "purpose";
  rdfs:comment "Intent or reason for the object/the description of the object."@en;
  rdfs:domain cdi:EnumerationDomain;
  rdfs:range cdi:InternationalString;
.


cdi:EnumerationDomain_isDefinedBy_Concept
  a rdf:Property, owl:ObjectProperty, ucmis:Association;
  # ASSOCIATION
  rdfs:label "isDefinedBy";
  skos:altLabel "EnumerationDomain_isDefinedBy_Concept";
  rdfs:comment "The conceptual basis for the collection of members."@en;
  rdfs:domain cdi:EnumerationDomain;
  rdfs:range cdi:Concept;
.

cdi:EnumerationDomain_references_CategorySet
  a rdf:Property, owl:ObjectProperty, ucmis:Association;
  # ASSOCIATION
  rdfs:label "references";
  skos:altLabel "EnumerationDomain_references_CategorySet";
  rdfs:comment "Category set associated with the enumeration."@en;
  rdfs:domain cdi:EnumerationDomain;
  rdfs:range cdi:CategorySet;
.

cdi:EnumerationDomain_uses_LevelStructure
  a rdf:Property, owl:ObjectProperty, ucmis:Association;
  # ASSOCIATION
  rdfs:label "uses";
  skos:altLabel "EnumerationDomain_uses_LevelStructure";
  rdfs:comment "Has meaningful level to which members belong."@en;
  rdfs:domain cdi:EnumerationDomain;
  rdfs:range cdi:LevelStructure;
.


# class Level
# based on the UML class DDICDIModels::DDICDILibrary::Classes::Representations::Level
cdi:Level
  a rdfs:Class, owl:Class, ucmis:Class;
  rdfs:label "Level";
  rdfs:comment "Definition\n============\nSet of all classification items the same number of relationships from the root (or top) classification item.\n\nExamples\n==========\nISCO-08: index='1' label of associated category 'Major', index='2' label of associated category 'Sub-Major',  index='3' label of associated category 'Minor', \n\nExplanatory notes\n===================\nProvides level information for the members of the level structure. levelNumber provides the level number which may or may not be associated with a category which defines level."@en;
  
.

cdi:Level-displayLabel
  a rdf:Property, owl:ObjectProperty, ucmis:Attribute;
  rdfs:label "displayLabel";
  rdfs:comment "A human-readable display label for the object. Supports the use of multiple languages. Repeat for labels with different content, for example, labels with differing length limitations."@en;
  rdfs:domain cdi:Level;
  rdfs:range cdi:LabelForDisplay;
.

cdi:Level-identifier
  a rdf:Property, owl:ObjectProperty, ucmis:Attribute;
  rdfs:label "identifier";
  rdfs:comment "Identifier for objects requiring short- or long-lasting referencing and management."@en;
  rdfs:domain cdi:Level;
  rdfs:range cdi:Identifier;
.

cdi:Level-levelNumber
  a rdf:Property, owl:DatatypeProperty, ucmis:Attribute;
  rdfs:label "levelNumber";
  rdfs:comment "Provides an association between a level number and optional concept which defines it within an ordered array. Use is required."@en;
  rdfs:domain cdi:Level;
  rdfs:range xsd:integer;
.


cdi:Level_isDefinedBy_Concept
  a rdf:Property, owl:ObjectProperty, ucmis:Association;
  # ASSOCIATION
  rdfs:label "isDefinedBy";
  skos:altLabel "Level_isDefinedBy_Concept";
  rdfs:comment "A concept or concept sub-type which describes the level."@en;
  rdfs:domain cdi:Level;
  rdfs:range cdi:Concept;
.

cdi:Level_groups_ClassificationItem
  a rdf:Property, owl:ObjectProperty, ucmis:Association;
  # ASSOCIATION
  rdfs:label "groups";
  skos:altLabel "Level_groups_ClassificationItem";
  
  rdfs:domain cdi:Level;
  rdfs:range cdi:ClassificationItem;
.


# class LevelStructure
# based on the UML class DDICDIModels::DDICDILibrary::Classes::Representations::LevelStructure
cdi:LevelStructure
  a rdfs:Class, owl:Class, ucmis:Class;
  rdfs:label "LevelStructure";
  rdfs:comment "Definition \n============ \nNesting structure of a hierarchical collection.   \n\nExamples \n========== \nThe International Standard Classification of Occupations (ISCO-08: https://www.ilo.org/public/english/bureau/stat/isco/isco08/) Major, Sub-Major, and Minor or the North American Industry Classification System (NAICS: https://www.census.gov/naics/) 2 digit sector codes, 3 digit subsector code list, 4 digit industry group code list, and 5 digit industry code list.\n\nExplanatory notes \n=================== \nThe levels within the structure begin at the root level '1' and continue as an ordered array through each level of nesting. Levels are used to organize a hierarchy. Usually, a hierarchy contains one root member at the top, though it could contain several. These are the first level. All members directly related to those  in the first level compose the second level. The third and subsequent levels are defined similarly.  A level often is associated with a concept, which defines it. These correspond to kinds of aggregates. For example, in the US Standard Occupational Classification (2010), the level below the top is called Major Occupation Groups, and the next level is called Minor Occupational Groups. These ideas convey the structure. In particular, Health Care Practitioners (a major group) can be broken into Chiropractors, Dentists, Physicians, Vets, Therapists, etc. (minor groups) The categories in the nodes at the lower level aggregate to the category in node above them.  \"Classification schemes are frequently organized in nested levels of increasing detail. ISCO-08, for example, has four levels: at the top level are ten major groups, each of which contain sub-major groups, which in turn are subdivided in minor groups, which contain unit groups. Even when a classification is not structured in levels (\"flat classification\"), the usual convention, which is adopted here, is to consider that it contains one unique level.\" (From the W3C Simple Knowlegde Organization System: http://rdf-vocabulary.ddialliance.org/xkos.html#) Individual classification items organized in a hierarchy may be associated with a specific level."@en;
  
.

cdi:LevelStructure-catalogDetails
  a rdf:Property, owl:ObjectProperty, ucmis:Attribute;
  rdfs:label "catalogDetails";
  rdfs:comment "Bundles the information useful for a data catalog entry. \n\nExamples would be creator, contributor, title, copyright, embargo, and license information\n\nA set of information useful for attribution, data discovery, and access.\nThis is information that is tied to the identity of the object. If this information changes the version of the associated object changes."@en;
  rdfs:domain cdi:LevelStructure;
  rdfs:range cdi:CatalogDetails;
.

cdi:LevelStructure-identifier
  a rdf:Property, owl:ObjectProperty, ucmis:Attribute;
  rdfs:label "identifier";
  rdfs:comment "Identifier for objects requiring short- or long-lasting referencing and management."@en;
  rdfs:domain cdi:LevelStructure;
  rdfs:range cdi:Identifier;
.

cdi:LevelStructure-name
  a rdf:Property, owl:ObjectProperty, ucmis:Attribute;
  rdfs:label "name";
  rdfs:comment "Human understandable name (liguistic signifier, word, phrase, or mnemonic). May follow ISO/IEC 11179-5 naming principles, and have context provided to specify usage."@en;
  rdfs:domain cdi:LevelStructure;
  rdfs:range cdi:ObjectName;
.

cdi:LevelStructure-usage
  a rdf:Property, owl:ObjectProperty, ucmis:Attribute;
  rdfs:label "usage";
  rdfs:comment "Explanation of the ways in which the object is employed."@en;
  rdfs:domain cdi:LevelStructure;
  rdfs:range cdi:InternationalString;
.

cdi:LevelStructure-validDateRange
  a rdf:Property, owl:ObjectProperty, ucmis:Attribute;
  rdfs:label "validDateRange";
  rdfs:comment "The period for which the level object is valid, expressed as a start and end date (supports both ISO-standard and non-ISO date formats)."@en;
  rdfs:domain cdi:LevelStructure;
  rdfs:range cdi:DateRange;
.


cdi:LevelStructure_has_Level
  a rdf:Property, owl:ObjectProperty, ucmis:Association;
  # ASSOCIATION
  rdfs:label "has";
  skos:altLabel "LevelStructure_has_Level";
  
  rdfs:domain cdi:LevelStructure;
  rdfs:range cdi:Level;
.


# class SentinelValueDomain
# based on the UML class DDICDIModels::DDICDILibrary::Classes::Representations::SentinelValueDomain
cdi:SentinelValueDomain
  a rdfs:Class, owl:Class, ucmis:Class;
  rdfs:label "SentinelValueDomain";
  rdfs:comment "Definition \n============ \nValue domain for a sentinel conceptual domain.   \n\nExamples \n========== \nMissing categories expressed as codes: -9, refused; -8, Don't Know; for a numeric variable with values greater than zero.    \n\nExplanatory notes \n=================== \nSentinel values are defined in ISO 11404 as \"element of a value space that is not completely consistent with a datatype's properties and characterizing operations...\". A common example would be codes for missing values. Sentinel values are used for processing, not to describe subject matter. Typical examples include missing values or invalid entry codes. Sentinel value domains are typically of the enumerated type, but they can be the described type, too. This is not to say that sentinel values carry no information. Data on gender might be enumerated by \"0, male\" and \"1, female\". These are the substantive values (see substantive value domain). However, there may be the need to include missing values along with that data, such as \"m, missing\" and \"r, refused\". These are sentinel values.  ISO/IEC 11404 - General Purpose Datatypes, defines sentinel values in terms of how that standard defines datatypes. But, the fact that the sentinels don't fit in terms of the calculations and statistics one would perform on the \"clean\" data is a distinguishing characteristic. In the example above, one would not include missing or refused data in calculating a ratio of females to the total population. Sentinel values may be described rather than enumerated. For instance, there might be a range of values, each representing an out of range value, but there could be too many to enumerate. It is easier to describe the range.  In some software missing values are represented as values not in the datatype of the valid values. R has values of NA, NaN, Inf, and -Inf. SAS and Stata have values displayed as \".\", \".A\" through \".Z\", and \"._\"  Other software might use values like 999 for missing that would otherwise be the same datatype as valid values but outside the parameters of the domain. In the gender example above: For SPSS the sentinel values might be represented as: 998 = \"refused\" 999 = \"not recorded\"  For SAS or Stata the sentinel values might be represented as: .R = \"refused\" .N = \"not recorded\"  Sentinel values can also be used for other purposes beyond missing. For a numeric variable \"A\" might represent a value somewhere in a defined range to prevent disclosure of information about an individual. This might be considered a \"semi-missing value\". In SAS or Stata for example: .A = \"greater than or equal to 100 and less than 1000 \"."@en;
  rdfs:subClassOf cdi:ValueDomain;
.

cdi:SentinelValueDomain-platformType
  a rdf:Property, owl:ObjectProperty, ucmis:Attribute;
  rdfs:label "platformType";
  rdfs:comment "The type of platform under which sentinel codes will be used. Statistical software platforms use different sets of codes to indicate missing values. The external controlled vocabulary should list platform types and a description of the allowed missing value types. A sample list would be: \n\n- BlankString - A Blank string indicates missing. Comparison is based on lexical order.  \n- EmptyString - An empty string indicates missing. Use in comparisons returns missing.   \n- Rstyle - Codes drawn from  NA and the IEEE 754 values of NaN  -Inf   +Inf.   Comparisons return NA.   \n- SASNumeric - codes drawn from . ._ .A .B .C .D .E .F .G .H .I .J .K .L .M .N .O .P .Q .R .S .T .U .V .W .X .Y .Z    Sentinel code treated as less than any substantive value   \n- SPSSstyle - System missing (a dot) a set of individual values drawn from the same datatype as the SubstantiveValueDomain, and a range of values  drawn from the same datatype as the SubstantiveValueDomain. Comparisons return system missing. Some functions substitute with valid values (e.g. SUM replaces missing values with 0).  \n- StataNumeric - codes drawn from . ._ .A .B .C .D .E .F .G .H .I .J .K .L .M .N .O .P .Q .R .S .T .U .V .W .X .Y .Z  Sentinel code treated as greater than any substantive value  - Unrestricted - No restrictions on codes for sentinel values. Use in comparisons is indeterminate."@en;
  rdfs:domain cdi:SentinelValueDomain;
  rdfs:range cdi:ControlledVocabularyEntry;
.


cdi:SentinelValueDomain_takesConceptsFrom_SentinelConceptualDomain
  a rdf:Property, owl:ObjectProperty, ucmis:Association;
  # ASSOCIATION
  rdfs:label "takesConceptsFrom";
  skos:altLabel "SentinelValueDomain_takesConceptsFrom_SentinelConceptualDomain";
  rdfs:comment "Corresponding conceptual definition given by a sentinel conceptual domain."@en;
  rdfs:domain cdi:SentinelValueDomain;
  rdfs:range cdi:SentinelConceptualDomain;
.

cdi:SentinelValueDomain_isDescribedBy_ValueAndConceptDescription
  a rdf:Property, owl:ObjectProperty, ucmis:Association;
  # ASSOCIATION
  rdfs:label "isDescribedBy";
  skos:altLabel "SentinelValueDomain_isDescribedBy_ValueAndConceptDescription";
  rdfs:comment "A formal description of the set of valid values - for described value domains."@en;
  rdfs:domain cdi:SentinelValueDomain;
  rdfs:range cdi:ValueAndConceptDescription;
.

cdi:SentinelValueDomain_takesValuesFrom_EnumerationDomain
  a rdf:Property, owl:ObjectProperty, ucmis:Association;
  # ASSOCIATION
  rdfs:label "takesValuesFrom";
  skos:altLabel "SentinelValueDomain_takesValuesFrom_EnumerationDomain";
  rdfs:comment "Any subtype of an enumeration domain enumerating the set of valid values."@en;
  rdfs:domain cdi:SentinelValueDomain;
  rdfs:range cdi:EnumerationDomain;
.


# class StatisticalClassification
# based on the UML class DDICDIModels::DDICDILibrary::Classes::Representations::StatisticalClassification
cdi:StatisticalClassification
  a rdfs:Class, owl:Class, ucmis:Class;
  rdfs:label "StatisticalClassification";
  rdfs:comment "Definition\n============\nSet of categories represented by classification items where the subset of immediate children categories for any given parent category are mutually exclusive and jointly exhaustive with respect to that parent.\n\nExamples\n==========\nISIC rev 4; NAICS 2017, SOC 2018\n\nExplanatory notes\n===================\nA statistical classification may have a flat, linear structure or may be hierarchically structured, such that all categories at lower levels are sub-categories of categories at the next Level up. (Source: GSIM StatisticalClassification)\nEach classification item represents a category. Every category is a member of a level within a statistical classification. The categories are defined with reference to one or more characteristics of a particular universe of units of observation."@en;
  rdfs:subClassOf cdi:EnumerationDomain;
.

cdi:StatisticalClassification-allowsDuplicates
  a rdf:Property, owl:DatatypeProperty, ucmis:Attribute;
  rdfs:label "allowsDuplicates";
  rdfs:comment "If value is False, the members are unique within the collection - if True, there may be duplicates. (Note that a mathematical “bag” permits duplicates and is unordered - a “set” does not have duplicates and may be ordered.)"@en;
  rdfs:domain cdi:StatisticalClassification;
  rdfs:range xsd:boolean;
.

cdi:StatisticalClassification-availableLanguage
  a rdf:Property, owl:DatatypeProperty, ucmis:Attribute;
  rdfs:label "availableLanguage";
  rdfs:comment "A list of languages in which the Statistical Classification is available. Supports the indication of multiple languages within a single property. Supports use of codes defined by the RFC 1766."@en;
  rdfs:domain cdi:StatisticalClassification;
  rdfs:range xsd:language;
.

cdi:StatisticalClassification-catalogDetails
  a rdf:Property, owl:ObjectProperty, ucmis:Attribute;
  rdfs:label "catalogDetails";
  rdfs:comment "Bundles the information useful for a data catalog entry. \n\nExamples would be creator, contributor, title, copyright, embargo, and license information\n\nA set of information useful for attribution, data discovery, and access.\nThis is information that is tied to the identity of the object. If this information changes the version of the associated object changes."@en;
  rdfs:domain cdi:StatisticalClassification;
  rdfs:range cdi:CatalogDetails;
.

cdi:StatisticalClassification-changeFromBase
  a rdf:Property, owl:ObjectProperty, ucmis:Attribute;
  rdfs:label "changeFromBase";
  rdfs:comment "Describes the relationship between the variant and its base Statistical Classification, including regroupings, aggregations added and extensions. (Source: GSIM StatisticalClassification/Changes from base Statistical Classification)."@en;
  rdfs:domain cdi:StatisticalClassification;
  rdfs:range cdi:InternationalString;
.

cdi:StatisticalClassification-copyright
  a rdf:Property, owl:ObjectProperty, ucmis:Attribute;
  rdfs:label "copyright";
  rdfs:comment "Copyright of the statistical classification."@en;
  rdfs:domain cdi:StatisticalClassification;
  rdfs:range cdi:InternationalString;
.

cdi:StatisticalClassification-displayLabel
  a rdf:Property, owl:ObjectProperty, ucmis:Attribute;
  rdfs:label "displayLabel";
  rdfs:comment "A human-readable display label for the object. Supports the use of multiple languages. Repeat for labels with different content, for example, labels with differing length limitations."@en;
  rdfs:domain cdi:StatisticalClassification;
  rdfs:range cdi:LabelForDisplay;
.

cdi:StatisticalClassification-isCurrent
  a rdf:Property, owl:DatatypeProperty, ucmis:Attribute;
  rdfs:label "isCurrent";
  rdfs:comment "Indicates if the statistical classification is currently valid."@en;
  rdfs:domain cdi:StatisticalClassification;
  rdfs:range xsd:boolean;
.

cdi:StatisticalClassification-isFloating
  a rdf:Property, owl:DatatypeProperty, ucmis:Attribute;
  rdfs:label "isFloating";
  rdfs:comment "Indicates if the Statistical Classification is a floating classification. In a floating statistical classification, a validity period should be defined for all classification Items which will allow the display of the item structure and content at different points of time. (Source: GSIM StatisticalClassification/Floating)."@en;
  rdfs:domain cdi:StatisticalClassification;
  rdfs:range xsd:boolean;
.

cdi:StatisticalClassification-purposeOfVariant
  a rdf:Property, owl:ObjectProperty, ucmis:Attribute;
  rdfs:label "purposeOfVariant";
  rdfs:comment "If the Statistical Classification is a variant, notes the specific purpose for which it was developed. (Source: GSIM StatisticalClassification/Purpose of variant)."@en;
  rdfs:domain cdi:StatisticalClassification;
  rdfs:range cdi:InternationalString;
.

cdi:StatisticalClassification-rationale
  a rdf:Property, owl:ObjectProperty, ucmis:Attribute;
  rdfs:label "rationale";
  rdfs:comment "Explanation of the reason(s) some decision was made or some object exists."@en;
  rdfs:domain cdi:StatisticalClassification;
  rdfs:range cdi:InternationalString;
.

cdi:StatisticalClassification-releaseDate
  a rdf:Property, owl:ObjectProperty, ucmis:Attribute;
  rdfs:label "releaseDate";
  rdfs:comment "Date when the current version of the Statistical Classification was released."@en;
  rdfs:domain cdi:StatisticalClassification;
  rdfs:range cdi:CombinedDate;
.

cdi:StatisticalClassification-updateChanges
  a rdf:Property, owl:ObjectProperty, ucmis:Attribute;
  rdfs:label "updateChanges";
  rdfs:comment "Summary description of changes which have occurred since the most recent classification version or classification update came into force."@en;
  rdfs:domain cdi:StatisticalClassification;
  rdfs:range cdi:InternationalString;
.

cdi:StatisticalClassification-usage
  a rdf:Property, owl:ObjectProperty, ucmis:Attribute;
  rdfs:label "usage";
  rdfs:comment "Explanation of the ways in which the object is employed."@en;
  rdfs:domain cdi:StatisticalClassification;
  rdfs:range cdi:InternationalString;
.

cdi:StatisticalClassification-validDates
  a rdf:Property, owl:ObjectProperty, ucmis:Attribute;
  rdfs:label "validDates";
  rdfs:comment "The dates describing the validity period of the object. The date from which the object became valid must be defined if the map belongs to a \"floating\" construct. The date at which the object became invalid must be defined if the map belongs to a \"floating\" construct and is no longer valid. Per the Generic Statistical Information Model, Statistical Classification: \"The date the statistical classification enters production use and the date on which the Statistical Classification was superseded by a successor version or otherwise ceased to be valid.\""@en;
  rdfs:domain cdi:StatisticalClassification;
  rdfs:range cdi:DateRange;
.


cdi:StatisticalClassification_isMaintainedBy_Organization
  a rdf:Property, owl:ObjectProperty, ucmis:Association;
  # ASSOCIATION
  rdfs:label "isMaintainedBy";
  skos:altLabel "StatisticalClassification_isMaintainedBy_Organization";
  rdfs:comment "Organization, agency, or group within an agency responsible for the maintenance and upkeep of the statistical classification."@en;
  rdfs:domain cdi:StatisticalClassification;
  rdfs:range cdi:Organization;
.

cdi:StatisticalClassification_has_ClassificationItem
  a rdf:Property, owl:ObjectProperty, ucmis:Association;
  # ASSOCIATION
  rdfs:label "has";
  skos:altLabel "StatisticalClassification_has_ClassificationItem";
  
  rdfs:domain cdi:StatisticalClassification;
  rdfs:range cdi:ClassificationItem;
.

cdi:StatisticalClassification_has_ClassificationItemPosition
  a rdf:Property, owl:ObjectProperty, ucmis:Association;
  # ASSOCIATION
  rdfs:label "has";
  skos:altLabel "StatisticalClassification_has_ClassificationItemPosition";
  
  rdfs:domain cdi:StatisticalClassification;
  rdfs:range cdi:ClassificationItemPosition;
.

cdi:StatisticalClassification_has_LevelStructure
  a rdf:Property, owl:ObjectProperty, ucmis:Association;
  # ASSOCIATION
  rdfs:label "has";
  skos:altLabel "StatisticalClassification_has_LevelStructure";
  
  rdfs:domain cdi:StatisticalClassification;
  rdfs:range cdi:LevelStructure;
.

cdi:StatisticalClassification_isIndexedBy_ClassificationIndex
  a rdf:Property, owl:ObjectProperty, ucmis:Association;
  # ASSOCIATION
  rdfs:label "isIndexedBy";
  skos:altLabel "StatisticalClassification_isIndexedBy_ClassificationIndex";
  
  rdfs:domain cdi:StatisticalClassification;
  rdfs:range cdi:ClassificationIndex;
.

cdi:StatisticalClassification_isPredecessorOf_StatisticalClassification
  a rdf:Property, owl:ObjectProperty, ucmis:Association;
  # ASSOCIATION
  rdfs:label "isPredecessorOf";
  skos:altLabel "StatisticalClassification_isPredecessorOf_StatisticalClassification";
  rdfs:comment "Statistical classification preceded by the actual statistical classification (for those statistical classifications that are versions or updates)."@en;
  rdfs:domain cdi:StatisticalClassification;
  rdfs:range cdi:StatisticalClassification;
.

cdi:StatisticalClassification_isSuccessorOf_StatisticalClassification
  a rdf:Property, owl:ObjectProperty, ucmis:Association;
  # ASSOCIATION
  rdfs:label "isSuccessorOf";
  skos:altLabel "StatisticalClassification_isSuccessorOf_StatisticalClassification";
  rdfs:comment "Statistical classification preceded by the actual statistical classification (for those statistical classifications that are versions or updates)."@en;
  rdfs:domain cdi:StatisticalClassification;
  rdfs:range cdi:StatisticalClassification;
.

cdi:StatisticalClassification_isVariantOf_StatisticalClassification
  a rdf:Property, owl:ObjectProperty, ucmis:Association;
  # ASSOCIATION
  rdfs:label "isVariantOf";
  skos:altLabel "StatisticalClassification_isVariantOf_StatisticalClassification";
  rdfs:comment "Statistical classification on which the current variant is based, and any subsequent versions of that statistical classification to which it is also applicable."@en;
  rdfs:domain cdi:StatisticalClassification;
  rdfs:range cdi:StatisticalClassification;
.


# class StatisticalClassificationRelationship
# based on the UML class DDICDIModels::DDICDILibrary::Classes::Representations::StatisticalClassificationRelationship
cdi:StatisticalClassificationRelationship
  a rdfs:Class, owl:Class, ucmis:Class;
  rdfs:label "StatisticalClassificationRelationship";
  rdfs:comment "Definition \n============ \nSpecifies the statistical classifications for the source and target of a complex relationship and defines the relationship."@en;
  
.

cdi:StatisticalClassificationRelationship-identifier
  a rdf:Property, owl:ObjectProperty, ucmis:Attribute;
  rdfs:label "identifier";
  rdfs:comment "Identifier for objects requiring short- or long-lasting referencing and management."@en;
  rdfs:domain cdi:StatisticalClassificationRelationship;
  rdfs:range cdi:Identifier;
.

cdi:StatisticalClassificationRelationship-semantics
  a rdf:Property, owl:ObjectProperty, ucmis:Attribute;
  rdfs:label "semantics";
  rdfs:comment "Specifies the semantics of the object in reference to a vocabulary, ontology, etc."@en;
  rdfs:domain cdi:StatisticalClassificationRelationship;
  rdfs:range cdi:ControlledVocabularyEntry;
.


cdi:StatisticalClassificationRelationship_hasSource_StatisticalClassification
  a rdf:Property, owl:ObjectProperty, ucmis:Association;
  # ASSOCIATION
  rdfs:label "hasSource";
  skos:altLabel "StatisticalClassificationRelationship_hasSource_StatisticalClassification";
  
  rdfs:domain cdi:StatisticalClassificationRelationship;
  rdfs:range cdi:StatisticalClassification;
.

cdi:StatisticalClassificationRelationship_hasTarget_StatisticalClassification
  a rdf:Property, owl:ObjectProperty, ucmis:Association;
  # ASSOCIATION
  rdfs:label "hasTarget";
  skos:altLabel "StatisticalClassificationRelationship_hasTarget_StatisticalClassification";
  
  rdfs:domain cdi:StatisticalClassificationRelationship;
  rdfs:range cdi:StatisticalClassification;
.


# class SubstantiveValueDomain
# based on the UML class DDICDIModels::DDICDILibrary::Classes::Representations::SubstantiveValueDomain
cdi:SubstantiveValueDomain
  a rdfs:Class, owl:Class, ucmis:Class;
  rdfs:label "SubstantiveValueDomain";
  rdfs:comment "Definition \n==========\nValue domain for a substantive conceptual domain. Typically a description and/or enumeration of allowed values of interest.  \n\nExamples \n========\nAll real decimal numbers relating to the subject matter of interest between 0 and 1 specified in Arabic numerals. (From the Generic Statistical Information Model [GSIM] 1.1). The codes \"M\" male and \"F\" for female .   \n\nExplanatory notes \n=================\nIn DDI-CDI the value domain for a variable is separated into \"substantive\" and \"sentinel\" values. Substantive values are the values of primary interest. Sentinel values are additional values that may carry supplementary information, such as reasons for missing. This duality is described in ISO 11404. Substantive values for height might be real numbers expressed in meters. The full value domain might also include codes for different kinds of missing values - one code for \"refused\" and another for \"don’t know\". Sentinel values may also convey some substantive information and at the same time represent missing values.\n\nAn example might be where a numeric variable like number of employees be sometimes a count and sometimes a code representing a range of counts in order to avoid disclosure of information about a specific entity. The substantive value domain may use either a value description, for described values, or a codelist for enumerated values, or both. A value domain may consist of substantive values or sentinel values. Substantive values are those associated directly with some subject matter area. They do not address concerns around processing, such as missing values. Substantive values are called \"regular values\" in ISO/IEC 11404 - General Purpose Datatypes. The enumerated case is one where all values are listed.\n\nAn example is the categorical values for gender: the conceptual domain could consist of the concept of male and the concept of female. These might be represented in codes and associated labels as 1 (\"Male\") 2 (\"Female\"). The described case is one where some description is needed to define the set of values. Take the following description for height in meters: \"a real number between 0 and 3, represented to two Arabic decimal places\". This description might be structured in some way to be machine actionable (datatype=\"double”, min=\"0\", max=\"3\", decimals=\"2\")."@en;
  rdfs:subClassOf cdi:ValueDomain;
.


cdi:SubstantiveValueDomain_takesConceptsFrom_SubstantiveConceptualDomain
  a rdf:Property, owl:ObjectProperty, ucmis:Association;
  # ASSOCIATION
  rdfs:label "takesConceptsFrom";
  skos:altLabel "SubstantiveValueDomain_takesConceptsFrom_SubstantiveConceptualDomain";
  rdfs:comment "Corresponding conceptual definition given by an substantive conceptual domain."@en;
  rdfs:domain cdi:SubstantiveValueDomain;
  rdfs:range cdi:SubstantiveConceptualDomain;
.

cdi:SubstantiveValueDomain_isDescribedBy_ValueAndConceptDescription
  a rdf:Property, owl:ObjectProperty, ucmis:Association;
  # ASSOCIATION
  rdfs:label "isDescribedBy";
  skos:altLabel "SubstantiveValueDomain_isDescribedBy_ValueAndConceptDescription";
  rdfs:comment "A formal description of the set of valid values - for described value domains."@en;
  rdfs:domain cdi:SubstantiveValueDomain;
  rdfs:range cdi:ValueAndConceptDescription;
.

cdi:SubstantiveValueDomain_takesValuesFrom_EnumerationDomain
  a rdf:Property, owl:ObjectProperty, ucmis:Association;
  # ASSOCIATION
  rdfs:label "takesValuesFrom";
  skos:altLabel "SubstantiveValueDomain_takesValuesFrom_EnumerationDomain";
  rdfs:comment "Any subtype of an enumeration domain enumerating the set of valid values."@en;
  rdfs:domain cdi:SubstantiveValueDomain;
  rdfs:range cdi:EnumerationDomain;
.


# class ValueAndConceptDescription
# based on the UML class DDICDIModels::DDICDILibrary::Classes::Representations::ValueAndConceptDescription
cdi:ValueAndConceptDescription
  a rdfs:Class, owl:Class, ucmis:Class;
  rdfs:label "ValueAndConceptDescription";
  rdfs:comment "Definition\n==========\nFormal description of a set of values.  \n\nExamples\n========\n\n1. The integers between 1 and 10, inclusive. The values of x satisfying the logicalExpression property: \" (1 less than or equal to X less than or equalto 10) AND mod(x,10)=0\" Also described with minimumValueInclusive = 1 and maximumValueInclusive = 10 (and datatype of integer).\n2. The upper case letters A through C and X described with the regularExpression \"/[A-CX]/\".\n3. A date-time described with the Unicode Locale Data Markup Language pattern yyyy.MM.dd G 'at' HH:mm:ss zzz.   \n\nExplanatory notes\n=================\nThe value and concept description may be used to describe either a value domain or a conceptual domain. For a value domain, the value and concept description contains the details for a described\" domain (as opposed to an enumerated domain). There are a number of properties which can be used for the description. The description could be just text such as: \"an even number greater than zero\", or a more formal logical expression like \"x>0 and mod(x,2)=0\". A regular expression might be useful for describing a textual domain. It could also employ a format pattern from the Unicode Locale Data Markup Language (LDML: http://www.unicode.org/reports/tr35/tr35.html). Some conceptual domains might be described with just a narrative. Others, though, might be described in much the same way as a value domain depending on the specificity of the concept. In ISO 11404 a value domain may be described either through enumeration or description, or both. This class provides the facility for that description. It may be just a text description, but a description through a logical expression is machine actionable and might, for example, be rendered as an integrity constraint. If both text and a logical expression are provided the logical expression is to be taken as the canonical description. The logical expression could conform to an expression syntax like that of the Validation and Transformation Language (VTL: https://sdmx.org/?page_id=5096) or the Structured Data Transformation Language (SDTL: https://ddialliance.org/products/sdtl/1.0)."@en;
  
.

cdi:ValueAndConceptDescription-classificationLevel
  a rdf:Property, owl:ObjectProperty, ucmis:Attribute;
  rdfs:label "classificationLevel";
  rdfs:comment "Indicates the type of relationship, nominal, ordinal, interval, ratio, or continuous. Use where appropriate for the representation type."@en;
  rdfs:domain cdi:ValueAndConceptDescription;
  rdfs:range cdi:CategoryRelationCode;
.

cdi:ValueAndConceptDescription-description
  a rdf:Property, owl:ObjectProperty, ucmis:Attribute;
  rdfs:label "description";
  rdfs:comment "A formal description of the set of values in human-readable language."@en;
  rdfs:domain cdi:ValueAndConceptDescription;
  rdfs:range cdi:InternationalString;
.

cdi:ValueAndConceptDescription-formatPattern
  a rdf:Property, owl:ObjectProperty, ucmis:Attribute;
  rdfs:label "formatPattern";
  rdfs:comment "A pattern for a number as described in Unicode Locale Data Markup Language (LDML) (http://www.unicode.org/reports/tr35/tr35.html) Part 3: Numbers  (http://www.unicode.org/reports/tr35/tr35-numbers.html#Number_Format_Patterns) and Part 4. Dates (http://www.unicode.org/reports/tr35/tr35-dates.html#Date_Format_Patterns) . Examples would be    #,##0.### to describe the pattern for a decimal number, or yyyy.MM.dd G 'at' HH:mm:ss zzz for a datetime pattern."@en;
  rdfs:domain cdi:ValueAndConceptDescription;
  rdfs:range cdi:ControlledVocabularyEntry;
.

cdi:ValueAndConceptDescription-identifier
  a rdf:Property, owl:ObjectProperty, ucmis:Attribute;
  rdfs:label "identifier";
  rdfs:comment "Identifier for objects requiring short- or long-lasting referencing and management."@en;
  rdfs:domain cdi:ValueAndConceptDescription;
  rdfs:range cdi:Identifier;
.

cdi:ValueAndConceptDescription-logicalExpression
  a rdf:Property, owl:ObjectProperty, ucmis:Attribute;
  rdfs:label "logicalExpression";
  rdfs:comment "A logical expression where the values of \"x\" making the expression true are the members of the set of valid values.  For example, \"(all reals x such that  x > 0)\" describes the real numbers greater than 0."@en;
  rdfs:domain cdi:ValueAndConceptDescription;
  rdfs:range cdi:ControlledVocabularyEntry;
.

cdi:ValueAndConceptDescription-maximumValueExclusive
  a rdf:Property, owl:DatatypeProperty, ucmis:Attribute;
  rdfs:label "maximumValueExclusive";
  rdfs:comment "A string denoting the maximum possible value (excluding this value). From the W3C Recommendation \"Metadata Vocabulary for Tabular Data\" (https://www.w3.org/TR/tabular-metadata/) 5.11.2: \"maxExclusive: An atomic property that contains a single number or string that is the maximum valid value (exclusive). The value of this property becomes the maximum exclusive annotation for the described datatype. See Value Constraints in [tabular-data-model] for details.\""@en;
  rdfs:domain cdi:ValueAndConceptDescription;
  rdfs:range xsd:string;
.

cdi:ValueAndConceptDescription-maximumValueInclusive
  a rdf:Property, owl:DatatypeProperty, ucmis:Attribute;
  rdfs:label "maximumValueInclusive";
  rdfs:comment "A string denoting the maximum possible value. From the W3C Recommendation \"Metadata Vocabulary for Tabular Data\" (https://www.w3.org/TR/tabular-metadata/) 5.11.2: \"maximum: An atomic property that contains a single number or string that is the maximum valid value (inclusive); equivalent to maxInclusive. The value of this property becomes the maximum annotation for the described datatype. See Value Constraints in [tabular-data-model] for details.\""@en;
  rdfs:domain cdi:ValueAndConceptDescription;
  rdfs:range xsd:string;
.

cdi:ValueAndConceptDescription-minimumValueExclusive
  a rdf:Property, owl:DatatypeProperty, ucmis:Attribute;
  rdfs:label "minimumValueExclusive";
  rdfs:comment "A string denoting the minimum possible value (excluding this value). From the W3C Recommendation \"Metadata Vocabulary for Tabular Data\" (https://www.w3.org/TR/tabular-metadata/) 5.11.2: \"minExclusive: An atomic property that contains a single number or string that is the minimum valid value (exclusive). The value of this property becomes the minimum exclusive annotation for the described datatype. See Value Constraints in [tabular-data-model] for details.\""@en;
  rdfs:domain cdi:ValueAndConceptDescription;
  rdfs:range xsd:string;
.

cdi:ValueAndConceptDescription-minimumValueInclusive
  a rdf:Property, owl:DatatypeProperty, ucmis:Attribute;
  rdfs:label "minimumValueInclusive";
  rdfs:comment "A string denoting the minimum possible value. From the W3C Recommendation \"Metadata Vocabulary for Tabular Data\" (https://www.w3.org/TR/tabular-metadata/) 5.11.2: \"minimum: An atomic property that contains a single number or string that is the minimum valid value (inclusive); equivalent to minInclusive. The value of this property becomes the minimum annotation for the described datatype. See Value Constraints in [tabular-data-model] for details.\""@en;
  rdfs:domain cdi:ValueAndConceptDescription;
  rdfs:range xsd:string;
.

cdi:ValueAndConceptDescription-regularExpression
  a rdf:Property, owl:ObjectProperty, ucmis:Attribute;
  rdfs:label "regularExpression";
  rdfs:comment "A regular expression where strings matching the expression belong to the set of valid values. Use typeOfContent to specify the syntax of the regularExpression found in content."@en;
  rdfs:domain cdi:ValueAndConceptDescription;
  rdfs:range cdi:TypedString;
.



# class ValueDomain
# based on the UML class DDICDIModels::DDICDILibrary::Classes::Representations::ValueDomain
cdi:ValueDomain
  a rdfs:Class, owl:Class, ucmis:Class;
  rdfs:label "ValueDomain";
  rdfs:comment "Definition \n============ \nSet of permissible values for a variable (adapted from ISO/IEC 11179).  \n\nExamples \n========== \nAge categories with a numeric code list; Age in years; Young, Middle-aged and Old.  \n\nExplanatory notes \n=================== \nThe values can be described by enumeration or by an expression. Value domains can be either substantive/sentinel, or described/enumeration."@en;
  
.

cdi:ValueDomain-catalogDetails
  a rdf:Property, owl:ObjectProperty, ucmis:Attribute;
  rdfs:label "catalogDetails";
  rdfs:comment "Bundles the information useful for a data catalog entry. \n\nExamples would be creator, contributor, title, copyright, embargo, and license information\n\nA set of information useful for attribution, data discovery, and access.\nThis is information that is tied to the identity of the object. If this information changes the version of the associated object changes."@en;
  rdfs:domain cdi:ValueDomain;
  rdfs:range cdi:CatalogDetails;
.

cdi:ValueDomain-displayLabel
  a rdf:Property, owl:ObjectProperty, ucmis:Attribute;
  rdfs:label "displayLabel";
  rdfs:comment "A human-readable display label for the object. Supports the use of multiple languages. Repeat for labels with different content, for example, labels with differing length limitations."@en;
  rdfs:domain cdi:ValueDomain;
  rdfs:range cdi:LabelForDisplay;
.

cdi:ValueDomain-identifier
  a rdf:Property, owl:ObjectProperty, ucmis:Attribute;
  rdfs:label "identifier";
  rdfs:comment "Identifier for objects requiring short- or long-lasting referencing and management."@en;
  rdfs:domain cdi:ValueDomain;
  rdfs:range cdi:Identifier;
.

cdi:ValueDomain-recommendedDataType
  a rdf:Property, owl:ObjectProperty, ucmis:Attribute;
  rdfs:label "recommendedDataType";
  rdfs:comment "The data types that are recommended for use with this domain."@en;
  rdfs:domain cdi:ValueDomain;
  rdfs:range cdi:ControlledVocabularyEntry;
.





