# PLEASE DO NOT EDIT THIS CODE!
# This code was generated by the Eclipse Acceleo module UCMIS M2T on 2023-05-25 10:41:35.
# Target language is 'Ontology Turtle' ('onto.ttl') generated on the basis of the model 'DDICDIModels'.

# Ontology for StructuredDataTypes
# based on the UML package DDICDIModels::DDICDILibrary::DataTypes::StructuredDataTypes
@prefix rdf:   <http://www.w3.org/1999/02/22-rdf-syntax-ns#> .
@prefix rdfs:  <http://www.w3.org/2000/01/rdf-schema#> .
@prefix owl:   <http://www.w3.org/2002/07/owl#> .
@prefix xsd:   <http://www.w3.org/2001/XMLSchema#> .
@prefix dc:    <http://purl.org/dc/elements/1.1/> .
@prefix skos:  <http://www.w3.org/2004/02/skos/core#> .
@prefix ucmis: <http://example.org/TODO/ucmis/> .
@prefix cdi:   <http://ddialliance.org/Specification/DDI-CDI/1.0/RDF/> .

<StructuredDataTypes.onto.ttl> a owl:Ontology;
  rdfs:label "StructuredDataTypes";
  rdfs:comment "This package contains classes which describe logical values that have a complex (multi-part) structure."@en;
.


# datatype AccessInformation
# based on the UML data type DDICDIModels::DDICDILibrary::DataTypes::StructuredDataTypes::AccessInformation
cdi:AccessInformation
  a rdfs:Class, owl:Class, ucmis:StructuredDataType;
  rdfs:label "AccessInformation";
  rdfs:comment "Definition\n============\nA set of information important for understanding access conditions. Examples include license, embargo details."@en;
  
  owl:hasKey (cdi:AccessInformation-copyright cdi:AccessInformation-embargo cdi:AccessInformation-license cdi:AccessInformation-rights);
.

cdi:AccessInformation-copyright
  a rdf:Property, owl:ObjectProperty, ucmis:Attribute;
  rdfs:label "copyright";
  rdfs:comment "The copyright statement."@en;
  rdfs:domain cdi:AccessInformation;
  rdfs:range cdi:InternationalString;
.

cdi:AccessInformation-embargo
  a rdf:Property, owl:ObjectProperty, ucmis:Attribute;
  rdfs:label "embargo";
  rdfs:comment "Specific information about any relevant embargo"@en;
  rdfs:domain cdi:AccessInformation;
  rdfs:range cdi:EmbargoInformation;
.

cdi:AccessInformation-license
  a rdf:Property, owl:ObjectProperty, ucmis:Attribute;
  rdfs:label "license";
  rdfs:comment "Information about any relevant license"@en;
  rdfs:domain cdi:AccessInformation;
  rdfs:range cdi:LicenseInformation;
.

cdi:AccessInformation-rights
  a rdf:Property, owl:ObjectProperty, ucmis:Attribute;
  rdfs:label "rights";
  rdfs:comment "Information about rights held in and over the resource. Typically, rights information includes a statement about various property rights associated with the resource, including intellectual property rights."@en;
  rdfs:domain cdi:AccessInformation;
  rdfs:range cdi:InternationalString;
.


# datatype AccessLocation
# based on the UML data type DDICDIModels::DDICDILibrary::DataTypes::StructuredDataTypes::AccessLocation
cdi:AccessLocation
  a rdfs:Class, owl:Class, ucmis:StructuredDataType;
  rdfs:label "AccessLocation";
  rdfs:comment "Definition\n============\nA set of access information for a machine including URI, mime type, and physical location."@en;
  
  owl:hasKey (cdi:AccessLocation-mimeType cdi:AccessLocation-physicalLocation cdi:AccessLocation-uri);
.

cdi:AccessLocation-mimeType
  a rdf:Property, owl:ObjectProperty, ucmis:Attribute;
  rdfs:label "mimeType";
  rdfs:comment "The MIME type. MIME stands for \"Multipurpose Internet Mail Extensions. It's a way of identifying files on the Internet according to their nature and format. Supports the use of an controlled vocabulary."@en;
  rdfs:domain cdi:AccessLocation;
  rdfs:range cdi:ControlledVocabularyEntry;
.

cdi:AccessLocation-physicalLocation
  a rdf:Property, owl:ObjectProperty, ucmis:Attribute;
  rdfs:label "physicalLocation";
  rdfs:comment "The physical location of the machine."@en;
  rdfs:domain cdi:AccessLocation;
  rdfs:range cdi:InternationalString;
.

cdi:AccessLocation-uri
  a rdf:Property, owl:DatatypeProperty, ucmis:Attribute;
  rdfs:label "uri";
  rdfs:comment "A Uniform Resource Identifier (URI) is a string of characters that unambiguously identifies a particular resource. A URI is normally expressed as a URL."@en;
  rdfs:domain cdi:AccessLocation;
  rdfs:range xsd:anyURI;
.


# datatype Address
# based on the UML data type DDICDIModels::DDICDILibrary::DataTypes::StructuredDataTypes::Address
cdi:Address
  a rdfs:Class, owl:Class, ucmis:StructuredDataType;
  rdfs:label "Address";
  rdfs:comment "Definition\n==========\nLocation address identifying each part of the address as separate elements, identifying the type of address, the level of privacy associated with the release of the address, and a flag to identify the preferred address for contact.\n\nExamples\n========\nFor example:\n\n1. OFFICE, ABS HOUSE, 45 Benjamin Way, Belconnen, Canberra, ACT, 2617, AU\n2. OFFICE, Institute of Education, 20 Bedford Way, London, WC1H 0AL, UK"@en;
  
  owl:hasKey (cdi:Address-cityPlaceLocal cdi:Address-countryCode cdi:Address-effectiveDates cdi:Address-geographicPoint cdi:Address-isPreferred cdi:Address-line cdi:Address-locationName cdi:Address-postalCode cdi:Address-privacy cdi:Address-regionalCoverage cdi:Address-stateProvince cdi:Address-timeZone cdi:Address-typeOfAddress cdi:Address-typeOfLocation);
.

cdi:Address-cityPlaceLocal
  a rdf:Property, owl:DatatypeProperty, ucmis:Attribute;
  rdfs:label "cityPlaceLocal";
  rdfs:comment "City, place, or local area used as part of an address."@en;
  rdfs:domain cdi:Address;
  rdfs:range xsd:string;
.

cdi:Address-countryCode
  a rdf:Property, owl:ObjectProperty, ucmis:Attribute;
  rdfs:label "countryCode";
  rdfs:comment "Country of the location."@en;
  rdfs:domain cdi:Address;
  rdfs:range cdi:ControlledVocabularyEntry;
.

cdi:Address-effectiveDates
  a rdf:Property, owl:ObjectProperty, ucmis:Attribute;
  rdfs:label "effectiveDates";
  rdfs:comment "Clarifies when the identification information is accurate."@en;
  rdfs:domain cdi:Address;
  rdfs:range cdi:DateRange;
.

cdi:Address-geographicPoint
  a rdf:Property, owl:ObjectProperty, ucmis:Attribute;
  rdfs:label "geographicPoint";
  rdfs:comment "Geographic coordinates corresponding to the address."@en;
  rdfs:domain cdi:Address;
  rdfs:range cdi:SpatialPoint;
.

cdi:Address-isPreferred
  a rdf:Property, owl:DatatypeProperty, ucmis:Attribute;
  rdfs:label "isPreferred";
  rdfs:comment "Set to True if this is the preferred location for contacting the organization or individual."@en;
  rdfs:domain cdi:Address;
  rdfs:range xsd:boolean;
.

cdi:Address-line
  a rdf:Property, owl:DatatypeProperty, ucmis:Attribute;
  rdfs:label "line";
  rdfs:comment "Number and street including office or suite number. May use multiple lines."@en;
  rdfs:domain cdi:Address;
  rdfs:range xsd:string;
.

cdi:Address-locationName
  a rdf:Property, owl:ObjectProperty, ucmis:Attribute;
  rdfs:label "locationName";
  rdfs:comment "Name of the location if applicable."@en;
  rdfs:domain cdi:Address;
  rdfs:range cdi:ObjectName;
.

cdi:Address-postalCode
  a rdf:Property, owl:DatatypeProperty, ucmis:Attribute;
  rdfs:label "postalCode";
  rdfs:comment "Postal or ZIP Code."@en;
  rdfs:domain cdi:Address;
  rdfs:range xsd:string;
.

cdi:Address-privacy
  a rdf:Property, owl:ObjectProperty, ucmis:Attribute;
  rdfs:label "privacy";
  rdfs:comment "Specify the level privacy for the address as public, restricted, or private. Supports the use of an external controlled vocabulary."@en;
  rdfs:domain cdi:Address;
  rdfs:range cdi:ControlledVocabularyEntry;
.

cdi:Address-regionalCoverage
  a rdf:Property, owl:ObjectProperty, ucmis:Attribute;
  rdfs:label "regionalCoverage";
  rdfs:comment "The region covered by the agent at this address."@en;
  rdfs:domain cdi:Address;
  rdfs:range cdi:ControlledVocabularyEntry;
.

cdi:Address-stateProvince
  a rdf:Property, owl:DatatypeProperty, ucmis:Attribute;
  rdfs:label "stateProvince";
  rdfs:comment "A major sub-national division such as a state or province used to identify a major region within an address."@en;
  rdfs:domain cdi:Address;
  rdfs:range xsd:string;
.

cdi:Address-timeZone
  a rdf:Property, owl:ObjectProperty, ucmis:Attribute;
  rdfs:label "timeZone";
  rdfs:comment "Time zone of the location expressed as code."@en;
  rdfs:domain cdi:Address;
  rdfs:range cdi:ControlledVocabularyEntry;
.

cdi:Address-typeOfAddress
  a rdf:Property, owl:ObjectProperty, ucmis:Attribute;
  rdfs:label "typeOfAddress";
  rdfs:comment "Indicates address type (i.e. home, office, mailing, etc.)."@en;
  rdfs:domain cdi:Address;
  rdfs:range cdi:ControlledVocabularyEntry;
.

cdi:Address-typeOfLocation
  a rdf:Property, owl:ObjectProperty, ucmis:Attribute;
  rdfs:label "typeOfLocation";
  rdfs:comment "The type or purpose of the location (i.e. regional office, distribution center, home)."@en;
  rdfs:domain cdi:Address;
  rdfs:range cdi:ControlledVocabularyEntry;
.


# datatype AgentInRole
# based on the UML data type DDICDIModels::DDICDILibrary::DataTypes::StructuredDataTypes::AgentInRole
cdi:AgentInRole
  a rdfs:Class, owl:Class, ucmis:StructuredDataType;
  rdfs:label "AgentInRole";
  rdfs:comment "Definition\n==========\nA reference to an agent (organization, individual, or machine) including a role for that agent in the context of this specific reference.\n\nExamples\n========\nReference to John Doe as the lead author."@en;
  
  owl:hasKey (cdi:AgentInRole-agentName cdi:AgentInRole-reference cdi:AgentInRole-role);
.

cdi:AgentInRole-agentName
  a rdf:Property, owl:ObjectProperty, ucmis:Attribute;
  rdfs:label "agentName";
  rdfs:comment "Full name of the contributor. Language equivalents should be expressed within the international string structure."@en;
  rdfs:domain cdi:AgentInRole;
  rdfs:range cdi:BibliographicName;
.

cdi:AgentInRole-reference
  a rdf:Property, owl:ObjectProperty, ucmis:Attribute;
  rdfs:label "reference";
  rdfs:comment "Reference to an agent described in DDI or some other platform."@en;
  rdfs:domain cdi:AgentInRole;
  rdfs:range cdi:Reference;
.

cdi:AgentInRole-role
  a rdf:Property, owl:ObjectProperty, ucmis:Attribute;
  rdfs:label "role";
  rdfs:comment "Role of the of the agent within the context of the parent property name."@en;
  rdfs:domain cdi:AgentInRole;
  rdfs:range cdi:PairedControlledVocabularyEntry;
.


# datatype BibliographicName
# based on the UML data type DDICDIModels::DDICDILibrary::DataTypes::StructuredDataTypes::BibliographicName
cdi:BibliographicName
  a rdfs:Class, owl:Class, ucmis:StructuredDataType;
  rdfs:label "BibliographicName";
  rdfs:comment "Definition\n============\nPersonal names should be listed surname or family name first, followed by forename or given name. When in doubt, give the name as it appears, and do not invert. In the case of organizations where there is clearly a hierarchy present, list the parts of the hierarchy from largest to smallest, separated by full stops and a space. If it is not clear whether there is a hierarchy present, or unclear which is the larger or smaller portion of the body, give the name as it appears in the item. The name may be provided in one or more languages."@en;
  rdfs:subClassOf cdi:InternationalString;
  owl:hasKey (cdi:BibliographicName-affiliation);
.

cdi:BibliographicName-affiliation
  a rdf:Property, owl:DatatypeProperty, ucmis:Attribute;
  rdfs:label "affiliation";
  rdfs:comment "The affiliation of this person to an organization. This is generally an organization or sub-organization name and should be related to the specific role within which the individual is being listed."@en;
  rdfs:domain cdi:BibliographicName;
  rdfs:range xsd:string;
.


# datatype CatalogDetails
# based on the UML data type DDICDIModels::DDICDILibrary::DataTypes::StructuredDataTypes::CatalogDetails
cdi:CatalogDetails
  a rdfs:Class, owl:Class, ucmis:StructuredDataType;
  rdfs:label "CatalogDetails";
  rdfs:comment "Definition\n============\nA set of information useful for attribution, data discovery, and access.\n\nExamples\n==========\nCreator, contributor, title, copyright, license information."@en;
  
  owl:hasKey (cdi:CatalogDetails-access cdi:CatalogDetails-alternativeTitle cdi:CatalogDetails-contributor cdi:CatalogDetails-creator cdi:CatalogDetails-date cdi:CatalogDetails-identifier cdi:CatalogDetails-informationSource cdi:CatalogDetails-languageOfObject cdi:CatalogDetails-provenance cdi:CatalogDetails-publisher cdi:CatalogDetails-relatedResource cdi:CatalogDetails-subTitle cdi:CatalogDetails-summary cdi:CatalogDetails-title cdi:CatalogDetails-typeOfResource);
.

cdi:CatalogDetails-access
  a rdf:Property, owl:ObjectProperty, ucmis:Attribute;
  rdfs:label "access";
  rdfs:comment "Information important for understanding access conditions."@en;
  rdfs:domain cdi:CatalogDetails;
  rdfs:range cdi:AccessInformation;
.

cdi:CatalogDetails-alternativeTitle
  a rdf:Property, owl:ObjectProperty, ucmis:Attribute;
  rdfs:label "alternativeTitle";
  rdfs:comment "An alternative title by which a data collection is commonly referred, or an abbreviation for the title."@en;
  rdfs:domain cdi:CatalogDetails;
  rdfs:range cdi:InternationalString;
.

cdi:CatalogDetails-contributor
  a rdf:Property, owl:ObjectProperty, ucmis:Attribute;
  rdfs:label "contributor";
  rdfs:comment "The name of a contributing author or creator, who worked in support of the primary creator given above."@en;
  rdfs:domain cdi:CatalogDetails;
  rdfs:range cdi:AgentInRole;
.

cdi:CatalogDetails-creator
  a rdf:Property, owl:ObjectProperty, ucmis:Attribute;
  rdfs:label "creator";
  rdfs:comment "Person, corporate body, or agency responsible for the substantive and intellectual content of the described object."@en;
  rdfs:domain cdi:CatalogDetails;
  rdfs:range cdi:AgentInRole;
.

cdi:CatalogDetails-date
  a rdf:Property, owl:ObjectProperty, ucmis:Attribute;
  rdfs:label "date";
  rdfs:comment "A date associated with the annotated object (not the coverage period). Use typeOfDate to specify the type of date such as Version, Publication, Submitted, Copyrighted, Accepted, etc."@en;
  rdfs:domain cdi:CatalogDetails;
  rdfs:range cdi:CombinedDate;
.

cdi:CatalogDetails-identifier
  a rdf:Property, owl:ObjectProperty, ucmis:Attribute;
  rdfs:label "identifier";
  rdfs:comment "An identifier or locator. Contains identifier and Managing agency (ISBN, ISSN, DOI, local archive). Indicates if it is a URI."@en;
  rdfs:domain cdi:CatalogDetails;
  rdfs:range cdi:InternationalIdentifier;
.

cdi:CatalogDetails-informationSource
  a rdf:Property, owl:ObjectProperty, ucmis:Attribute;
  rdfs:label "informationSource";
  rdfs:comment "The name or identifier of source information for the annotated object."@en;
  rdfs:domain cdi:CatalogDetails;
  rdfs:range cdi:InternationalString;
.

cdi:CatalogDetails-languageOfObject
  a rdf:Property, owl:DatatypeProperty, ucmis:Attribute;
  rdfs:label "languageOfObject";
  rdfs:comment "Language of the intellectual content of the described object. Multiple languages are supported by the structure itself as defined in the transformation to specific bindings. Use language codes supported by xs:language which include the 2 and 3 character and extended structures defined by RFC4646 or its successors. Supports multiple language codes."@en;
  rdfs:domain cdi:CatalogDetails;
  rdfs:range xsd:language;
.

cdi:CatalogDetails-provenance
  a rdf:Property, owl:ObjectProperty, ucmis:Attribute;
  rdfs:label "provenance";
  rdfs:comment "Information about the origins of the object."@en;
  rdfs:domain cdi:CatalogDetails;
  rdfs:range cdi:ProvenanceInformation;
.

cdi:CatalogDetails-publisher
  a rdf:Property, owl:ObjectProperty, ucmis:Attribute;
  rdfs:label "publisher";
  rdfs:comment "Person or organization responsible for making the resource available in its present form."@en;
  rdfs:domain cdi:CatalogDetails;
  rdfs:range cdi:AgentInRole;
.

cdi:CatalogDetails-relatedResource
  a rdf:Property, owl:ObjectProperty, ucmis:Attribute;
  rdfs:label "relatedResource";
  rdfs:comment "Provide the identifier, managing agency, and type of resource related to this object. Use to specify related resources similar to Dublin Core isPartOf and hasPart to indicate collection/series membership for objects where there is an identifiable record. If not an identified object use the relationship to ExternalMaterial using a type that indicates a series description."@en;
  rdfs:domain cdi:CatalogDetails;
  rdfs:range cdi:Reference;
.

cdi:CatalogDetails-subTitle
  a rdf:Property, owl:ObjectProperty, ucmis:Attribute;
  rdfs:label "subTitle";
  rdfs:comment "Secondary or explanatory title."@en;
  rdfs:domain cdi:CatalogDetails;
  rdfs:range cdi:InternationalString;
.

cdi:CatalogDetails-summary
  a rdf:Property, owl:ObjectProperty, ucmis:Attribute;
  rdfs:label "summary";
  rdfs:comment "A summary description (abstract) of the annotated object."@en;
  rdfs:domain cdi:CatalogDetails;
  rdfs:range cdi:InternationalString;
.

cdi:CatalogDetails-title
  a rdf:Property, owl:ObjectProperty, ucmis:Attribute;
  rdfs:label "title";
  rdfs:comment "Full authoritative title. List any additional titles for this item as alternativeTitle."@en;
  rdfs:domain cdi:CatalogDetails;
  rdfs:range cdi:InternationalString;
.

cdi:CatalogDetails-typeOfResource
  a rdf:Property, owl:ObjectProperty, ucmis:Attribute;
  rdfs:label "typeOfResource";
  rdfs:comment "Provide the type of the resource. This supports the use of a controlled vocabulary. It should be appropriate to the level of the annotation."@en;
  rdfs:domain cdi:CatalogDetails;
  rdfs:range cdi:ControlledVocabularyEntry;
.


# datatype CombinedDate
# based on the UML data type DDICDIModels::DDICDILibrary::DataTypes::StructuredDataTypes::CombinedDate
cdi:CombinedDate
  a rdfs:Class, owl:Class, ucmis:StructuredDataType;
  rdfs:label "CombinedDate";
  rdfs:comment "Definition\n============\nProvides the structure of a single Date expressed in an ISO date structure along with equivalent expression in any number of non-ISO formats. While it supports the use of the ISO time interval structure this should only be used when the exact date is unclear (i.e. occurring at some point in time between the two specified dates) or in specified applications. Ranges with specified start and end dates should use the DateRange as a datatype. Commonly uses property names include: eventDate, issueDate, and releaseDate.\n\nExplanatory notes\n===================\nDate allows one of a set of date-time (YYYY-MM-DDThh:mm:ss), date (YYYY-MM-DD), year-month (YYYY-MM), year (YYYY), time (hh:mm:ss) and duration (PnYnMnDnHnMnS), or time interval (YYYY-MM-DDThh:mm:ss/YYYY-MM-DDThh:mm:ss, YYYY-MM-DDThh:mm:ss/PnYnMnDnHnMnS, PnYnMnDnHnMnS/ YYYY-MM-DDThh:mm:ss) which is formatted according to ISO 8601 and backed supported by regular expressions in the BaseDateType. Time Zone designation and negative/positive prefixes are allowed as are dates before and after 0000 through 9999."@en;
  
  owl:hasKey (cdi:CombinedDate-isoDate cdi:CombinedDate-nonIsoDate cdi:CombinedDate-semantics);
.

cdi:CombinedDate-isoDate
  a rdf:Property, owl:DatatypeProperty, ucmis:Attribute;
  rdfs:label "isoDate";
  rdfs:comment "Strongly recommend that ALL dates be expressed in an ISO format at a minimum. A single point in time expressed in an ISO standard structure. Note that while it supports an ISO date range structure this should be used in Date only when the single date is unclear i.e. occurring at some time between two dates."@en;
  rdfs:domain cdi:CombinedDate;
  rdfs:range xsd:date;
.

cdi:CombinedDate-nonIsoDate
  a rdf:Property, owl:ObjectProperty, ucmis:Attribute;
  rdfs:label "nonIsoDate";
  rdfs:comment "A simple date expressed in a non-ISO date format, including a specification of the date format and calendar used."@en;
  rdfs:domain cdi:CombinedDate;
  rdfs:range cdi:NonIsoDate;
.

cdi:CombinedDate-semantics
  a rdf:Property, owl:ObjectProperty, ucmis:Attribute;
  rdfs:label "semantics";
  rdfs:comment "Use to specify the type of date. This may reflect the refinements of dc:date such as dateAccepted, dateCopyrighted, dateSubmitted, etc."@en;
  rdfs:domain cdi:CombinedDate;
  rdfs:range cdi:ControlledVocabularyEntry;
.


# datatype Command
# based on the UML data type DDICDIModels::DDICDILibrary::DataTypes::StructuredDataTypes::Command
cdi:Command
  a rdfs:Class, owl:Class, ucmis:StructuredDataType;
  rdfs:label "Command";
  rdfs:comment "Definition\n============\nProvides the following information on the command: The content of the command and the programming language used."@en;
  
  owl:hasKey (cdi:Command-commandContent cdi:Command-programLanguage);
.

cdi:Command-commandContent
  a rdf:Property, owl:ObjectProperty, ucmis:Attribute;
  rdfs:label "commandContent";
  rdfs:comment "Content of the command itself expressed in the language designated in programming language."@en;
  rdfs:domain cdi:Command;
  rdfs:range cdi:TypedString;
.

cdi:Command-programLanguage
  a rdf:Property, owl:ObjectProperty, ucmis:Attribute;
  rdfs:label "programLanguage";
  rdfs:comment "Designates the programming language used for the command. Supports the use of a controlled vocabulary."@en;
  rdfs:domain cdi:Command;
  rdfs:range cdi:ControlledVocabularyEntry;
.


# datatype CommandCode
# based on the UML data type DDICDIModels::DDICDILibrary::DataTypes::StructuredDataTypes::CommandCode
cdi:CommandCode
  a rdfs:Class, owl:Class, ucmis:StructuredDataType;
  rdfs:label "CommandCode";
  rdfs:comment "Definition\n============\nContains information on the command used for processing data. Contains a description of the command which should clarify for the user the purpose and process of the command, an in-line provision of the command itself, and a reference to an external version of the command such as a coding script."@en;
  
  owl:hasKey (cdi:CommandCode-command cdi:CommandCode-commandFile cdi:CommandCode-description);
.

cdi:CommandCode-command
  a rdf:Property, owl:ObjectProperty, ucmis:Attribute;
  rdfs:label "command";
  rdfs:comment "This is an in-line provision of the command itself. It provides the programming language used as well as the command."@en;
  rdfs:domain cdi:CommandCode;
  rdfs:range cdi:Command;
.

cdi:CommandCode-commandFile
  a rdf:Property, owl:ObjectProperty, ucmis:Attribute;
  rdfs:label "commandFile";
  rdfs:comment "Identifies and provides a link to an external copy of the command, for example, a SAS Command Code script. Designates the programming language of the command file as well as the URI for the file."@en;
  rdfs:domain cdi:CommandCode;
  rdfs:range cdi:CommandFile;
.

cdi:CommandCode-description
  a rdf:Property, owl:ObjectProperty, ucmis:Attribute;
  rdfs:label "description";
  rdfs:comment "A description of the purpose and use of the command code provided. Supports multiple languages."@en;
  rdfs:domain cdi:CommandCode;
  rdfs:range cdi:InternationalString;
.


# datatype CommandFile
# based on the UML data type DDICDIModels::DDICDILibrary::DataTypes::StructuredDataTypes::CommandFile
cdi:CommandFile
  a rdfs:Class, owl:Class, ucmis:StructuredDataType;
  rdfs:label "CommandFile";
  rdfs:comment "Definition\n============\nIdentifies and provides a link to an external copy of the command, for example, a SAS Command Code script. Designates the programming language of the command file, a description of the location of the file , and a URN or URL for the command file."@en;
  
  owl:hasKey (cdi:CommandFile-location cdi:CommandFile-uri);
.

cdi:CommandFile-location
  a rdf:Property, owl:ObjectProperty, ucmis:Attribute;
  rdfs:label "location";
  rdfs:comment "A description of the location of the file. This may not be machine actionable. It supports a description expressed in multiple languages."@en;
  rdfs:domain cdi:CommandFile;
  rdfs:range cdi:InternationalString;
.

cdi:CommandFile-uri
  a rdf:Property, owl:DatatypeProperty, ucmis:Attribute;
  rdfs:label "uri";
  rdfs:comment "The URL or URN of the command file."@en;
  rdfs:domain cdi:CommandFile;
  rdfs:range xsd:anyURI;
.


# datatype ComplexLanguageString
# based on the UML data type DDICDIModels::DDICDILibrary::DataTypes::StructuredDataTypes::ComplexLanguageString
cdi:ComplexLanguageString
  a rdfs:Class, owl:Class, ucmis:StructuredDataType;
  rdfs:label "ComplexLanguageString";
  rdfs:comment "Definition\n============\nAllows for non-formatted language specific strings that may be translations from other languages, or that may be translatable into other languages. Only one string per language/scope type is allowed. Language specific string contains the following attributes, xmlang to designate the language, isTranslated with a default value of false to designate if an object is a translation of another language, isTranslatable with a default value of true to designate if the content can be translated, translationSourceLanguage to indicate the source languages used in creating this translation, translationDate, and scope which can be used to define intended audience or use such as internal, external, etc."@en;
  rdfs:subClassOf rdf:langString;
  owl:hasKey (cdi:ComplexLanguageString-isTranslatable cdi:ComplexLanguageString-isTranslated cdi:ComplexLanguageString-scope cdi:ComplexLanguageString-structureUsed cdi:ComplexLanguageString-translationDate cdi:ComplexLanguageString-translationSourceLanguage);
.

cdi:ComplexLanguageString-isTranslatable
  a rdf:Property, owl:DatatypeProperty, ucmis:Attribute;
  rdfs:label "isTranslatable";
  rdfs:comment "Indicates whether content is translatable (True) or not (False). An example of something that is not translatable would be a MNEMONIC of an object or a number."@en;
  rdfs:domain cdi:ComplexLanguageString;
  rdfs:range xsd:boolean;
.

cdi:ComplexLanguageString-isTranslated
  a rdf:Property, owl:DatatypeProperty, ucmis:Attribute;
  rdfs:label "isTranslated";
  rdfs:comment "Indicates whether content is a translation (True) or an original (False)."@en;
  rdfs:domain cdi:ComplexLanguageString;
  rdfs:range xsd:boolean;
.

cdi:ComplexLanguageString-scope
  a rdf:Property, owl:DatatypeProperty, ucmis:Attribute;
  rdfs:label "scope";
  rdfs:comment "Supports specification of scope for the contained content. Use with the language specification to filter application of content."@en;
  rdfs:domain cdi:ComplexLanguageString;
  rdfs:range xsd:string;
.

cdi:ComplexLanguageString-structureUsed
  a rdf:Property, owl:ObjectProperty, ucmis:Attribute;
  rdfs:label "structureUsed";
  rdfs:comment "The structure type used. Examples are HTML or restructured text."@en;
  rdfs:domain cdi:ComplexLanguageString;
  rdfs:range cdi:ControlledVocabularyEntry;
.

cdi:ComplexLanguageString-translationDate
  a rdf:Property, owl:DatatypeProperty, ucmis:Attribute;
  rdfs:label "translationDate";
  rdfs:comment "The date the content was translated. Provision of translation date allows user to verify if translation was available during data collection or other time linked activity."@en;
  rdfs:domain cdi:ComplexLanguageString;
  rdfs:range xsd:date;
.

cdi:ComplexLanguageString-translationSourceLanguage
  a rdf:Property, owl:DatatypeProperty, ucmis:Attribute;
  rdfs:label "translationSourceLanguage";
  rdfs:comment "List the language code of the source. Repeat of multiple language sources are used."@en;
  rdfs:domain cdi:ComplexLanguageString;
  rdfs:range xsd:language;
.


# datatype ContactInformation
# based on the UML data type DDICDIModels::DDICDILibrary::DataTypes::StructuredDataTypes::ContactInformation
cdi:ContactInformation
  a rdfs:Class, owl:Class, ucmis:StructuredDataType;
  rdfs:label "ContactInformation";
  rdfs:comment "Definition\n============\nContact information for the individual or organization including location specification, address, web site, phone numbers, and other means of communication access. Address, location, telephone, and other means of communication can be repeated to express multiple means of a single type or change over time. Each major piece of contact information contains the element effectiveDates in order to date stamp the period for which the information is valid."@en;
  
  owl:hasKey (cdi:ContactInformation-address cdi:ContactInformation-email cdi:ContactInformation-emessaging cdi:ContactInformation-telephone cdi:ContactInformation-website);
.

cdi:ContactInformation-address
  a rdf:Property, owl:ObjectProperty, ucmis:Attribute;
  rdfs:label "address";
  rdfs:comment "The address for contact."@en;
  rdfs:domain cdi:ContactInformation;
  rdfs:range cdi:Address;
.

cdi:ContactInformation-email
  a rdf:Property, owl:ObjectProperty, ucmis:Attribute;
  rdfs:label "email";
  rdfs:comment "Email contact information."@en;
  rdfs:domain cdi:ContactInformation;
  rdfs:range cdi:Email;
.

cdi:ContactInformation-emessaging
  a rdf:Property, owl:ObjectProperty, ucmis:Attribute;
  rdfs:label "emessaging";
  rdfs:comment "Electronic messaging other than email."@en;
  rdfs:domain cdi:ContactInformation;
  rdfs:range cdi:ElectronicMessageSystem;
.

cdi:ContactInformation-telephone
  a rdf:Property, owl:ObjectProperty, ucmis:Attribute;
  rdfs:label "telephone";
  rdfs:comment "Telephone for contact."@en;
  rdfs:domain cdi:ContactInformation;
  rdfs:range cdi:Telephone;
.

cdi:ContactInformation-website
  a rdf:Property, owl:ObjectProperty, ucmis:Attribute;
  rdfs:label "website";
  rdfs:comment "The URL of the Agent's website."@en;
  rdfs:domain cdi:ContactInformation;
  rdfs:range cdi:WebLink;
.


# datatype ControlledVocabularyEntry
# based on the UML data type DDICDIModels::DDICDILibrary::DataTypes::StructuredDataTypes::ControlledVocabularyEntry
cdi:ControlledVocabularyEntry
  a rdfs:Class, owl:Class, ucmis:StructuredDataType;
  rdfs:label "ControlledVocabularyEntry";
  rdfs:comment "Definition\n============\nAllows for unstructured content which may be an entry from an externally maintained controlled vocabulary.If the content is from a controlled vocabulary provide the code value of the entry, as well as a reference to the controlled vocabulary from which the value is taken. Provide as many of the identifying attributes as needed to adequately identify the controlled vocabulary. Note that DDI has published a number of controlled vocabularies applicable to several locations using the external controlled vocabulary entry structure. If the code portion of the controlled vocabulary entry is language specific (i.e. a list of keywords or subject headings) use language to specify that language. In most cases the code portion of an entry is not language specific although the description and usage may be managed in one or more languages. Use of shared controlled vocabularies helps support interoperability and machine actionability."@en;
  
  owl:hasKey (cdi:ControlledVocabularyEntry-entryReference cdi:ControlledVocabularyEntry-entryValue cdi:ControlledVocabularyEntry-name cdi:ControlledVocabularyEntry-valueForOther cdi:ControlledVocabularyEntry-vocabulary);
.

cdi:ControlledVocabularyEntry-entryReference
  a rdf:Property, owl:ObjectProperty, ucmis:Attribute;
  rdfs:label "entryReference";
  rdfs:comment "A reference to the specific item in the vocabulary referenced in the vocabulary attribute, using a URI or other resolvable identifier."@en;
  rdfs:domain cdi:ControlledVocabularyEntry;
  rdfs:range cdi:Reference;
.

cdi:ControlledVocabularyEntry-entryValue
  a rdf:Property, owl:DatatypeProperty, ucmis:Attribute;
  rdfs:label "entryValue";
  rdfs:comment "The value of the entry of the controlled vocabulary. If no controlled vocabulary is used the term is entered here and none of the properties defining the controlled vocabulary location are used."@en;
  rdfs:domain cdi:ControlledVocabularyEntry;
  rdfs:range xsd:string;
.

cdi:ControlledVocabularyEntry-name
  a rdf:Property, owl:DatatypeProperty, ucmis:Attribute;
  rdfs:label "name";
  rdfs:comment "The name of the code list (controlled vocabulary)."@en;
  rdfs:domain cdi:ControlledVocabularyEntry;
  rdfs:range xsd:string;
.

cdi:ControlledVocabularyEntry-valueForOther
  a rdf:Property, owl:DatatypeProperty, ucmis:Attribute;
  rdfs:label "valueForOther";
  rdfs:comment "If the value of the string is \"Other\" or the equivalent from the codelist, this attribute can provide a more specific value not found in the codelist."@en;
  rdfs:domain cdi:ControlledVocabularyEntry;
  rdfs:range xsd:string;
.

cdi:ControlledVocabularyEntry-vocabulary
  a rdf:Property, owl:ObjectProperty, ucmis:Attribute;
  rdfs:label "vocabulary";
  rdfs:comment "A reference to the external controlled vocabulary, using a URI or other resolvable identifier."@en;
  rdfs:domain cdi:ControlledVocabularyEntry;
  rdfs:range cdi:Reference;
.


# datatype CorrespondenceDefinition
# based on the UML data type DDICDIModels::DDICDILibrary::DataTypes::StructuredDataTypes::CorrespondenceDefinition
cdi:CorrespondenceDefinition
  a rdfs:Class, owl:Class, ucmis:StructuredDataType;
  rdfs:label "CorrespondenceDefinition";
  rdfs:comment "Definition\n============\nDescribes the commonalities and differences between two members using a textual description of both commonalities and differences plus an optional coding of the type of commonality."@en;
  
  owl:hasKey (cdi:CorrespondenceDefinition-commonality cdi:CorrespondenceDefinition-commonalityCode cdi:CorrespondenceDefinition-difference cdi:CorrespondenceDefinition-matching);
.

cdi:CorrespondenceDefinition-commonality
  a rdf:Property, owl:ObjectProperty, ucmis:Attribute;
  rdfs:label "commonality";
  rdfs:comment "A description of the common features of the two items. Supports multiple language versions of the same content as well as optional formatting of the content."@en;
  rdfs:domain cdi:CorrespondenceDefinition;
  rdfs:range cdi:InternationalString;
.

cdi:CorrespondenceDefinition-commonalityCode
  a rdf:Property, owl:ObjectProperty, ucmis:Attribute;
  rdfs:label "commonalityCode";
  rdfs:comment "Commonality expressed as a term or code. Supports the use of an external controlled vocabulary. If repeated, clarify each external controlled vocabulary used."@en;
  rdfs:domain cdi:CorrespondenceDefinition;
  rdfs:range cdi:ControlledVocabularyEntry;
.

cdi:CorrespondenceDefinition-difference
  a rdf:Property, owl:ObjectProperty, ucmis:Attribute;
  rdfs:label "difference";
  rdfs:comment "A description of the differences between the two items. Supports multiple language versions of the same content as well as optional formatting of the content."@en;
  rdfs:domain cdi:CorrespondenceDefinition;
  rdfs:range cdi:InternationalString;
.

cdi:CorrespondenceDefinition-matching
  a rdf:Property, owl:ObjectProperty, ucmis:Attribute;
  rdfs:label "matching";
  rdfs:comment "Allows specification of exact match, close match, or disjoint. These relationships can be further defined by describing commonalities or differences or providing additional controlled vocabulary descriptions of relationships."@en;
  rdfs:domain cdi:CorrespondenceDefinition;
  rdfs:range cdi:MatchingCriterion;
.


# datatype DateRange
# based on the UML data type DDICDIModels::DDICDILibrary::DataTypes::StructuredDataTypes::DateRange
cdi:DateRange
  a rdfs:Class, owl:Class, ucmis:StructuredDataType;
  rdfs:label "DateRange";
  rdfs:comment "Definition\n============\nExpresses a date/time range using a start date and end date (both with the structure of Date and supporting the use of ISO and non-ISO date structures). Use in all locations where a range of dates is required, i.e. validFor, embargoPeriod, collectionPeriod, etc."@en;
  
  owl:hasKey (cdi:DateRange-endDate cdi:DateRange-startDate);
.

cdi:DateRange-endDate
  a rdf:Property, owl:ObjectProperty, ucmis:Attribute;
  rdfs:label "endDate";
  rdfs:comment "The date (time) designating the end of the period or range."@en;
  rdfs:domain cdi:DateRange;
  rdfs:range cdi:CombinedDate;
.

cdi:DateRange-startDate
  a rdf:Property, owl:ObjectProperty, ucmis:Attribute;
  rdfs:label "startDate";
  rdfs:comment "The date (time) designating the beginning of the period or range."@en;
  rdfs:domain cdi:DateRange;
  rdfs:range cdi:CombinedDate;
.


# datatype ElectronicMessageSystem
# based on the UML data type DDICDIModels::DDICDILibrary::DataTypes::StructuredDataTypes::ElectronicMessageSystem
cdi:ElectronicMessageSystem
  a rdfs:Class, owl:Class, ucmis:StructuredDataType;
  rdfs:label "ElectronicMessageSystem";
  rdfs:comment "Definition\n============\nAny non-email means of relaying a message electronically. This would include text messaging, Skype, Twitter, ICQ, or other emerging means of electronic message conveyance. \n\nExamples\n==========\nSkype account, etc."@en;
  
  owl:hasKey (cdi:ElectronicMessageSystem-contactAddress cdi:ElectronicMessageSystem-effectiveDates cdi:ElectronicMessageSystem-isPreferred cdi:ElectronicMessageSystem-privacy cdi:ElectronicMessageSystem-typeOfService);
.

cdi:ElectronicMessageSystem-contactAddress
  a rdf:Property, owl:DatatypeProperty, ucmis:Attribute;
  rdfs:label "contactAddress";
  rdfs:comment "Account identification for contacting."@en;
  rdfs:domain cdi:ElectronicMessageSystem;
  rdfs:range xsd:string;
.

cdi:ElectronicMessageSystem-effectiveDates
  a rdf:Property, owl:ObjectProperty, ucmis:Attribute;
  rdfs:label "effectiveDates";
  rdfs:comment "Time period during which the account is valid."@en;
  rdfs:domain cdi:ElectronicMessageSystem;
  rdfs:range cdi:DateRange;
.

cdi:ElectronicMessageSystem-isPreferred
  a rdf:Property, owl:DatatypeProperty, ucmis:Attribute;
  rdfs:label "isPreferred";
  rdfs:comment "Set to True if this is the preferred address."@en;
  rdfs:domain cdi:ElectronicMessageSystem;
  rdfs:range xsd:boolean;
.

cdi:ElectronicMessageSystem-privacy
  a rdf:Property, owl:ObjectProperty, ucmis:Attribute;
  rdfs:label "privacy";
  rdfs:comment "Specify the level privacy for the address as public, restricted, or private. Supports the use of an external controlled vocabulary."@en;
  rdfs:domain cdi:ElectronicMessageSystem;
  rdfs:range cdi:ControlledVocabularyEntry;
.

cdi:ElectronicMessageSystem-typeOfService
  a rdf:Property, owl:ObjectProperty, ucmis:Attribute;
  rdfs:label "typeOfService";
  rdfs:comment "Indicates the type of service used. Supports the use of a controlled vocabulary."@en;
  rdfs:domain cdi:ElectronicMessageSystem;
  rdfs:range cdi:ControlledVocabularyEntry;
.


# datatype Email
# based on the UML data type DDICDIModels::DDICDILibrary::DataTypes::StructuredDataTypes::Email
cdi:Email
  a rdfs:Class, owl:Class, ucmis:StructuredDataType;
  rdfs:label "Email";
  rdfs:comment "Definition\n============\nAn e-mail address which conforms to the internet format (RFC 822) including its type and time period for which it is valid.\n\nExamples\n==========\ninfo@ddialliance.org; ex.ample@somewhere.org"@en;
  
  owl:hasKey (cdi:Email-effectiveDates cdi:Email-internetEmail cdi:Email-isPreferred cdi:Email-privacy cdi:Email-typeOfEmail);
.

cdi:Email-effectiveDates
  a rdf:Property, owl:ObjectProperty, ucmis:Attribute;
  rdfs:label "effectiveDates";
  rdfs:comment "Time period for which the e-mail address is valid."@en;
  rdfs:domain cdi:Email;
  rdfs:range cdi:DateRange;
.

cdi:Email-internetEmail
  a rdf:Property, owl:DatatypeProperty, ucmis:Attribute;
  rdfs:label "internetEmail";
  rdfs:comment "The email address expressed as a string (should follow the Internet format specification - RFC 5322) e.g. user@server.ext, more complex and flexible examples are also supported by the format."@en;
  rdfs:domain cdi:Email;
  rdfs:range xsd:string;
.

cdi:Email-isPreferred
  a rdf:Property, owl:DatatypeProperty, ucmis:Attribute;
  rdfs:label "isPreferred";
  rdfs:comment "Set to True if this is the preferred email."@en;
  rdfs:domain cdi:Email;
  rdfs:range xsd:boolean;
.

cdi:Email-privacy
  a rdf:Property, owl:ObjectProperty, ucmis:Attribute;
  rdfs:label "privacy";
  rdfs:comment "Indicates the level of privacy."@en;
  rdfs:domain cdi:Email;
  rdfs:range cdi:ControlledVocabularyEntry;
.

cdi:Email-typeOfEmail
  a rdf:Property, owl:ObjectProperty, ucmis:Attribute;
  rdfs:label "typeOfEmail";
  rdfs:comment "Code indicating the type of e-mail address. Supports the use of an external controlled vocabulary. (e.g. home, office)."@en;
  rdfs:domain cdi:Email;
  rdfs:range cdi:ControlledVocabularyEntry;
.


# datatype EmbargoInformation
# based on the UML data type DDICDIModels::DDICDILibrary::DataTypes::StructuredDataTypes::EmbargoInformation
cdi:EmbargoInformation
  a rdfs:Class, owl:Class, ucmis:StructuredDataType;
  rdfs:label "EmbargoInformation";
  rdfs:comment "Definition\n============\nSpecific information about any relevant embargo."@en;
  
  owl:hasKey (cdi:EmbargoInformation-description cdi:EmbargoInformation-period);
.

cdi:EmbargoInformation-description
  a rdf:Property, owl:ObjectProperty, ucmis:Attribute;
  rdfs:label "description";
  rdfs:comment "A text desription of the terms of an embarog on the object."@en;
  rdfs:domain cdi:EmbargoInformation;
  rdfs:range cdi:InternationalString;
.

cdi:EmbargoInformation-period
  a rdf:Property, owl:ObjectProperty, ucmis:Attribute;
  rdfs:label "period";
  rdfs:comment "The time range(s) for embargo of the object"@en;
  rdfs:domain cdi:EmbargoInformation;
  rdfs:range cdi:DateRange;
.


# datatype FundingInformation
# based on the UML data type DDICDIModels::DDICDILibrary::DataTypes::StructuredDataTypes::FundingInformation
cdi:FundingInformation
  a rdfs:Class, owl:Class, ucmis:StructuredDataType;
  rdfs:label "FundingInformation";
  rdfs:comment "Information regarding the source of funds used to develop or support the resource being described."@en;
  
  owl:hasKey (cdi:FundingInformation-fundingAgent cdi:FundingInformation-grantNumber);
.

cdi:FundingInformation-fundingAgent
  a rdf:Property, owl:ObjectProperty, ucmis:Attribute;
  rdfs:label "fundingAgent";
  rdfs:comment "A reference to the agent (e.g. organization) that provided funding for a grant."@en;
  rdfs:domain cdi:FundingInformation;
  rdfs:range cdi:AgentInRole;
.

cdi:FundingInformation-grantNumber
  a rdf:Property, owl:DatatypeProperty, ucmis:Attribute;
  rdfs:label "grantNumber";
  rdfs:comment "The identification number for the grant at least partly provided by the funding agent."@en;
  rdfs:domain cdi:FundingInformation;
  rdfs:range xsd:string;
.


# datatype GeoRole
# based on the UML data type DDICDIModels::DDICDILibrary::DataTypes::StructuredDataTypes::GeoRole
cdi:GeoRole
  a rdfs:Class, owl:Class, ucmis:StructuredDataType;
  rdfs:label "GeoRole";
  rdfs:comment "Definition\n============\nGeography-specific role given to a represented variable in the context of a data structure. The specific characterization of the role (e.g. reference, coordinates, etc.) may be given by a controlled vocabulary."@en;
  rdfs:subClassOf cdi:SpecializationRole;
  owl:hasKey (cdi:GeoRole-geography);
.

cdi:GeoRole-geography
  a rdf:Property, owl:ObjectProperty, ucmis:Attribute;
  rdfs:label "geography";
  rdfs:comment "Function in relation to the specification of a place or physical area or feature, ideally drawn from a controlled vocabulary."@en;
  rdfs:domain cdi:GeoRole;
  rdfs:range cdi:ControlledVocabularyEntry;
.


# datatype Identifier
# based on the UML data type DDICDIModels::DDICDILibrary::DataTypes::StructuredDataTypes::Identifier
cdi:Identifier
  a rdfs:Class, owl:Class, ucmis:StructuredDataType;
  rdfs:label "Identifier";
  rdfs:comment "Definition\n============\nIdentifier for objects requiring short- or long-lasting referencing and management."@en;
  
  owl:hasKey (cdi:Identifier-ddiIdentifier cdi:Identifier-isDdiIdentifierPersistent cdi:Identifier-isDdiIdentifierUniversallyUnique cdi:Identifier-nonDdiIdentifier cdi:Identifier-uri cdi:Identifier-versionDate cdi:Identifier-versionRationale cdi:Identifier-versionResponsibility);
.

cdi:Identifier-ddiIdentifier
  a rdf:Property, owl:ObjectProperty, ucmis:Attribute;
  rdfs:label "ddiIdentifier";
  rdfs:comment "A globally unique identifier. The values of the three attributes can be used to create a DDI URN."@en;
  rdfs:domain cdi:Identifier;
  rdfs:range cdi:InternationalRegistrationDataIdentifier;
.

cdi:Identifier-isDdiIdentifierPersistent
  a rdf:Property, owl:DatatypeProperty, ucmis:Attribute;
  rdfs:label "isDdiIdentifierPersistent";
  rdfs:comment "Default value is False indicating that the content of the current version may change (may be in development mode). Set to True when the content of this version will no longer change."@en;
  rdfs:domain cdi:Identifier;
  rdfs:range xsd:boolean;
.

cdi:Identifier-isDdiIdentifierUniversallyUnique
  a rdf:Property, owl:DatatypeProperty, ucmis:Attribute;
  rdfs:label "isDdiIdentifierUniversallyUnique";
  rdfs:comment "Default value is False. If the id of the object was created as a Universally Unique ID (UUID) set to True."@en;
  rdfs:domain cdi:Identifier;
  rdfs:range xsd:boolean;
.

cdi:Identifier-nonDdiIdentifier
  a rdf:Property, owl:ObjectProperty, ucmis:Attribute;
  rdfs:label "nonDdiIdentifier";
  rdfs:comment "Any identifier other than a DDI identifier."@en;
  rdfs:domain cdi:Identifier;
  rdfs:range cdi:NonDdiIdentifier;
.

cdi:Identifier-uri
  a rdf:Property, owl:DatatypeProperty, ucmis:Attribute;
  rdfs:label "uri";
  rdfs:comment "A Universal Resource Identifier, valid according to the W3C XML Schema specification."@en;
  rdfs:domain cdi:Identifier;
  rdfs:range xsd:anyURI;
.

cdi:Identifier-versionDate
  a rdf:Property, owl:DatatypeProperty, ucmis:Attribute;
  rdfs:label "versionDate";
  rdfs:comment "Date and time the object was changed expressed in standard ISO formats."@en;
  rdfs:domain cdi:Identifier;
  rdfs:range xsd:date;
.

cdi:Identifier-versionRationale
  a rdf:Property, owl:ObjectProperty, ucmis:Attribute;
  rdfs:label "versionRationale";
  rdfs:comment "Reason for making a new version of the object."@en;
  rdfs:domain cdi:Identifier;
  rdfs:range cdi:RationaleDefinition;
.

cdi:Identifier-versionResponsibility
  a rdf:Property, owl:ObjectProperty, ucmis:Attribute;
  rdfs:label "versionResponsibility";
  rdfs:comment "Contributor who has the ownership and responsibility for the current version."@en;
  rdfs:domain cdi:Identifier;
  rdfs:range cdi:AgentInRole;
.


# datatype IndividualName
# based on the UML data type DDICDIModels::DDICDILibrary::DataTypes::StructuredDataTypes::IndividualName
cdi:IndividualName
  a rdfs:Class, owl:Class, ucmis:StructuredDataType;
  rdfs:label "IndividualName";
  rdfs:comment "Definition\n============\nThe name of an individual broken out into its component parts of prefix, first/given name, middle name, last/family/surname, and suffix. The preferred compilation of the name parts may also be provided. The legal or formal name of the individual should have the isFormal attribute set to true. The preferred name should be noted with the isPreferred attribute. The attribute sex provides information to assist in the appropriate use of pronouns."@en;
  
  owl:hasKey (cdi:IndividualName-abbreviation cdi:IndividualName-context cdi:IndividualName-effectiveDates cdi:IndividualName-firstGiven cdi:IndividualName-fullName cdi:IndividualName-isFormal cdi:IndividualName-isPreferred cdi:IndividualName-lastFamily cdi:IndividualName-middle cdi:IndividualName-prefix cdi:IndividualName-sex cdi:IndividualName-suffix cdi:IndividualName-typeOfIndividualName);
.

cdi:IndividualName-abbreviation
  a rdf:Property, owl:ObjectProperty, ucmis:Attribute;
  rdfs:label "abbreviation";
  rdfs:comment "An abbreviation or acronym for the name. This may be expressed in multiple languages. It is assumed that if only a single language is provided that it may be used in any of the other languages within which the name itself is expressed."@en;
  rdfs:domain cdi:IndividualName;
  rdfs:range cdi:InternationalString;
.

cdi:IndividualName-context
  a rdf:Property, owl:ObjectProperty, ucmis:Attribute;
  rdfs:label "context";
  rdfs:comment "A name may be specific to a particular context, i.e. common usage, business, social, etc.. Identify the context related to the specified name. Supports the use of an external controlled vocabulary."@en;
  rdfs:domain cdi:IndividualName;
  rdfs:range cdi:ControlledVocabularyEntry;
.

cdi:IndividualName-effectiveDates
  a rdf:Property, owl:ObjectProperty, ucmis:Attribute;
  rdfs:label "effectiveDates";
  rdfs:comment "Clarifies when the name information is accurate."@en;
  rdfs:domain cdi:IndividualName;
  rdfs:range cdi:DateRange;
.

cdi:IndividualName-firstGiven
  a rdf:Property, owl:DatatypeProperty, ucmis:Attribute;
  rdfs:label "firstGiven";
  rdfs:comment "First (given) name of the individual."@en;
  rdfs:domain cdi:IndividualName;
  rdfs:range xsd:string;
.

cdi:IndividualName-fullName
  a rdf:Property, owl:ObjectProperty, ucmis:Attribute;
  rdfs:label "fullName";
  rdfs:comment "This provides a means of providing a full name as a single object for display or print such as identification badges etc. For example a person with the name of William Grace for official use may prefer a display name of Bill Grace on a name tag or other informal publication."@en;
  rdfs:domain cdi:IndividualName;
  rdfs:range cdi:InternationalString;
.

cdi:IndividualName-isFormal
  a rdf:Property, owl:DatatypeProperty, ucmis:Attribute;
  rdfs:label "isFormal";
  rdfs:comment "The legal or formal name of the individual should have the isFormal attribute set to True. To avoid confusion only one individual name should have the isFormal attribute set to True. Use the TypeOfIndividualName to further differentiate the type and applied usage when multiple names are provided."@en;
  rdfs:domain cdi:IndividualName;
  rdfs:range xsd:boolean;
.

cdi:IndividualName-isPreferred
  a rdf:Property, owl:DatatypeProperty, ucmis:Attribute;
  rdfs:label "isPreferred";
  rdfs:comment "If more than one name for the object is provided, use the isPreferred attribute to indicate which is the preferred name content. All other names should be set to isPreferred=False."@en;
  rdfs:domain cdi:IndividualName;
  rdfs:range xsd:boolean;
.

cdi:IndividualName-lastFamily
  a rdf:Property, owl:DatatypeProperty, ucmis:Attribute;
  rdfs:label "lastFamily";
  rdfs:comment "Last (family) name /surname of the individual."@en;
  rdfs:domain cdi:IndividualName;
  rdfs:range xsd:string;
.

cdi:IndividualName-middle
  a rdf:Property, owl:DatatypeProperty, ucmis:Attribute;
  rdfs:label "middle";
  rdfs:comment "Middle name or initial of the individual."@en;
  rdfs:domain cdi:IndividualName;
  rdfs:range xsd:string;
.

cdi:IndividualName-prefix
  a rdf:Property, owl:DatatypeProperty, ucmis:Attribute;
  rdfs:label "prefix";
  rdfs:comment "Title that precedes the name of the individual, such as Ms., or Dr."@en;
  rdfs:domain cdi:IndividualName;
  rdfs:range xsd:string;
.

cdi:IndividualName-sex
  a rdf:Property, owl:ObjectProperty, ucmis:Attribute;
  rdfs:label "sex";
  rdfs:comment "Sex allows for the specification of male, female or neutral. The purpose of providing this information is to assist others in the appropriate use of pronouns when addressing the individual. Note that many countries/languages may offer a neutral pronoun form."@en;
  rdfs:domain cdi:IndividualName;
  rdfs:range cdi:SexSpecification;
.

cdi:IndividualName-suffix
  a rdf:Property, owl:DatatypeProperty, ucmis:Attribute;
  rdfs:label "suffix";
  rdfs:comment "Title that follows the name of the individual, such as Esq. (abbreviation for Esquire. This is usually a courtesy title)."@en;
  rdfs:domain cdi:IndividualName;
  rdfs:range xsd:string;
.

cdi:IndividualName-typeOfIndividualName
  a rdf:Property, owl:ObjectProperty, ucmis:Attribute;
  rdfs:label "typeOfIndividualName";
  rdfs:comment "The type of individual name provided. the use of a controlled vocabulary is strongly recommended. At minimum his should include, e.g. PreviousFormalName, Nickname (or CommonName), Other."@en;
  rdfs:domain cdi:IndividualName;
  rdfs:range cdi:ControlledVocabularyEntry;
.


# datatype InternationalIdentifier
# based on the UML data type DDICDIModels::DDICDILibrary::DataTypes::StructuredDataTypes::InternationalIdentifier
cdi:InternationalIdentifier
  a rdfs:Class, owl:Class, ucmis:StructuredDataType;
  rdfs:label "InternationalIdentifier";
  rdfs:comment "Definition\n============\nAn identifier whose scope of uniqueness is broader than the local archive. Common forms of an international identifier are ISBN, ISSN, DOI or similar designator. Provides both the value of the identifier and the agency who manages it.\n\nExplanatory notes\n===================\nFor use in annotation or other citation format."@en;
  
  owl:hasKey (cdi:InternationalIdentifier-identifierContent cdi:InternationalIdentifier-isURI cdi:InternationalIdentifier-managingAgency);
.

cdi:InternationalIdentifier-identifierContent
  a rdf:Property, owl:DatatypeProperty, ucmis:Attribute;
  rdfs:label "identifierContent";
  rdfs:comment "An identifier as it should be listed for identification purposes."@en;
  rdfs:domain cdi:InternationalIdentifier;
  rdfs:range xsd:string;
.

cdi:InternationalIdentifier-isURI
  a rdf:Property, owl:DatatypeProperty, ucmis:Attribute;
  rdfs:label "isURI";
  rdfs:comment "Set to True if Identifier is a URI."@en;
  rdfs:domain cdi:InternationalIdentifier;
  rdfs:range xsd:boolean;
.

cdi:InternationalIdentifier-managingAgency
  a rdf:Property, owl:ObjectProperty, ucmis:Attribute;
  rdfs:label "managingAgency";
  rdfs:comment "The identification of the Agency which assigns and manages the identifier, i.e., ISBN, ISSN, DOI, etc."@en;
  rdfs:domain cdi:InternationalIdentifier;
  rdfs:range cdi:ControlledVocabularyEntry;
.


# datatype InternationalRegistrationDataIdentifier
# based on the UML data type DDICDIModels::DDICDILibrary::DataTypes::StructuredDataTypes::InternationalRegistrationDataIdentifier
cdi:InternationalRegistrationDataIdentifier
  a rdfs:Class, owl:Class, ucmis:StructuredDataType;
  rdfs:label "InternationalRegistrationDataIdentifier";
  rdfs:comment "Definition\n==========\nPersistent, globally unique object identifier aligned with ISO/IEC 11179-6:2015, Information technology - Metadata registries (MDR) - Part 6: Registration, Annex A, Identifiers based on ISO/IEC 6523, http://standards.iso.org/ittf/PubliclyAvailableStandards/c060342_ISO_IEC_11179-6_2015.zip.\nThe uniqueness of an InternationalRegistrationDataIdentifier (IRDI) is determined by the combination of the values of three identifying attributes."@en;
  
  owl:hasKey (cdi:InternationalRegistrationDataIdentifier-dataIdentifier cdi:InternationalRegistrationDataIdentifier-registrationAuthorityIdentifier cdi:InternationalRegistrationDataIdentifier-versionIdentifier);
.

cdi:InternationalRegistrationDataIdentifier-dataIdentifier
  a rdf:Property, owl:DatatypeProperty, ucmis:Attribute;
  rdfs:label "dataIdentifier";
  rdfs:comment "Identifier assigned to an Administered Item within a Registration Authority, hereafter called Data Identifier (DI). The DI is called 'id' in DDI-Codebook and DDI-Lifecycle."@en;
  rdfs:domain cdi:InternationalRegistrationDataIdentifier;
  rdfs:range xsd:string;
.

cdi:InternationalRegistrationDataIdentifier-registrationAuthorityIdentifier
  a rdf:Property, owl:DatatypeProperty, ucmis:Attribute;
  rdfs:label "registrationAuthorityIdentifier";
  rdfs:comment "Identifier assigned to a Registration Authority, hereafter called Registration Authority Identifier (RAI). The RAI is called 'agency' in DDI-Codebook and DDI-Lifecycle."@en;
  rdfs:domain cdi:InternationalRegistrationDataIdentifier;
  rdfs:range xsd:string;
.

cdi:InternationalRegistrationDataIdentifier-versionIdentifier
  a rdf:Property, owl:DatatypeProperty, ucmis:Attribute;
  rdfs:label "versionIdentifier";
  rdfs:comment "Identifier assigned to a version under which an Administered Item registration is submitted or updated hereafter called Version Identifier (VI). The VI is called \"version\" in DDI-Codebook and DDI-Lifecycle."@en;
  rdfs:domain cdi:InternationalRegistrationDataIdentifier;
  rdfs:range xsd:string;
.


# datatype InternationalString
# based on the UML data type DDICDIModels::DDICDILibrary::DataTypes::StructuredDataTypes::InternationalString
cdi:InternationalString
  a rdfs:Class, owl:Class, ucmis:StructuredDataType;
  rdfs:label "InternationalString";
  rdfs:comment "Definition\n============\nPackaging structure for multiple language versions of the same string content. Where an element of this type is repeatable, the expectation is that each repetition contains different content, each of which can be expressed in multiple languages. The language designation goes on the individual String."@en;
  
  owl:hasKey (cdi:InternationalString-languageSpecificString);
.

cdi:InternationalString-languageSpecificString
  a rdf:Property, owl:ObjectProperty, ucmis:Attribute;
  rdfs:label "languageSpecificString";
  rdfs:comment "A non-formatted string of text with an attribute that designates the language of the text. Repeat this object to express the same content in another language."@en;
  rdfs:domain cdi:InternationalString;
  rdfs:range cdi:ComplexLanguageString;
.


# datatype LabelForDisplay
# based on the UML data type DDICDIModels::DDICDILibrary::DataTypes::StructuredDataTypes::LabelForDisplay
cdi:LabelForDisplay
  a rdfs:Class, owl:Class, ucmis:StructuredDataType;
  rdfs:label "LabelForDisplay";
  rdfs:comment "Definition\n============\nA structured display label. Label provides display content of a fully human readable display for the identification of the object."@en;
  rdfs:subClassOf cdi:InternationalString;
  owl:hasKey (cdi:LabelForDisplay-locationVariant cdi:LabelForDisplay-maxLength cdi:LabelForDisplay-validDates);
.

cdi:LabelForDisplay-locationVariant
  a rdf:Property, owl:ObjectProperty, ucmis:Attribute;
  rdfs:label "locationVariant";
  rdfs:comment "Indicate the locality specification for content that is specific to a geographic area. May be a country code, sub-country code, or area name."@en;
  rdfs:domain cdi:LabelForDisplay;
  rdfs:range cdi:ControlledVocabularyEntry;
.

cdi:LabelForDisplay-maxLength
  a rdf:Property, owl:DatatypeProperty, ucmis:Attribute;
  rdfs:label "maxLength";
  rdfs:comment "A positive integer indicating the maximum number of characters in the label."@en;
  rdfs:domain cdi:LabelForDisplay;
  rdfs:range xsd:integer;
.

cdi:LabelForDisplay-validDates
  a rdf:Property, owl:ObjectProperty, ucmis:Attribute;
  rdfs:label "validDates";
  rdfs:comment "Allows for the specification of a starting date and ending date for the period that this label is valid."@en;
  rdfs:domain cdi:LabelForDisplay;
  rdfs:range cdi:DateRange;
.


# datatype LanguageSpecificString
# based on the UML data type DDICDIModels::DDICDILibrary::DataTypes::StructuredDataTypes::LanguageSpecificString
cdi:LanguageSpecificString
  a rdfs:Class, owl:Class, ucmis:StructuredDataType;
  rdfs:label "LanguageSpecificString";
  rdfs:comment "Definition\n============\nAllows for non-formatted language specific strings that may be translations from other languages, or that may be translatable into other languages. Only one string per language/scope type is allowed. language specific string contains the following attributes, xmlang to designate the language, isTranslated with a default value of false to designate if an object is a translation of another language, isTranslatable with a default value of true to designate if the content can be translated, translationSourceLanguage to indicate the source languages used in creating this translation, translationDate, and scope which can be used to define intended audience or use such as internal, external, etc."@en;
  
  owl:hasKey (cdi:LanguageSpecificString-content cdi:LanguageSpecificString-isTranslatable cdi:LanguageSpecificString-isTranslated cdi:LanguageSpecificString-language cdi:LanguageSpecificString-scope cdi:LanguageSpecificString-structureUsed cdi:LanguageSpecificString-translationDate cdi:LanguageSpecificString-translationSourceLanguage);
.

cdi:LanguageSpecificString-content
  a rdf:Property, owl:DatatypeProperty, ucmis:Attribute;
  rdfs:label "content";
  rdfs:comment "Value of this string."@en;
  rdfs:domain cdi:LanguageSpecificString;
  rdfs:range xsd:string;
.

cdi:LanguageSpecificString-isTranslatable
  a rdf:Property, owl:DatatypeProperty, ucmis:Attribute;
  rdfs:label "isTranslatable";
  rdfs:comment "Indicates whether content is translatable (True) or not (False). An example of something that is not translatable would be a MNEMONIC of an object or a number."@en;
  rdfs:domain cdi:LanguageSpecificString;
  rdfs:range xsd:boolean;
.

cdi:LanguageSpecificString-isTranslated
  a rdf:Property, owl:DatatypeProperty, ucmis:Attribute;
  rdfs:label "isTranslated";
  rdfs:comment "Indicates whether content is a translation (True) or an original (False)."@en;
  rdfs:domain cdi:LanguageSpecificString;
  rdfs:range xsd:boolean;
.

cdi:LanguageSpecificString-language
  a rdf:Property, owl:DatatypeProperty, ucmis:Attribute;
  rdfs:label "language";
  rdfs:comment "Indicates the language of content. Note that language allows for a simple 2 or 3 character language code or a language code extended by a country code , for example en-au for English as used in Australia."@en;
  rdfs:domain cdi:LanguageSpecificString;
  rdfs:range xsd:language;
.

cdi:LanguageSpecificString-scope
  a rdf:Property, owl:DatatypeProperty, ucmis:Attribute;
  rdfs:label "scope";
  rdfs:comment "Supports specification of scope for the contained content. Use with the language specification to filter application of content."@en;
  rdfs:domain cdi:LanguageSpecificString;
  rdfs:range xsd:string;
.

cdi:LanguageSpecificString-structureUsed
  a rdf:Property, owl:ObjectProperty, ucmis:Attribute;
  rdfs:label "structureUsed";
  rdfs:comment "The structure type used. Examples are HTML or restructured text."@en;
  rdfs:domain cdi:LanguageSpecificString;
  rdfs:range cdi:ControlledVocabularyEntry;
.

cdi:LanguageSpecificString-translationDate
  a rdf:Property, owl:DatatypeProperty, ucmis:Attribute;
  rdfs:label "translationDate";
  rdfs:comment "The date the content was translated. Provision of translation date allows user to verify if translation was available during data collection or other time linked activity."@en;
  rdfs:domain cdi:LanguageSpecificString;
  rdfs:range xsd:date;
.

cdi:LanguageSpecificString-translationSourceLanguage
  a rdf:Property, owl:DatatypeProperty, ucmis:Attribute;
  rdfs:label "translationSourceLanguage";
  rdfs:comment "List the language code of the source. Repeat of multiple language sources are used."@en;
  rdfs:domain cdi:LanguageSpecificString;
  rdfs:range xsd:language;
.


# datatype LicenseInformation
# based on the UML data type DDICDIModels::DDICDILibrary::DataTypes::StructuredDataTypes::LicenseInformation
cdi:LicenseInformation
  a rdfs:Class, owl:Class, ucmis:StructuredDataType;
  rdfs:label "LicenseInformation";
  rdfs:comment "Definition\n============\nInformation about any relevant license.\n\nExamples\n==========\nLicensed under Creative Commons Attribution 2.0 Generic (CC BY 2.0)."@en;
  
  owl:hasKey (cdi:LicenseInformation-contact cdi:LicenseInformation-description cdi:LicenseInformation-licenseAgent cdi:LicenseInformation-licenseReference);
.

cdi:LicenseInformation-contact
  a rdf:Property, owl:ObjectProperty, ucmis:Attribute;
  rdfs:label "contact";
  rdfs:comment "Information on whom to contact for details on licensing."@en;
  rdfs:domain cdi:LicenseInformation;
  rdfs:range cdi:ContactInformation;
.

cdi:LicenseInformation-description
  a rdf:Property, owl:ObjectProperty, ucmis:Attribute;
  rdfs:label "description";
  rdfs:comment "A description of licensing terms."@en;
  rdfs:domain cdi:LicenseInformation;
  rdfs:range cdi:InternationalString;
.

cdi:LicenseInformation-licenseAgent
  a rdf:Property, owl:ObjectProperty, ucmis:Attribute;
  rdfs:label "licenseAgent";
  rdfs:comment "Points to a description of an agent with information about, or responsible for licensing of the object."@en;
  rdfs:domain cdi:LicenseInformation;
  rdfs:range cdi:AgentInRole;
.

cdi:LicenseInformation-licenseReference
  a rdf:Property, owl:ObjectProperty, ucmis:Attribute;
  rdfs:label "licenseReference";
  rdfs:comment "Points to published license terms, such as to a specific Creative Commons license."@en;
  rdfs:domain cdi:LicenseInformation;
  rdfs:range cdi:Reference;
.


# datatype NonDdiIdentifier
# based on the UML data type DDICDIModels::DDICDILibrary::DataTypes::StructuredDataTypes::NonDdiIdentifier
cdi:NonDdiIdentifier
  a rdfs:Class, owl:Class, ucmis:StructuredDataType;
  rdfs:label "NonDdiIdentifier";
  rdfs:comment "Definition\n============\nA unique set of attributes, not conforming to the DDI identifier structure nor structured as a URI, used to identify some entity."@en;
  
  owl:hasKey (cdi:NonDdiIdentifier-managingAgency cdi:NonDdiIdentifier-type cdi:NonDdiIdentifier-value cdi:NonDdiIdentifier-version);
.

cdi:NonDdiIdentifier-managingAgency
  a rdf:Property, owl:DatatypeProperty, ucmis:Attribute;
  rdfs:label "managingAgency";
  rdfs:comment "The authority which maintains the identification scheme."@en;
  rdfs:domain cdi:NonDdiIdentifier;
  rdfs:range xsd:string;
.

cdi:NonDdiIdentifier-type
  a rdf:Property, owl:DatatypeProperty, ucmis:Attribute;
  rdfs:label "type";
  rdfs:comment "The scheme of identifier, as distinct from a URI or a DDI-conforming identifier."@en;
  rdfs:domain cdi:NonDdiIdentifier;
  rdfs:range xsd:string;
.

cdi:NonDdiIdentifier-value
  a rdf:Property, owl:DatatypeProperty, ucmis:Attribute;
  rdfs:label "value";
  rdfs:comment "The identifier, structured according to the specified type."@en;
  rdfs:domain cdi:NonDdiIdentifier;
  rdfs:range xsd:string;
.

cdi:NonDdiIdentifier-version
  a rdf:Property, owl:DatatypeProperty, ucmis:Attribute;
  rdfs:label "version";
  rdfs:comment "The version of the object being identified, according to the versioning system provided by the identified scheme."@en;
  rdfs:domain cdi:NonDdiIdentifier;
  rdfs:range xsd:string;
.


# datatype NonIsoDate
# based on the UML data type DDICDIModels::DDICDILibrary::DataTypes::StructuredDataTypes::NonIsoDate
cdi:NonIsoDate
  a rdfs:Class, owl:Class, ucmis:StructuredDataType;
  rdfs:label "NonIsoDate";
  rdfs:comment "Definition\n============\nUsed to preserve an historical date, formatted in a non-ISO fashion."@en;
  
  owl:hasKey (cdi:NonIsoDate-calendar cdi:NonIsoDate-dateContent cdi:NonIsoDate-nonIsoDateFormat);
.

cdi:NonIsoDate-calendar
  a rdf:Property, owl:ObjectProperty, ucmis:Attribute;
  rdfs:label "calendar";
  rdfs:comment "Specifies the type of calendar used (e.g., Gregorian, Julian, Jewish)."@en;
  rdfs:domain cdi:NonIsoDate;
  rdfs:range cdi:ControlledVocabularyEntry;
.

cdi:NonIsoDate-dateContent
  a rdf:Property, owl:DatatypeProperty, ucmis:Attribute;
  rdfs:label "dateContent";
  rdfs:comment "This is the date expressed in a non-ISO compliant structure. Primarily used to retain legacy content or to express non-Gregorian calendar dates."@en;
  rdfs:domain cdi:NonIsoDate;
  rdfs:range xsd:string;
.

cdi:NonIsoDate-nonIsoDateFormat
  a rdf:Property, owl:ObjectProperty, ucmis:Attribute;
  rdfs:label "nonIsoDateFormat";
  rdfs:comment "Indicate the structure of the date provided in NonISODate. For example if the NonISODate contained 4/1/2000 the Historical Date Format would be mm/dd/yyyy. The use of a controlled vocabulary is strongly recommended to support interoperability."@en;
  rdfs:domain cdi:NonIsoDate;
  rdfs:range cdi:ControlledVocabularyEntry;
.


# datatype ObjectAttributeSelector
# based on the UML data type DDICDIModels::DDICDILibrary::DataTypes::StructuredDataTypes::ObjectAttributeSelector
cdi:ObjectAttributeSelector
  a rdfs:Class, owl:Class, ucmis:StructuredDataType;
  rdfs:label "ObjectAttributeSelector";
  rdfs:comment "Definition\n==========\nA resource which describes a specific attribute of an object. It is defined in the style of selectors of the Web Annotation Vocabulary, see https://www.w3.org/TR/annotation-vocab/. The selector can be nested dependent on the structure of the referenced object."@en;
  rdfs:subClassOf cdi:Selector;
  owl:hasKey (cdi:ObjectAttributeSelector-refinedBy cdi:ObjectAttributeSelector-refinedByOrderNumber cdi:ObjectAttributeSelector-value);
.

cdi:ObjectAttributeSelector-refinedBy
  a rdf:Property, owl:ObjectProperty, ucmis:Attribute;
  rdfs:label "refinedBy";
  rdfs:comment "Nested object attribute selector."@en;
  rdfs:domain cdi:ObjectAttributeSelector;
  rdfs:range cdi:ObjectAttributeSelector;
.

cdi:ObjectAttributeSelector-refinedByOrderNumber
  a rdf:Property, owl:DatatypeProperty, ucmis:Attribute;
  rdfs:label "refinedByOrderNumber";
  rdfs:comment "Order number of the specific attribute."@en;
  rdfs:domain cdi:ObjectAttributeSelector;
  rdfs:range xsd:integer;
.

cdi:ObjectAttributeSelector-value
  a rdf:Property, owl:DatatypeProperty, ucmis:Attribute;
  rdfs:label "value";
  rdfs:comment "Name of the attribute."@en;
  rdfs:domain cdi:ObjectAttributeSelector;
  rdfs:range xsd:string;
.


# datatype ObjectName
# based on the UML data type DDICDIModels::DDICDILibrary::DataTypes::StructuredDataTypes::ObjectName
cdi:ObjectName
  a rdfs:Class, owl:Class, ucmis:StructuredDataType;
  rdfs:label "ObjectName";
  rdfs:comment "Definition\n==========\nA standard means of expressing a name for a class object. A linguistic signifier. Human understandable name (word, phrase, or mnemonic) that reflects the ISO/IEC 11179-5 naming principles.\n\nExplanatory notes\n=================\nUse in model: In general the property name should be \"name\" as it is the name of the class object of which it is an attribute. Use a specific name (i.e. xxxName) only when naming something other than the class object of which it is an attribute."@en;
  
  owl:hasKey (cdi:ObjectName-context cdi:ObjectName-name);
.

cdi:ObjectName-context
  a rdf:Property, owl:ObjectProperty, ucmis:Attribute;
  rdfs:label "context";
  rdfs:comment "A name may be specific to a particular context, i.e., a type of software, or a section of a registry. Identify the context related to the specified name."@en;
  rdfs:domain cdi:ObjectName;
  rdfs:range cdi:ControlledVocabularyEntry;
.

cdi:ObjectName-name
  a rdf:Property, owl:DatatypeProperty, ucmis:Attribute;
  rdfs:label "name";
  rdfs:comment "The expressed name of the object."@en;
  rdfs:domain cdi:ObjectName;
  rdfs:range xsd:string;
.


# datatype OrganizationName
# based on the UML data type DDICDIModels::DDICDILibrary::DataTypes::StructuredDataTypes::OrganizationName
cdi:OrganizationName
  a rdfs:Class, owl:Class, ucmis:StructuredDataType;
  rdfs:label "OrganizationName";
  rdfs:comment "Definition\n==========\nNames by which the organization is known. Use the attribute isFormal with a value of True to designate the legal or formal name of the organization. Names may be typed with typeOfOrganizationName to indicate their appropriate usage."@en;
  rdfs:subClassOf cdi:ObjectName;
  owl:hasKey (cdi:OrganizationName-abbreviation cdi:OrganizationName-effectiveDates cdi:OrganizationName-isFormal cdi:OrganizationName-typeOfOrganizationName);
.

cdi:OrganizationName-abbreviation
  a rdf:Property, owl:ObjectProperty, ucmis:Attribute;
  rdfs:label "abbreviation";
  rdfs:comment "An abbreviation or acronym for the name. This may be expressed in multiple languages. It is assumed that if only a single language is provided that it may be used in any of the other languages within which the name itself is expressed."@en;
  rdfs:domain cdi:OrganizationName;
  rdfs:range cdi:InternationalString;
.

cdi:OrganizationName-effectiveDates
  a rdf:Property, owl:ObjectProperty, ucmis:Attribute;
  rdfs:label "effectiveDates";
  rdfs:comment "The time period for which this name is accurate and in use."@en;
  rdfs:domain cdi:OrganizationName;
  rdfs:range cdi:DateRange;
.

cdi:OrganizationName-isFormal
  a rdf:Property, owl:DatatypeProperty, ucmis:Attribute;
  rdfs:label "isFormal";
  rdfs:comment "The legal or formal name of the organization should have the isFormal attribute set to True. To avoid confusion only one organization name should have the isFormal attribute set to True. Use the typeOfOrganizationName to further differentiate the type and applied usage when multiple names are provided."@en;
  rdfs:domain cdi:OrganizationName;
  rdfs:range xsd:boolean;
.

cdi:OrganizationName-typeOfOrganizationName
  a rdf:Property, owl:ObjectProperty, ucmis:Attribute;
  rdfs:label "typeOfOrganizationName";
  rdfs:comment "The type of organization name provided. the use of a controlled vocabulary is strongly recommended. At minimum this should include, e.g. PreviousFormalName, Nickname (or CommonName), Other."@en;
  rdfs:domain cdi:OrganizationName;
  rdfs:range cdi:ControlledVocabularyEntry;
.


# datatype PairedControlledVocabularyEntry
# based on the UML data type DDICDIModels::DDICDILibrary::DataTypes::StructuredDataTypes::PairedControlledVocabularyEntry
cdi:PairedControlledVocabularyEntry
  a rdfs:Class, owl:Class, ucmis:StructuredDataType;
  rdfs:label "PairedControlledVocabularyEntry";
  rdfs:comment "Definition\n==========\nA tightly bound pair of items from an external controlled vocabulary. The extent property describes the extent to which the parent term applies for the specific case.\n\nExamples\n========\nWhen used to assign a role to an actor within a specific activity this term would express the degree of contribution. Contributor with term (role) \"Editor\" and extent \"Lead\".\n\nAlternatively the term might be a controlled vocabulary from a list of controlled vocabularies, e.g. the Generic Longitudinal Business Process Model (GLBPM) in a list that could include other business process model frameworks. In this context the extent becomes the name of a business process model task, e.g. \"integrate data\" from the GLBPM."@en;
  
  owl:hasKey (cdi:PairedControlledVocabularyEntry-extent cdi:PairedControlledVocabularyEntry-term);
.

cdi:PairedControlledVocabularyEntry-extent
  a rdf:Property, owl:ObjectProperty, ucmis:Attribute;
  rdfs:label "extent";
  rdfs:comment "Describes the extent to which the parent term applies for the specific case using an external controlled vocabulary. When associated with a role from the CASRAI Contributor Roles Taxonomy an appropriate vocabulary should be specified as either \"lead\", \"equal\", or \"supporting\"."@en;
  rdfs:domain cdi:PairedControlledVocabularyEntry;
  rdfs:range cdi:ControlledVocabularyEntry;
.

cdi:PairedControlledVocabularyEntry-term
  a rdf:Property, owl:ObjectProperty, ucmis:Attribute;
  rdfs:label "term";
  rdfs:comment "The term attributed to the parent class, for example the role of a contributor."@en;
  rdfs:domain cdi:PairedControlledVocabularyEntry;
  rdfs:range cdi:ControlledVocabularyEntry;
.


# datatype PrivateImage
# based on the UML data type DDICDIModels::DDICDILibrary::DataTypes::StructuredDataTypes::PrivateImage
cdi:PrivateImage
  a rdfs:Class, owl:Class, ucmis:StructuredDataType;
  rdfs:label "PrivateImage";
  rdfs:comment "Definition\n============\nReferences an image using the standard Image description. In addition to the standard attributes provides an effective date (period) and a privacy ranking."@en;
  
  owl:hasKey (cdi:PrivateImage-effectiveDates cdi:PrivateImage-privacy);
.

cdi:PrivateImage-effectiveDates
  a rdf:Property, owl:ObjectProperty, ucmis:Attribute;
  rdfs:label "effectiveDates";
  rdfs:comment "The period for which this image is effective/valid."@en;
  rdfs:domain cdi:PrivateImage;
  rdfs:range cdi:DateRange;
.

cdi:PrivateImage-privacy
  a rdf:Property, owl:ObjectProperty, ucmis:Attribute;
  rdfs:label "privacy";
  rdfs:comment "Specify the level privacy for the image as public, restricted, or private. Supports the use of an external controlled vocabulary."@en;
  rdfs:domain cdi:PrivateImage;
  rdfs:range cdi:ControlledVocabularyEntry;
.


# datatype ProvenanceInformation
# based on the UML data type DDICDIModels::DDICDILibrary::DataTypes::StructuredDataTypes::ProvenanceInformation
cdi:ProvenanceInformation
  a rdfs:Class, owl:Class, ucmis:StructuredDataType;
  rdfs:label "ProvenanceInformation";
  rdfs:comment "Definition\n============\nBasic information about the provenance of the object. Includes a simple description, but not detailed modeling of a process."@en;
  
  owl:hasKey (cdi:ProvenanceInformation-funding cdi:ProvenanceInformation-provenanceStatement cdi:ProvenanceInformation-recordCreationDate cdi:ProvenanceInformation-recordLastRevisionDate);
.

cdi:ProvenanceInformation-funding
  a rdf:Property, owl:ObjectProperty, ucmis:Attribute;
  rdfs:label "funding";
  rdfs:comment "Information about a funding source."@en;
  rdfs:domain cdi:ProvenanceInformation;
  rdfs:range cdi:FundingInformation;
.

cdi:ProvenanceInformation-provenanceStatement
  a rdf:Property, owl:ObjectProperty, ucmis:Attribute;
  rdfs:label "provenanceStatement";
  rdfs:comment "A statement of any changes in ownership and custody of the resource since its creation that are significant for its authenticity, integrity, and interpretation."@en;
  rdfs:domain cdi:ProvenanceInformation;
  rdfs:range cdi:InternationalString;
.

cdi:ProvenanceInformation-recordCreationDate
  a rdf:Property, owl:DatatypeProperty, ucmis:Attribute;
  rdfs:label "recordCreationDate";
  rdfs:comment "Date the record was created."@en;
  rdfs:domain cdi:ProvenanceInformation;
  rdfs:range xsd:date;
.

cdi:ProvenanceInformation-recordLastRevisionDate
  a rdf:Property, owl:DatatypeProperty, ucmis:Attribute;
  rdfs:label "recordLastRevisionDate";
  rdfs:comment "Date the record was last revised."@en;
  rdfs:domain cdi:ProvenanceInformation;
  rdfs:range xsd:date;
.


# datatype RationaleDefinition
# based on the UML data type DDICDIModels::DDICDILibrary::DataTypes::StructuredDataTypes::RationaleDefinition
cdi:RationaleDefinition
  a rdfs:Class, owl:Class, ucmis:StructuredDataType;
  rdfs:label "RationaleDefinition";
  rdfs:comment "Definition\n============\nTextual description of the rationale/purpose for the version change and a coded value to provide an internal processing flag within and organization or system."@en;
  
  owl:hasKey (cdi:RationaleDefinition-rationaleCode cdi:RationaleDefinition-rationaleDescription);
.

cdi:RationaleDefinition-rationaleCode
  a rdf:Property, owl:ObjectProperty, ucmis:Attribute;
  rdfs:label "rationaleCode";
  rdfs:comment "Rationale  ode is primarily for internal processing flags within an organization or system. Supports the use of an external controlled vocabulary."@en;
  rdfs:domain cdi:RationaleDefinition;
  rdfs:range cdi:ControlledVocabularyEntry;
.

cdi:RationaleDefinition-rationaleDescription
  a rdf:Property, owl:ObjectProperty, ucmis:Attribute;
  rdfs:label "rationaleDescription";
  rdfs:comment "Textual description of the rationale/purpose for the version change to inform users as to the extent and implication of the version change. May be expressed in multiple languages."@en;
  rdfs:domain cdi:RationaleDefinition;
  rdfs:range cdi:InternationalString;
.


# datatype Reference
# based on the UML data type DDICDIModels::DDICDILibrary::DataTypes::StructuredDataTypes::Reference
cdi:Reference
  a rdfs:Class, owl:Class, ucmis:StructuredDataType;
  rdfs:label "Reference";
  rdfs:comment "Definition\n============\nProvides a way of pointing to resources outside of the information described in the set of DDI-CDI metadata."@en;
  
  owl:hasKey (cdi:Reference-ddiReference cdi:Reference-deepLink cdi:Reference-description cdi:Reference-location cdi:Reference-nonDdiReference cdi:Reference-semantic cdi:Reference-uri cdi:Reference-validType);
.

cdi:Reference-ddiReference
  a rdf:Property, owl:ObjectProperty, ucmis:Attribute;
  rdfs:label "ddiReference";
  rdfs:comment "A DDI type reference to a DDI object."@en;
  rdfs:domain cdi:Reference;
  rdfs:range cdi:InternationalRegistrationDataIdentifier;
.

cdi:Reference-deepLink
  a rdf:Property, owl:ObjectProperty, ucmis:Attribute;
  rdfs:label "deepLink";
  rdfs:comment "The selector refers to the object identifier by the ddiReference and has deep linking purposes."@en;
  rdfs:domain cdi:Reference;
  rdfs:range cdi:Selector;
.

cdi:Reference-description
  a rdf:Property, owl:DatatypeProperty, ucmis:Attribute;
  rdfs:label "description";
  rdfs:comment "Human-readable description of the reference."@en;
  rdfs:domain cdi:Reference;
  rdfs:range xsd:string;
.

cdi:Reference-location
  a rdf:Property, owl:ObjectProperty, ucmis:Attribute;
  rdfs:label "location";
  rdfs:comment "The location of the referenced resource, as appropriate to support retrieval."@en;
  rdfs:domain cdi:Reference;
  rdfs:range cdi:InternationalString;
.

cdi:Reference-nonDdiReference
  a rdf:Property, owl:ObjectProperty, ucmis:Attribute;
  rdfs:label "nonDdiReference";
  rdfs:comment "A non-DDI reference to any object using a system of identification which is not supported by a URI."@en;
  rdfs:domain cdi:Reference;
  rdfs:range cdi:NonDdiIdentifier;
.

cdi:Reference-semantic
  a rdf:Property, owl:ObjectProperty, ucmis:Attribute;
  rdfs:label "semantic";
  rdfs:comment "External qualifier to describe the purpose or meaning of the reference."@en;
  rdfs:domain cdi:Reference;
  rdfs:range cdi:ControlledVocabularyEntry;
.

cdi:Reference-uri
  a rdf:Property, owl:DatatypeProperty, ucmis:Attribute;
  rdfs:label "uri";
  rdfs:comment "A URI to any object."@en;
  rdfs:domain cdi:Reference;
  rdfs:range xsd:anyURI;
.

cdi:Reference-validType
  a rdf:Property, owl:DatatypeProperty, ucmis:Attribute;
  rdfs:label "validType";
  rdfs:comment "The expected type of the reference (e.g., the class or element according to the schema of the referenced resource)."@en;
  rdfs:domain cdi:Reference;
  rdfs:range xsd:string;
.


# datatype Selector
# based on the UML data type DDICDIModels::DDICDILibrary::DataTypes::StructuredDataTypes::Selector
cdi:Selector
  a rdfs:Class, owl:Class, ucmis:StructuredDataType;
  rdfs:label "Selector";
  rdfs:comment "Definition\n==========\nA resource which describes the segment of interest in a representation of a resource. This class is not used directly, only its subclasses. It is defined accordingly the related selector of the Web Annotation Vocabulary, see https://www.w3.org/TR/annotation-vocab/#selector."@en;
  
  owl:hasKey ();
.


# datatype SpatialCoordinate
# based on the UML data type DDICDIModels::DDICDILibrary::DataTypes::StructuredDataTypes::SpatialCoordinate
cdi:SpatialCoordinate
  a rdfs:Class, owl:Class, ucmis:StructuredDataType;
  rdfs:label "SpatialCoordinate";
  rdfs:comment "Definition\n============\nLists the value and format type for the coordinate value. Note that this is a single value (X coordinate or Y coordinate) rather than a coordinate pair."@en;
  
  owl:hasKey (cdi:SpatialCoordinate-content cdi:SpatialCoordinate-coordinateType);
.

cdi:SpatialCoordinate-content
  a rdf:Property, owl:DatatypeProperty, ucmis:Attribute;
  rdfs:label "content";
  rdfs:comment "The value of the coordinate expressed as a string."@en;
  rdfs:domain cdi:SpatialCoordinate;
  rdfs:range xsd:string;
.

cdi:SpatialCoordinate-coordinateType
  a rdf:Property, owl:ObjectProperty, ucmis:Attribute;
  rdfs:label "coordinateType";
  rdfs:comment "Identifies the type of point coordinate system using a controlled vocabulary. Point formats include decimal degree, degrees minutes seconds, decimal minutes, meters, and feet."@en;
  rdfs:domain cdi:SpatialCoordinate;
  rdfs:range cdi:PointFormat;
.


# datatype SpatialPoint
# based on the UML data type DDICDIModels::DDICDILibrary::DataTypes::StructuredDataTypes::SpatialPoint
cdi:SpatialPoint
  a rdfs:Class, owl:Class, ucmis:StructuredDataType;
  rdfs:label "SpatialPoint";
  rdfs:comment "Definition\n============\nA geographic point consisting of an X and Y coordinate. Each coordinate value is expressed separately providing its value and format."@en;
  
  owl:hasKey (cdi:SpatialPoint-xCoordinate cdi:SpatialPoint-yCoordinate);
.

cdi:SpatialPoint-xCoordinate
  a rdf:Property, owl:ObjectProperty, ucmis:Attribute;
  rdfs:label "xCoordinate";
  rdfs:comment "An X coordinate (latitudinal equivalent) value and format expressed using the Spatial Coordinate structure."@en;
  rdfs:domain cdi:SpatialPoint;
  rdfs:range cdi:SpatialCoordinate;
.

cdi:SpatialPoint-yCoordinate
  a rdf:Property, owl:ObjectProperty, ucmis:Attribute;
  rdfs:label "yCoordinate";
  rdfs:comment "A Y coordinate (longitudinal equivalent) value and format expressed using the Spatial Coordinate structure."@en;
  rdfs:domain cdi:SpatialPoint;
  rdfs:range cdi:SpatialCoordinate;
.


# datatype SpecializationRole
# based on the UML data type DDICDIModels::DDICDILibrary::DataTypes::StructuredDataTypes::SpecializationRole
cdi:SpecializationRole
  a rdfs:Class, owl:Class, ucmis:StructuredDataType;
  rdfs:label "SpecializationRole";
  rdfs:comment "Definition\n============\nSpecific roles played by represented variables in terms of time, geography, and other concepts which are important for the harmonization and integration of data."@en;
  
  owl:hasKey ();
.


# datatype Statistic
# based on the UML data type DDICDIModels::DDICDILibrary::DataTypes::StructuredDataTypes::Statistic
cdi:Statistic
  a rdfs:Class, owl:Class, ucmis:StructuredDataType;
  rdfs:label "Statistic";
  rdfs:comment "Definition\n============\nThe value of the statistic expressed as a decimal, float and/or double. Indicates whether it is weighted value and the computation base."@en;
  
  owl:hasKey (cdi:Statistic-computationBase cdi:Statistic-content cdi:Statistic-isWeighted cdi:Statistic-typeOfNumericValue);
.

cdi:Statistic-computationBase
  a rdf:Property, owl:ObjectProperty, ucmis:Attribute;
  rdfs:label "computationBase";
  rdfs:comment "Defines the cases included in determining the statistic. The options are total = all cases, valid and missing (invalid); validOnly = Only valid values, missing (invalid) are not included in the calculation; missingOnly = Only missing (invalid) cases included in the calculation."@en;
  rdfs:domain cdi:Statistic;
  rdfs:range cdi:ComputationBaseList;
.

cdi:Statistic-content
  a rdf:Property, owl:DatatypeProperty, ucmis:Attribute;
  rdfs:label "content";
  rdfs:comment "The value of the statistic expressed as a real number."@en;
  rdfs:domain cdi:Statistic;
  rdfs:range xsd:double;
.

cdi:Statistic-isWeighted
  a rdf:Property, owl:DatatypeProperty, ucmis:Attribute;
  rdfs:label "isWeighted";
  rdfs:comment "Set to True if the statistic is weighted."@en;
  rdfs:domain cdi:Statistic;
  rdfs:range xsd:boolean;
.

cdi:Statistic-typeOfNumericValue
  a rdf:Property, owl:DatatypeProperty, ucmis:Attribute;
  rdfs:label "typeOfNumericValue";
  rdfs:comment "Indicate the type of numeric value as decimal, float, double."@en;
  rdfs:domain cdi:Statistic;
  rdfs:range xsd:string;
.


# datatype StructureSpecification
# based on the UML data type DDICDIModels::DDICDILibrary::DataTypes::StructuredDataTypes::StructureSpecification
cdi:StructureSpecification
  a rdfs:Class, owl:Class, ucmis:StructuredDataType;
  rdfs:label "StructureSpecification";
  rdfs:comment "Definition\n============\nThe mathematical properties of the structure."@en;
  
  owl:hasKey (cdi:StructureSpecification-reflexive cdi:StructureSpecification-symmetric cdi:StructureSpecification-transitive);
.

cdi:StructureSpecification-reflexive
  a rdf:Property, owl:ObjectProperty, ucmis:Attribute;
  rdfs:label "reflexive";
  rdfs:comment "Members of the selected scope of the collection are related to themselves."@en;
  rdfs:domain cdi:StructureSpecification;
  rdfs:range cdi:MemberRelationshipScope;
.

cdi:StructureSpecification-symmetric
  a rdf:Property, owl:ObjectProperty, ucmis:Attribute;
  rdfs:label "symmetric";
  rdfs:comment "For pairs of members, a, b in the indicated scope of the associated collection, whenever a is related to b then also b is related to a."@en;
  rdfs:domain cdi:StructureSpecification;
  rdfs:range cdi:MemberRelationshipScope;
.

cdi:StructureSpecification-transitive
  a rdf:Property, owl:ObjectProperty, ucmis:Attribute;
  rdfs:label "transitive";
  rdfs:comment "For members a, b, c in the indicated scope of the associated collection, whenever a is related to b and b is related to c then a is also related to c."@en;
  rdfs:domain cdi:StructureSpecification;
  rdfs:range cdi:MemberRelationshipScope;
.


# datatype Telephone
# based on the UML data type DDICDIModels::DDICDILibrary::DataTypes::StructuredDataTypes::Telephone
cdi:Telephone
  a rdfs:Class, owl:Class, ucmis:StructuredDataType;
  rdfs:label "Telephone";
  rdfs:comment "Definition\n============\nDetails of a telephone number including the number, type of telephone number, a privacy setting and an indication of whether this is the preferred contact number.\n\nExamples\n==========\n+12 345 67890123"@en;
  
  owl:hasKey (cdi:Telephone-effectiveDates cdi:Telephone-isPreferred cdi:Telephone-privacy cdi:Telephone-telephoneNumber cdi:Telephone-typeOfTelephone);
.

cdi:Telephone-effectiveDates
  a rdf:Property, owl:ObjectProperty, ucmis:Attribute;
  rdfs:label "effectiveDates";
  rdfs:comment "Time period during which the telephone number is valid."@en;
  rdfs:domain cdi:Telephone;
  rdfs:range cdi:DateRange;
.

cdi:Telephone-isPreferred
  a rdf:Property, owl:DatatypeProperty, ucmis:Attribute;
  rdfs:label "isPreferred";
  rdfs:comment "Set to True if this is the preferred telephone number for contact."@en;
  rdfs:domain cdi:Telephone;
  rdfs:range xsd:boolean;
.

cdi:Telephone-privacy
  a rdf:Property, owl:ObjectProperty, ucmis:Attribute;
  rdfs:label "privacy";
  rdfs:comment "Specify the level privacy for the telephone number as public, restricted, or private. Supports the use of an external controlled vocabulary."@en;
  rdfs:domain cdi:Telephone;
  rdfs:range cdi:ControlledVocabularyEntry;
.

cdi:Telephone-telephoneNumber
  a rdf:Property, owl:DatatypeProperty, ucmis:Attribute;
  rdfs:label "telephoneNumber";
  rdfs:comment "The telephone number including country code if appropriate."@en;
  rdfs:domain cdi:Telephone;
  rdfs:range xsd:string;
.

cdi:Telephone-typeOfTelephone
  a rdf:Property, owl:ObjectProperty, ucmis:Attribute;
  rdfs:label "typeOfTelephone";
  rdfs:comment "Indicates type of telephone number provided (home, fax, office, cell, etc.). Supports the use of a controlled vocabulary."@en;
  rdfs:domain cdi:Telephone;
  rdfs:range cdi:ControlledVocabularyEntry;
.


# datatype TextPositionSelector
# based on the UML data type DDICDIModels::DDICDILibrary::DataTypes::StructuredDataTypes::TextPositionSelector
cdi:TextPositionSelector
  a rdfs:Class, owl:Class, ucmis:StructuredDataType;
  rdfs:label "TextPositionSelector";
  rdfs:comment "Definition\n==========\nDescribes a range of text by recording the start and end positions of the selection in the object. Position 0 would be immediately before the first character, position 1 would be immediately before the second character, and so on. It is defined accordingly the related selector of the Web Annotation Vocabulary, see https://www.w3.org/TR/annotation-vocab/#textpositionselector."@en;
  rdfs:subClassOf cdi:Selector;
  owl:hasKey (cdi:TextPositionSelector-end cdi:TextPositionSelector-start);
.

cdi:TextPositionSelector-end
  a rdf:Property, owl:DatatypeProperty, ucmis:Attribute;
  rdfs:label "end";
  rdfs:comment "Position of the last character of the selection. Position 8 would be the end of the word \"Position\" of the previous sentence."@en;
  rdfs:domain cdi:TextPositionSelector;
  rdfs:range xsd:integer;
.

cdi:TextPositionSelector-start
  a rdf:Property, owl:DatatypeProperty, ucmis:Attribute;
  rdfs:label "start";
  rdfs:comment "Position of the first character of the selection. Position 0 would be the start of the word \"Position\" of the previous sentence."@en;
  rdfs:domain cdi:TextPositionSelector;
  rdfs:range xsd:integer;
.


# datatype TimeRole
# based on the UML data type DDICDIModels::DDICDILibrary::DataTypes::StructuredDataTypes::TimeRole
cdi:TimeRole
  a rdfs:Class, owl:Class, ucmis:StructuredDataType;
  rdfs:label "TimeRole";
  rdfs:comment "Definition\n============\nTime-specific role given to a represented variable in the context of a data structure. The specific characterization of the role (e.g. event, valid, transaction, reference, etc.) may be given by a controlled vocabulary."@en;
  rdfs:subClassOf cdi:SpecializationRole;
  owl:hasKey (cdi:TimeRole-time);
.

cdi:TimeRole-time
  a rdf:Property, owl:ObjectProperty, ucmis:Attribute;
  rdfs:label "time";
  rdfs:comment "Holds a value from an external controlled vocabulary defining the time role."@en;
  rdfs:domain cdi:TimeRole;
  rdfs:range cdi:ControlledVocabularyEntry;
.


# datatype TypedString
# based on the UML data type DDICDIModels::DDICDILibrary::DataTypes::StructuredDataTypes::TypedString
cdi:TypedString
  a rdfs:Class, owl:Class, ucmis:StructuredDataType;
  rdfs:label "TypedString";
  rdfs:comment "Definition\n============\nTypedString combines a type with content defined as a simple string. May be used wherever a simple string needs to support a type definition to clarify its content.\n\nExamples\n==========\nContent is a regular expression and the typeOfContent attribute is used to define the syntax of the regular expression content.\n\nExplanatory notes\n===================\nThis is a generic type + string where property name and documentation should be used to define any specification for the content. If international structured string content is required use TypedStructuredString."@en;
  
  owl:hasKey (cdi:TypedString-content cdi:TypedString-typeOfContent);
.

cdi:TypedString-content
  a rdf:Property, owl:DatatypeProperty, ucmis:Attribute;
  rdfs:label "content";
  rdfs:comment "Content of the property expressed as a simple string."@en;
  rdfs:domain cdi:TypedString;
  rdfs:range xsd:string;
.

cdi:TypedString-typeOfContent
  a rdf:Property, owl:ObjectProperty, ucmis:Attribute;
  rdfs:label "typeOfContent";
  rdfs:comment "Optional use of a controlled vocabulary to specifically type the associated content."@en;
  rdfs:domain cdi:TypedString;
  rdfs:range cdi:ControlledVocabularyEntry;
.


# datatype WebLink
# based on the UML data type DDICDIModels::DDICDILibrary::DataTypes::StructuredDataTypes::WebLink
cdi:WebLink
  a rdfs:Class, owl:Class, ucmis:StructuredDataType;
  rdfs:label "WebLink";
  rdfs:comment "Definition\n============\nA web site (normally a URL) with information on type of site, privacy flag, and effective dates."@en;
  
  owl:hasKey (cdi:WebLink-effectiveDates cdi:WebLink-isPreferred cdi:WebLink-privacy cdi:WebLink-typeOfWebsite cdi:WebLink-uri);
.

cdi:WebLink-effectiveDates
  a rdf:Property, owl:ObjectProperty, ucmis:Attribute;
  rdfs:label "effectiveDates";
  rdfs:comment "The period for which this URL is valid."@en;
  rdfs:domain cdi:WebLink;
  rdfs:range cdi:DateRange;
.

cdi:WebLink-isPreferred
  a rdf:Property, owl:DatatypeProperty, ucmis:Attribute;
  rdfs:label "isPreferred";
  rdfs:comment "Set to True if this is the preferred URL."@en;
  rdfs:domain cdi:WebLink;
  rdfs:range xsd:boolean;
.

cdi:WebLink-privacy
  a rdf:Property, owl:ObjectProperty, ucmis:Attribute;
  rdfs:label "privacy";
  rdfs:comment "Indicates the privacy level of this URL."@en;
  rdfs:domain cdi:WebLink;
  rdfs:range cdi:ControlledVocabularyEntry;
.

cdi:WebLink-typeOfWebsite
  a rdf:Property, owl:ObjectProperty, ucmis:Attribute;
  rdfs:label "typeOfWebsite";
  rdfs:comment "The type of Website URL, for example personal, project, organization, division, etc."@en;
  rdfs:domain cdi:WebLink;
  rdfs:range cdi:ControlledVocabularyEntry;
.

cdi:WebLink-uri
  a rdf:Property, owl:DatatypeProperty, ucmis:Attribute;
  rdfs:label "uri";
  rdfs:comment "A Uniform Resource Identifier (URI) is a compact sequence of characters that identifies an abstract or physical resource. Normally a URL."@en;
  rdfs:domain cdi:WebLink;
  rdfs:range xsd:anyURI;
.



