# PLEASE DO NOT EDIT THIS CODE!
# This code was generated by the Eclipse Acceleo module UCMIS M2T on 2024-03-01 13:10:40.
# Target language is 'Ontology Turtle' ('onto.ttl') generated on the basis of the model 'DDICDIModels'.

# Ontology for Wide
# based on the UML package DDICDIModels::DDICDILibrary::Classes::DataDescription::Wide
@prefix rdf:   <http://www.w3.org/1999/02/22-rdf-syntax-ns#> .
@prefix rdfs:  <http://www.w3.org/2000/01/rdf-schema#> .
@prefix owl:   <http://www.w3.org/2002/07/owl#> .
@prefix xsd:   <http://www.w3.org/2001/XMLSchema#> .
@prefix dc:    <http://purl.org/dc/elements/1.1/> .
@prefix skos:  <http://www.w3.org/2004/02/skos/core#> .
@prefix ucmis: <http://example.org/TODO/ucmis/> .
@prefix cdi:   <http://ddialliance.org/Specification/DDI-CDI/1.0/RDF/> .

<Wide.onto.ttl> a owl:Ontology;
  rdfs:label "Wide";
  rdfs:comment "This package contains classes for defining \"rectangular\" data files where each unit has a series of measurements recorded for it about a regular set of variables. (Although we often think of such data as existing in rows, logically it is independent of the specific formatting, and can be seen as a repeated cluster of measures across a set of units.)"@en;
.

# class WideDataSet
# based on the UML class DDICDIModels::DDICDILibrary::Classes::DataDescription::Wide::WideDataSet
cdi:WideDataSet
  a rdfs:Class, owl:Class, ucmis:Class;
  rdfs:label "WideDataSet";
  rdfs:comment "Definition\n============\nOrganized collection of wide data. It is structured by a wide data structure.\n\nExamples\n==========\nA unit dataset where each row corresponds to a set of data points capturing different characteristics of a unit."@en;
  rdfs:subClassOf cdi:DataSet;
.



# class WideDataStructure
# based on the UML class DDICDIModels::DDICDILibrary::Classes::DataDescription::Wide::WideDataStructure
cdi:WideDataStructure
  a rdfs:Class, owl:Class, ucmis:Class;
  rdfs:label "WideDataStructure";
  rdfs:comment "Definition\n==========\nStructure of a wide dataset (organized collection of wide data). It is described by identifier, measure and attribute components.\n\nExamples\n==========\nThe structure described by [Unit id, Income, Province] where Unit id identifies a statistical unit and Income and Province are two instance variables capturing characteristics."@en;
  rdfs:subClassOf cdi:DataStructure;
.



# class WideKey
# based on the UML class DDICDIModels::DDICDILibrary::Classes::DataDescription::Wide::WideKey
cdi:WideKey
  a rdfs:Class, owl:Class, ucmis:Class;
  rdfs:label "WideKey";
  rdfs:comment "Definition\n==========\nCollection of data instances that uniquely identify a collection of data points in a wide dataset.\n\nExamples\n==========\nCollection containing the single \"1A2B3C\" string in a wide dataset where rows are identified by postal code representations."@en;
  rdfs:subClassOf cdi:Key;
.



# class WideKeyMember
# based on the UML class DDICDIModels::DDICDILibrary::Classes::DataDescription::Wide::WideKeyMember
cdi:WideKeyMember
  a rdfs:Class, owl:Class, ucmis:Class;
  rdfs:label "WideKeyMember";
  rdfs:comment "Definition \n============ \nSingle data instance that is part of a wide key.   \n\nExamples \n========== \nThe \"1A2B3C\" string in a wide dataset where rows are identified by postal code representations."@en;
  rdfs:subClassOf cdi:KeyMember;
.





