# PLEASE DO NOT EDIT THIS CODE!
# This code was generated by the Eclipse Acceleo module UCMIS M2T on 2023-05-25 10:41:35.
# Target language is 'Ontology Turtle' ('onto.ttl') generated on the basis of the model 'DDICDIModels'.

# Ontology for Wide
# based on the UML package DDICDIModels::DDICDILibrary::Classes::DataDescription::Wide
@prefix rdf:   <http://www.w3.org/1999/02/22-rdf-syntax-ns#> .
@prefix rdfs:  <http://www.w3.org/2000/01/rdf-schema#> .
@prefix owl:   <http://www.w3.org/2002/07/owl#> .
@prefix xsd:   <http://www.w3.org/2001/XMLSchema#> .
@prefix dc:    <http://purl.org/dc/elements/1.1/> .
@prefix skos:  <http://www.w3.org/2004/02/skos/core#> .
@prefix ucmis: <http://example.org/TODO/ucmis/> .
@prefix cdi:   <http://ddialliance.org/Specification/DDI-CDI/1.0/RDF/> .

<Wide.onto.ttl> a owl:Ontology;
  rdfs:label "Wide";
  rdfs:comment "This package contains classes for defining \"rectangular\" data files where each unit has a series of measurements recorded for it about a regular set of variables. (Although we often think of such data as existing in rows, logically it is independent of the specific formatting, and can be seen as a repeated cluster of measures across a set of units.)"@en;
.

# class WideDataSet
# based on the UML class DDICDIModels::DDICDILibrary::Classes::DataDescription::Wide::WideDataSet
cdi:WideDataSet
  a rdfs:Class, owl:Class, ucmis:Class;
  rdfs:label "WideDataSet";
  rdfs:comment "Definition\n============\nOrganized collection of wide data. It is structured by a wide data structure.\n\nExamples\n==========\nA unit dataset where each row corresponds to a set of data points capturing different characteristics of a unit."@en;
  rdfs:subClassOf cdi:DataSet;
.


cdi:WideDataSet_has_WideKey
  a rdf:Property, owl:ObjectProperty, ucmis:Association;
  # ASSOCIATION
  rdfs:label "has";
  skos:altLabel "WideDataSet_has_WideKey";
  
  rdfs:domain cdi:WideDataSet;
  rdfs:range cdi:WideKey;
.


# class WideDataStructure
# based on the UML class DDICDIModels::DDICDILibrary::Classes::DataDescription::Wide::WideDataStructure
cdi:WideDataStructure
  a rdfs:Class, owl:Class, ucmis:Class;
  rdfs:label "WideDataStructure";
  rdfs:comment "Definition\n==========\nStructure of a wide dataset (organized collection of wide data). It is described by identifier, measure and attribute components.\n\nExamples\n==========\nThe structure described by [Unit id, Income, Province] where Unit id identifies a statistical unit and Income and Province are two instance variables capturing characteristics."@en;
  rdfs:subClassOf cdi:DataStructure;
.



# class WideKey
# based on the UML class DDICDIModels::DDICDILibrary::Classes::DataDescription::Wide::WideKey
cdi:WideKey
  a rdfs:Class, owl:Class, ucmis:Class;
  rdfs:label "WideKey";
  rdfs:comment "Definition\n==========\nCollection of data instances that uniquely identify a collection of data points in a wide dataset.\n\nExamples\n==========\nCollection containing the single \"1A2B3C\" string in a wide dataset where rows are identified by postal code representations."@en;
  
.

cdi:WideKey-identifier
  a rdf:Property, owl:ObjectProperty, ucmis:Attribute;
  rdfs:label "identifier";
  rdfs:comment "Identifier for objects requiring short- or long-lasting referencing and management."@en;
  rdfs:domain cdi:WideKey;
  rdfs:range cdi:Identifier;
.


cdi:WideKey_correspondsTo_Unit
  a rdf:Property, owl:ObjectProperty, ucmis:Association;
  # ASSOCIATION
  rdfs:label "correspondsTo";
  skos:altLabel "WideKey_correspondsTo_Unit";
  rdfs:comment "Wide key corresponds to zero to one unit."@en;
  rdfs:domain cdi:WideKey;
  rdfs:range cdi:Unit;
.

cdi:WideKey_identifies_DataPoint
  a rdf:Property, owl:ObjectProperty, ucmis:Association;
  # ASSOCIATION
  rdfs:label "identifies";
  skos:altLabel "WideKey_identifies_DataPoint";
  
  rdfs:domain cdi:WideKey;
  rdfs:range cdi:DataPoint;
.

cdi:WideKey_has_WideKeyMember
  a rdf:Property, owl:ObjectProperty, ucmis:Association;
  # ASSOCIATION
  rdfs:label "has";
  skos:altLabel "WideKey_has_WideKeyMember";
  
  rdfs:domain cdi:WideKey;
  rdfs:range cdi:WideKeyMember;
.


# class WideKeyMember
# based on the UML class DDICDIModels::DDICDILibrary::Classes::DataDescription::Wide::WideKeyMember
cdi:WideKeyMember
  a rdfs:Class, owl:Class, ucmis:Class;
  rdfs:label "WideKeyMember";
  rdfs:comment "Definition \n============ \nSingle data instance that is part of a wide key.   \n\nExamples \n========== \nThe \"1A2B3C\" string in a wide dataset where rows are identified by postal code representations."@en;
  rdfs:subClassOf cdi:InstanceValue;
.


cdi:WideKeyMember_isBasedOn_IdentifierComponent
  a rdf:Property, owl:ObjectProperty, ucmis:Association;
  # ASSOCIATION
  rdfs:label "isBasedOn";
  skos:altLabel "WideKeyMember_isBasedOn_IdentifierComponent";
  
  rdfs:domain cdi:WideKeyMember;
  rdfs:range cdi:IdentifierComponent;
.




